@prefix cidoc_crm: <http://www.cidoc-crm.org/cidoc-crm/> .
@prefix ns1: <http://www.w3.org/2004/02/skos/core#> .
@prefix ontohgis: <http://purl.org/ontohgis#> .
@prefix owl: <http://www.w3.org/2002/07/owl#> .
@prefix rdfs: <http://www.w3.org/2000/01/rdf-schema#> .
@prefix urbanonto: <https://purl.org/urbanonto#> .
@prefix xsd: <http://www.w3.org/2001/XMLSchema#> .

ontohgis:object_10 rdfs:subClassOf cidoc_crm:E24_Physical_Man-Made_Thing .

ontohgis:object_20 rdfs:subClassOf cidoc_crm:E22_Man-Made_Object .

ontohgis:object_200 rdfs:subClassOf cidoc_crm:E22_Man-Made_Object .

ontohgis:object_21 rdfs:subClassOf cidoc_crm:E90_Symbolic_Object .

ontohgis:object_30 rdfs:subClassOf cidoc_crm:E22_Man-Made_Object .

ontohgis:object_31 rdfs:subClassOf cidoc_crm:E48_Place_Name .

ontohgis:object_40 rdfs:subClassOf cidoc_crm:E22_Man-Made_Object .

ontohgis:object_60 rdfs:subClassOf cidoc_crm:E41_Appellation .

ontohgis:object_800 rdfs:subClassOf cidoc_crm:E73_Information_Object .

ontohgis:settlement_unit2000 rdfs:subClassOf cidoc_crm:E25_Man-Made_Feature .

ontohgis:settlement_unit2001 rdfs:subClassOf cidoc_crm:E25_Man-Made_Feature .

ontohgis:source rdfs:subClassOf cidoc_crm:E31_Document .

cidoc_crm:E27_Site a owl:Class ;
    rdfs:label "Gelände"@de,
        "Φυσικός Χώρος"@el,
        "Site"@en,
        "Site"@fr,
        "Lugar"@pt,
        "Участок"@ru,
        "场地"@zh ;
    rdfs:comment """This class comprises pieces of land or sea floor. \r
In contrast to the purely geometric notion of E53 Place, this class describes constellations of matter on the surface of the Earth or other celestial body, which can be represented by photographs, paintings and maps.\r
 Instances of E27 Site are composed of relatively immobile material items and features in a particular configuration at a particular location"""@en ;
    rdfs:subClassOf cidoc_crm:E26_Physical_Feature .

cidoc_crm:E34_Inscription a owl:Class ;
    rdfs:label "Inschrift"@de,
        "Επιγραφή"@el,
        "Inscription"@en,
        "Inscription"@fr,
        "Inscrição"@pt,
        "Надпись"@ru,
        "题字"@zh ;
    rdfs:comment """This class comprises recognisable, short texts attached to instances of E24 Physical Man-Made Thing. \r
The transcription of the text can be documented in a note by P3 has note: E62 String. The alphabet used can be documented by P2 has type: E55 Type. This class does not intend to describe the idiosyncratic characteristics of an individual physical embodiment of an inscription, but the underlying prototype. The physical embodiment is modelled in the CRM as E24 Physical Man-Made Thing.\r
The relationship of a physical copy of a book to the text it contains is modelled using E84 Information Carrier. P128 carries (is carried by): E33 Linguistic Object. \r
"""@en ;
    rdfs:subClassOf cidoc_crm:E33_Linguistic_Object,
        cidoc_crm:E37_Mark .

cidoc_crm:E38_Image a owl:Class ;
    rdfs:label "Bild"@de,
        "Εικόνα"@el,
        "Image"@en,
        "Image"@fr,
        "Imagem"@pt,
        "Изображение"@ru,
        "图像"@zh ;
    rdfs:comment """This class comprises distributions of form, tone and colour that may be found on surfaces such as photos, paintings, prints and sculptures or directly on electronic media. \r
The degree to which variations in the distribution of form and colour affect the identity of an instance of E38 Image depends on a given purpose. The original painting of the Mona Lisa in the Louvre may be said to bear the same instance of E38 Image as reproductions in the form of transparencies, postcards, posters or T-shirts, even though they may differ in size and carrier and may vary in tone and colour. The images in a “spot the difference” competition are not the same with respect to their context, however similar they may at first appear.\r
"""@en ;
    rdfs:subClassOf cidoc_crm:E36_Visual_Item .

cidoc_crm:E40_Legal_Body a owl:Class ;
    rdfs:label "Juristische Person"@de,
        "Νομικό Πρόσωπο"@el,
        "Legal Body"@en,
        "Collectivité"@fr,
        "Pessoa Jurídica"@pt,
        "Юридическое Лицо"@ru,
        "法律组织"@zh ;
    rdfs:comment """This class comprises institutions or groups of people that have obtained a legal recognition as a group and can act collectively as agents.  \r
This means that they can perform actions, own property, create or destroy things and can be held collectively responsible for their actions like individual people. The term 'personne morale' is often used for this in French. \r
"""@en ;
    rdfs:subClassOf cidoc_crm:E74_Group .

cidoc_crm:E45_Address a owl:Class ;
    rdfs:label "Adresse"@de,
        "Διεύθυνση"@el,
        "Address"@en,
        "Adresse"@fr,
        "Endereço"@pt,
        "Адрес"@ru,
        "地址"@zh ;
    rdfs:comment """This class comprises identifiers expressed in coding systems for places, such as postal addresses used for mailing.\r
An E45 Address can be considered both as the name of an E53 Place and as an E51 Contact Point for an E39 Actor. This dual aspect is reflected in the multiple inheritance. However, some forms of mailing addresses, such as a postal box, are only instances of E51 Contact Point, since they do not identify any particular Place. These should not be documented as instances of E45 Address.\r
"""@en ;
    rdfs:subClassOf cidoc_crm:E44_Place_Appellation,
        cidoc_crm:E51_Contact_Point .

cidoc_crm:E47_Spatial_Coordinates a owl:Class ;
    rdfs:label "Raumkoordinaten"@de,
        "Χωρικές Συντεταγμένες"@el,
        "Spatial Coordinates"@en,
        "Coordonnées spatiales"@fr,
        "Coordenadas Espaciais"@pt,
        "Пространственные Координаты"@ru,
        "空间坐标"@zh ;
    rdfs:comment """This class comprises the textual or numeric information required to locate specific instances of E53 Place within schemes of spatial identification. \r
\r
Coordinates are a specific form of E44 Place Appellation, that is, a means of referring to a particular E53 Place. Coordinates are not restricted to longitude, latitude and altitude. Any regular system of reference that maps onto an E19 Physical Object can be used to generate coordinates.\r
"""@en ;
    rdfs:subClassOf cidoc_crm:E44_Place_Appellation .

cidoc_crm:E50_Date a owl:Class ;
    rdfs:label "Datum"@de,
        "Ημερομηνία"@el,
        "Date"@en,
        "Date"@fr,
        "Data"@pt,
        "Дата"@ru,
        "日期"@zh ;
    rdfs:comment "This class comprises specific forms of E49 Time Appellation."@en ;
    rdfs:subClassOf cidoc_crm:E49_Time_Appellation .

cidoc_crm:E84_Information_Carrier a owl:Class ;
    rdfs:label "Informationsträger"@de,
        "Φορέας Πληροφορίας"@el,
        "Information Carrier"@en,
        "Support d'information"@fr,
        "Suporte de Informação"@pt,
        "Носитель Информации"@ru,
        "信息载体"@zh ;
    rdfs:comment """This class comprises all instances of E22 Man-Made Object that are explicitly designed to act as persistent physical carriers for instances of E73 Information Object.\r
An E84 Information Carrier may or may not contain information, e.g., a diskette. Note that any E18 Physical Thing may carry information, such as an E34 Inscription. However, unless it was specifically designed for this purpose, it is not an Information Carrier. Therefore the property P128 carries (is carried by) applies to E18 Physical Thing in general.\r
	"""@en ;
    rdfs:subClassOf cidoc_crm:E22_Man-Made_Object .

cidoc_crm:P100_was_death_of a owl:ObjectProperty ;
    rdfs:label "Tod von"@de,
        "ήταν θάνατος του/της"@el,
        "was death of"@en,
        "a été la mort de"@fr,
        "foi a morte para "@pt,
        "был смертью для"@ru,
        "灭亡了"@zh ;
    rdfs:comment "This property property links an E69 Death event to the E21 Person that died."@en ;
    rdfs:domain cidoc_crm:E69_Death ;
    rdfs:range cidoc_crm:E21_Person ;
    rdfs:subPropertyOf cidoc_crm:P93_took_out_of_existence .

cidoc_crm:P100i_died_in a owl:ObjectProperty ;
    rdfs:label "starb in"@de,
        "πέθανε σε"@el,
        "died in"@en,
        "est mort par"@fr,
        "morreu em"@pt,
        "умер в"@ru,
        "死亡於"@zh ;
    rdfs:domain cidoc_crm:E21_Person ;
    rdfs:range cidoc_crm:E69_Death ;
    rdfs:subPropertyOf cidoc_crm:P93i_was_taken_out_of_existence_by .

cidoc_crm:P101_had_as_general_use a owl:ObjectProperty ;
    rdfs:label "hatte die allgemeine Verwendung"@de,
        "είχε ως γενική χρήση"@el,
        "had as general use"@en,
        "avait comme utilisation générale"@fr,
        "tem como uso geral"@pt,
        "имел основное применение"@ru,
        "被惯用於"@zh ;
    rdfs:comment """This property links an instance of E70 Thing to an E55 Type of usage.\r
It allows the relationship between particular things, both physical and immaterial, and general methods and techniques of use to be documented. Thus it can be asserted that a baseball bat had a general use for sport and a specific use for threatening people during the Great Train Robbery.\r
"""@en ;
    rdfs:domain cidoc_crm:E70_Thing ;
    rdfs:range cidoc_crm:E55_Type .

cidoc_crm:P101i_was_use_of a owl:ObjectProperty ;
    rdfs:label "war die Verwendung von"@de,
        "ήταν χρήση του/της"@el,
        "was use of"@en,
        "était l’utilisation de"@fr,
        "foi uso de"@pt,
        "был применением для"@ru,
        "可使用"@zh ;
    rdfs:domain cidoc_crm:E55_Type ;
    rdfs:range cidoc_crm:E70_Thing .

cidoc_crm:P102_has_title a owl:ObjectProperty ;
    rdfs:label "trägt den Titel"@de,
        "έχει τίτλο"@el,
        "has title"@en,
        "a pour titre"@fr,
        "tem título"@pt,
        "имеет заголовок"@ru,
        "有标题"@zh ;
    rdfs:comment """This property describes the E35 Title applied to an instance of E71 Man-Made Thing. The E55 Type of Title is assigned in a sub property.\r
The P102.1 has type property of the P102 has title (is title of) property enables the relationship between the Title and the thing to be further clarified, for example, if the Title was a given Title, a supplied Title etc.\r
It allows any man-made material or immaterial thing to be given a Title. It is possible to imagine a Title being created without a specific object in mind.\r
"""@en ;
    rdfs:domain cidoc_crm:E71_Man-Made_Thing ;
    rdfs:range cidoc_crm:E35_Title ;
    rdfs:subPropertyOf cidoc_crm:P1_is_identified_by .

cidoc_crm:P102i_is_title_of a owl:ObjectProperty ;
    rdfs:label "ist der Titel von"@de,
        "είναι τίτλος του/της"@el,
        "is title of"@en,
        "est le titre de"@fr,
        "é título de"@pt,
        "является заголовком для"@ru,
        "被用为标题来称呼"@zh ;
    rdfs:domain cidoc_crm:E35_Title ;
    rdfs:range cidoc_crm:E71_Man-Made_Thing ;
    rdfs:subPropertyOf cidoc_crm:P1i_identifies .

cidoc_crm:P103_was_intended_for a owl:ObjectProperty ;
    rdfs:label "bestimmt für"@de,
        "προοριζόταν για"@el,
        "was intended for"@en,
        "était destiné à"@fr,
        "era destinado à"@pt,
        "был задуман для"@ru,
        "被制作来用於"@zh ;
    rdfs:comment """This property links an instance of E71 Man-Made Thing to an E55 Type of usage. \r
It creates a property between specific man-made things, both physical and immaterial, to Types of intended methods and techniques of use. Note: A link between specific man-made things and a specific use activity should be expressed using P19 was intended use of (was made for)."""@en ;
    rdfs:domain cidoc_crm:E71_Man-Made_Thing ;
    rdfs:range cidoc_crm:E55_Type .

cidoc_crm:P103i_was_intention_of a owl:ObjectProperty ;
    rdfs:label "war Bestimmung von"@de,
        "ήταν προορισμός του"@el,
        "was intention of"@en,
        "était la raison d'être de"@fr,
        "era a destinação de"@pt,
        "был интенцией для"@ru ;
    rdfs:domain cidoc_crm:E55_Type ;
    rdfs:range cidoc_crm:E71_Man-Made_Thing .

cidoc_crm:P104_is_subject_to a owl:ObjectProperty ;
    rdfs:label "Gegenstand von"@de,
        "υπόκειται σε"@el,
        "is subject to"@en,
        "est sujet à"@fr,
        "está sujeito à"@pt,
        "является объектом для"@ru,
        "受制於"@zh ;
    rdfs:comment """This property links a particular E72 Legal Object to the instances of E30 Right to which it is subject.\r
The Right is held by an E39 Actor as described by P75 possesses (is possessed by).\r
"""@en ;
    rdfs:domain cidoc_crm:E72_Legal_Object ;
    rdfs:range cidoc_crm:E30_Right .

cidoc_crm:P104i_applies_to a owl:ObjectProperty ;
    rdfs:label "findet Anwendung auf"@de,
        "ισχύει για"@el,
        "applies to"@en,
        "s’applique à"@fr,
        "se aplicam à"@pt,
        "применяется к"@ru,
        "被应用於"@zh ;
    rdfs:domain cidoc_crm:E30_Right ;
    rdfs:range cidoc_crm:E72_Legal_Object .

cidoc_crm:P107_has_current_or_former_member a owl:ObjectProperty ;
    rdfs:label "hat derzeitiges oder früheres Mitglied"@de,
        "έχει ή είχε μέλος"@el,
        "has current or former member"@en,
        "a pour membre actuel ou ancien"@fr,
        "tem ou teve membro"@pt,
        "имеет действующего или бывшего члена"@ru,
        "有现任或前任成员"@zh ;
    rdfs:comment """This property relates an E39 Actor to the E74 Group of which that E39 Actor is a member.\r
Groups, Legal Bodies and Persons, may all be members of Groups. A Group necessarily consists of more than one member.\r
This property is a shortcut of the more fully developed path from E74 Group through P144 joined with (gained member by), E85 Joining, P143 joined (was joined by) to E39 Actor\r
The property P107.1 kind of member can be used to specify the type of membership or the role the member has in the group. \r
"""@en ;
    rdfs:domain cidoc_crm:E74_Group ;
    rdfs:range cidoc_crm:E39_Actor .

cidoc_crm:P107i_is_current_or_former_member_of a owl:ObjectProperty ;
    rdfs:label "ist derzeitiges oder früheres Mitglied von"@de,
        "είναι ή ήταν μέλος του/της"@el,
        "is current or former member of"@en,
        "est actuel ou ancien membre de"@fr,
        "é ou foi membro de"@pt,
        "является действующим или бывшим членом"@ru,
        "目前或曾经加入群组"@zh ;
    rdfs:domain cidoc_crm:E39_Actor ;
    rdfs:range cidoc_crm:E74_Group .

cidoc_crm:P108_has_produced a owl:ObjectProperty ;
    rdfs:label "hat hergestellt"@de,
        "παρήγαγε"@el,
        "has produced"@en,
        "a produit"@fr,
        "produziu"@pt,
        "произвел"@ru,
        "有产出物"@zh ;
    rdfs:comment """This property identifies the E24 Physical Man-Made Thing that came into existence as a result of an E12 Production.\r
The identity of an instance of E24 Physical Man-Made Thing is not defined by its matter, but by its existence as a subject of documentation. An E12 Production can result in the creation of multiple instances of E24 Physical Man-Made Thing.\r
"""@en ;
    rdfs:domain cidoc_crm:E12_Production ;
    rdfs:range cidoc_crm:E24_Physical_Man-Made_Thing ;
    rdfs:subPropertyOf cidoc_crm:P31_has_modified,
        cidoc_crm:P92_brought_into_existence .

cidoc_crm:P108i_was_produced_by a owl:ObjectProperty ;
    rdfs:label "wurde hergestellt durch"@de,
        "παρήχθη από"@el,
        "was produced by"@en,
        "a été produit par"@fr,
        "foi produzido por"@pt,
        "был произведен посредством"@ru,
        "被制作於"@zh ;
    rdfs:domain cidoc_crm:E24_Physical_Man-Made_Thing ;
    rdfs:range cidoc_crm:E12_Production ;
    rdfs:subPropertyOf cidoc_crm:P31i_was_modified_by,
        cidoc_crm:P92i_was_brought_into_existence_by .

cidoc_crm:P109_has_current_or_former_curator a owl:ObjectProperty ;
    rdfs:label "hat derzeitigen oder früheren Kurator"@de,
        "έχει ή είχε επιμελητή"@el,
        "has current or former curator"@en,
        "a pour conservateur actuel ou ancien"@fr,
        "tem ou teve curador"@pt,
        "имеет действующего или бывшего хранителя"@ru,
        "有现任或前任典藏管理员"@zh ;
    rdfs:comment """This property identifies the E39 Actor or Actors who assume or have assumed overall curatorial responsibility for an E78 Collection.\r
\r
It does not allow a history of curation to be recorded. This would require use of an Event  initiating a curator being responsible for  a Collection.\r
"""@en ;
    rdfs:domain cidoc_crm:E78_Collection ;
    rdfs:range cidoc_crm:E39_Actor ;
    rdfs:subPropertyOf cidoc_crm:P49_has_former_or_current_keeper .

cidoc_crm:P109i_is_current_or_former_curator_of a owl:ObjectProperty ;
    rdfs:label "ist derzeitiger oder früherer Kurator von"@de,
        "είναι ή ήταν επιμελητής του/της"@el,
        "is current or former curator of"@en,
        "est ou a été le conservateur de"@fr,
        "é ou foi curador de"@pt,
        "является действующим или бывшим хранителем"@ru,
        "目前或曾经典藏管理"@zh ;
    rdfs:domain cidoc_crm:E39_Actor ;
    rdfs:range cidoc_crm:E78_Collection ;
    rdfs:subPropertyOf cidoc_crm:P49i_is_former_or_current_keeper_of .

cidoc_crm:P110_augmented a owl:ObjectProperty ;
    rdfs:label "erweiterte"@de,
        "επαύξησε"@el,
        "augmented"@en,
        "a augmenté"@fr,
        "aumentou"@pt,
        "увеличил"@ru,
        "扩增了"@zh ;
    rdfs:comment """This property identifies the E24 Physical Man-Made Thing that is added to (augmented) in an E79 Part Addition.\r
Although a Part Addition event normally concerns only one item of Physical Man-Made Thing, it is possible to imagine circumstances under which more than one item might be added to (augmented). For example, the artist Jackson Pollock trailing paint onto multiple canvasses.\r
"""@en ;
    rdfs:domain cidoc_crm:E79_Part_Addition ;
    rdfs:range cidoc_crm:E24_Physical_Man-Made_Thing ;
    rdfs:subPropertyOf cidoc_crm:P31_has_modified .

cidoc_crm:P110i_was_augmented_by a owl:ObjectProperty ;
    rdfs:label "wurde erweitert durch"@de,
        "επαυξήθηκε από"@el,
        "was augmented by"@en,
        "a été augmenté par"@fr,
        "foi aumentada por"@pt,
        "был увеличен посредством"@ru,
        "被扩增於"@zh ;
    rdfs:domain cidoc_crm:E24_Physical_Man-Made_Thing ;
    rdfs:range cidoc_crm:E79_Part_Addition ;
    rdfs:subPropertyOf cidoc_crm:P31i_was_modified_by .

cidoc_crm:P111_added a owl:ObjectProperty ;
    rdfs:label "fügte hinzu"@de,
        "προσέθεσε"@el,
        "added"@en,
        "a ajouté"@fr,
        "adicionou"@pt,
        "добавил"@ru,
        "附加上部件"@zh ;
    rdfs:comment """This property identifies the E18 Physical Thing that is added during an E79 Part Addition activity\r
"""@en ;
    rdfs:domain cidoc_crm:E79_Part_Addition ;
    rdfs:range cidoc_crm:E18_Physical_Thing ;
    rdfs:subPropertyOf cidoc_crm:P12_occurred_in_the_presence_of,
        cidoc_crm:P16_used_specific_object .

cidoc_crm:P111i_was_added_by a owl:ObjectProperty ;
    rdfs:label "wurde hinzugefügt durch"@de,
        "προστέθηκε από"@el,
        "was added by"@en,
        "a été ajouté par"@fr,
        "foi adicionado por"@pt,
        "был добавлен посредством"@ru,
        "被附加於"@zh ;
    rdfs:domain cidoc_crm:E18_Physical_Thing ;
    rdfs:range cidoc_crm:E79_Part_Addition ;
    rdfs:subPropertyOf cidoc_crm:P12i_was_present_at,
        cidoc_crm:P16i_was_used_for .

cidoc_crm:P112_diminished a owl:ObjectProperty ;
    rdfs:label "verminderte"@de,
        "εξάλειψε"@el,
        "diminished"@en,
        "a diminué"@fr,
        "diminuiu"@pt,
        "уменьшил"@ru,
        "缩减了"@zh ;
    rdfs:comment """This property identifies the E24 Physical Man-Made Thing that was diminished by E80 Part Removal.\r
Although a Part removal activity normally concerns only one item of Physical Man-Made Thing, it is possible to imagine circumstances under which more than one item might be diminished by a single Part Removal activity. \r
"""@en ;
    rdfs:domain cidoc_crm:E80_Part_Removal ;
    rdfs:range cidoc_crm:E24_Physical_Man-Made_Thing ;
    rdfs:subPropertyOf cidoc_crm:P31_has_modified .

cidoc_crm:P112i_was_diminished_by a owl:ObjectProperty ;
    rdfs:label "wurde vermindert durch"@de,
        "εξαλείφθηκε από"@el,
        "was diminished by"@en,
        "a été diminué par"@fr,
        "foi diminuído por"@pt,
        "был уменьшен посредством"@ru,
        "被缩减於"@zh ;
    rdfs:domain cidoc_crm:E24_Physical_Man-Made_Thing ;
    rdfs:range cidoc_crm:E80_Part_Removal ;
    rdfs:subPropertyOf cidoc_crm:P31i_was_modified_by .

cidoc_crm:P113_removed a owl:ObjectProperty ;
    rdfs:label "entfernte"@de,
        "αφαίρεσε"@el,
        "removed"@en,
        "a enlevé"@fr,
        "removeu"@pt,
        "удален"@ru,
        "移除了"@zh ;
    rdfs:comment "This property identifies the E18 Physical Thing that is removed during an E80 Part Removal activity."@en ;
    rdfs:domain cidoc_crm:E80_Part_Removal ;
    rdfs:range cidoc_crm:E18_Physical_Thing ;
    rdfs:subPropertyOf cidoc_crm:P12_occurred_in_the_presence_of .

cidoc_crm:P113i_was_removed_by a owl:ObjectProperty ;
    rdfs:label "wurde entfernt durch"@de,
        "αφαιρέθηκε από"@el,
        "was removed by"@en,
        "a été enlevée par"@fr,
        "foi removido por"@pt,
        "был удален посредством"@ru,
        "被移除於"@zh ;
    rdfs:domain cidoc_crm:E18_Physical_Thing ;
    rdfs:range cidoc_crm:E80_Part_Removal ;
    rdfs:subPropertyOf cidoc_crm:P12i_was_present_at .

cidoc_crm:P114_is_equal_in_time_to a owl:ObjectProperty ;
    rdfs:label "zeitgleich zu"@de,
        "συμπίπτει χρονικά με"@el,
        "is equal in time to"@en,
        "est temporellement égale à"@fr,
        "é temporalmente igual a"@pt,
        "равен по времени"@ru,
        "时段相同於"@zh ;
    rdfs:comment """This symmetric property allows the instances of E2 Temporal Entity with the same E52 Time-Span to be equated. \r
This property is only necessary if the time span is unknown (otherwise the equivalence can be calculated).\r
This property is the same as the "equal" relationship of Allen’s temporal logic (Allen, 1983, pp. 832-843).\r
"""@en ;
    rdfs:domain cidoc_crm:E2_Temporal_Entity ;
    rdfs:range cidoc_crm:E2_Temporal_Entity .

cidoc_crm:P115_finishes a owl:ObjectProperty ;
    rdfs:label "beendet"@de,
        "περατώνει"@el,
        "finishes"@en,
        "termine"@fr,
        "finaliza"@pt,
        "заканчивает"@ru,
        "结束了"@zh ;
    rdfs:comment """This property allows the ending point for a E2 Temporal Entity to be situated by reference to the ending point of another temporal entity of longer duration.  \r
This property is only necessary if the time span is unknown (otherwise the relationship can be calculated). This property is the same as the "finishes / finished-by" relationships of Allen’s temporal logic (Allen, 1983, pp. 832-843).\r
"""@en ;
    rdfs:domain cidoc_crm:E2_Temporal_Entity ;
    rdfs:range cidoc_crm:E2_Temporal_Entity .

cidoc_crm:P115i_is_finished_by a owl:ObjectProperty ;
    rdfs:label "wurde beendet mit"@de,
        "περατώνεται με"@el,
        "is finished by"@en,
        "est terminée par"@fr,
        "é finalizada por"@pt,
        "заканчивается"@ru,
        "被结束于"@zh ;
    rdfs:domain cidoc_crm:E2_Temporal_Entity ;
    rdfs:range cidoc_crm:E2_Temporal_Entity .

cidoc_crm:P116_starts a owl:ObjectProperty ;
    rdfs:label "beginnt"@de,
        "αρχίζει"@el,
        "starts"@en,
        "commence"@fr,
        "inicia"@pt,
        "начинает"@ru,
        "开始了"@zh ;
    rdfs:comment """This property allows the starting point for a E2 Temporal Entity to be situated by reference to the starting point of another temporal entity of longer duration.  \r
This property is only necessary if the time span is unknown (otherwise the relationship can be calculated). This property is the same as the "starts / started-by" relationships of Allen’s temporal logic (Allen, 1983, pp. 832-843).\r
"""@en ;
    rdfs:domain cidoc_crm:E2_Temporal_Entity ;
    rdfs:range cidoc_crm:E2_Temporal_Entity .

cidoc_crm:P116i_is_started_by a owl:ObjectProperty ;
    rdfs:label "wurde begonnen mit"@de,
        "αρχίζει με"@el,
        "is started by"@en,
        "est commencée par"@fr,
        "é iniciada por"@pt,
        "начинается"@ru,
        "被开始于"@zh ;
    rdfs:domain cidoc_crm:E2_Temporal_Entity ;
    rdfs:range cidoc_crm:E2_Temporal_Entity .

cidoc_crm:P117_occurs_during a owl:ObjectProperty ;
    rdfs:label "fällt in"@de,
        "εμφανίζεται κατά τη διάρκεια"@el,
        "occurs during"@en,
        "a lieu pendant"@fr,
        "ocorre durante"@pt,
        "появляется во течение"@ru,
        "时段被涵盖於"@zh ;
    rdfs:comment """This property allows the entire E52 Time-Span of an E2 Temporal Entity to be situated within the Time-Span of another temporal entity that starts before and ends after the included temporal entity.   \r
This property is only necessary if the time span is unknown (otherwise the relationship can be calculated). This property is the same as the "during / includes" relationships of Allen’s temporal logic (Allen, 1983, pp. 832-843).\r
"""@en ;
    rdfs:domain cidoc_crm:E2_Temporal_Entity ;
    rdfs:range cidoc_crm:E2_Temporal_Entity .

cidoc_crm:P117i_includes a owl:ObjectProperty ;
    rdfs:label "beinhaltet"@de,
        "περιλαμβάνει"@el,
        "includes"@en,
        "comporte"@fr,
        "inclui"@pt,
        "включает"@ru,
        "时段涵盖了"@zh ;
    rdfs:domain cidoc_crm:E2_Temporal_Entity ;
    rdfs:range cidoc_crm:E2_Temporal_Entity .

cidoc_crm:P118_overlaps_in_time_with a owl:ObjectProperty ;
    rdfs:label "überlappt zeitlich mit"@de,
        "προηγείται μερικώς επικαλύπτοντας"@el,
        "overlaps in time with"@en,
        "est partiellement recouverte dans le temps par"@fr,
        "sobrepõe temporalmente"@pt,
        "перекрывает во времени"@ru,
        "时段重叠了"@zh ;
    rdfs:comment """This property identifies an overlap between the instances of E52 Time-Span of two instances of E2 Temporal Entity. \r
It implies a temporal order between the two entities: if A overlaps in time B, then A must start before B, and B must end after A. This property is only necessary if the relevant time spans are unknown (otherwise the relationship can be calculated).\r
This property is the same as the "overlaps / overlapped-by" relationships of Allen’s temporal logic (Allen, 1983, pp. 832-843).\r
"""@en ;
    rdfs:domain cidoc_crm:E2_Temporal_Entity ;
    rdfs:range cidoc_crm:E2_Temporal_Entity .

cidoc_crm:P118i_is_overlapped_in_time_by a owl:ObjectProperty ;
    rdfs:label "wird zeitlich überlappt von"@de,
        "έπεται μερικώς επικαλυπτόμενο"@el,
        "is overlapped in time by"@en,
        "recouvre partiellement dans le temps"@fr,
        "é sobreposto temporalmente por"@pt,
        "перекрывается во времени"@ru,
        "时段被重叠于"@zh ;
    rdfs:domain cidoc_crm:E2_Temporal_Entity ;
    rdfs:range cidoc_crm:E2_Temporal_Entity .

cidoc_crm:P119_meets_in_time_with a owl:ObjectProperty ;
    rdfs:label "trifft zeitlich auf"@de,
        "προηγείται"@el,
        "meets in time with"@en,
        "est temporellement contiguë avec"@fr,
        "é temporalmente contíguo com"@pt,
        "следует во времени за"@ru,
        "紧接续了"@zh ;
    rdfs:comment """This property indicates that one E2 Temporal Entity immediately follows another. \r
It implies a particular order between the two entities: if A meets in time with B, then A must precede B. This property is only necessary if the relevant time spans are unknown (otherwise the relationship can be calculated). \r
This property is the same as the "meets / met-by" relationships of Allen’s temporal logic (Allen, 1983, pp. 832-843).\r
"""@en ;
    rdfs:domain cidoc_crm:E2_Temporal_Entity ;
    rdfs:range cidoc_crm:E2_Temporal_Entity .

cidoc_crm:P119i_is_met_in_time_by a owl:ObjectProperty ;
    rdfs:label "wird zeitlich getroffen von"@de,
        "έπεται"@el,
        "is met in time by"@en,
        "est immédiatement précédé par"@fr,
        "é imediatamente precedido por"@pt,
        "предшествует во времени"@ru,
        "紧接续於"@zh ;
    rdfs:domain cidoc_crm:E2_Temporal_Entity ;
    rdfs:range cidoc_crm:E2_Temporal_Entity .

cidoc_crm:P120_occurs_before a owl:ObjectProperty ;
    rdfs:label "kommt vor"@de,
        "εμφανίζεται πριν"@el,
        "occurs before"@en,
        "a lieu avant"@fr,
        "ocorre antes"@pt,
        "появляется до"@ru,
        "发生时段先於"@zh ;
    rdfs:comment """This property identifies the relative chronological sequence of two temporal entities. \r
It implies that a temporal gap exists between the end of A and the start of B. This property is only necessary if the relevant time spans are unknown (otherwise the relationship can be calculated).\r
This property is the same as the "before / after" relationships of Allen’s temporal logic (Allen, 1983, pp. 832-843).\r
"""@en ;
    rdfs:domain cidoc_crm:E2_Temporal_Entity ;
    rdfs:range cidoc_crm:E2_Temporal_Entity .

cidoc_crm:P120i_occurs_after a owl:ObjectProperty ;
    rdfs:label "kommt nach"@de,
        "εμφανίζεται μετά"@el,
        "occurs after"@en,
        "a lieu après"@fr,
        "ocorre depois"@pt,
        "появляется после"@ru,
        "发生时段后於"@zh ;
    rdfs:domain cidoc_crm:E2_Temporal_Entity ;
    rdfs:range cidoc_crm:E2_Temporal_Entity .

cidoc_crm:P121_overlaps_with a owl:ObjectProperty ;
    rdfs:label "überlappt mit"@de,
        "επικαλύπτεται με"@el,
        "overlaps with"@en,
        "chevauche"@fr,
        "sobrepõe com"@pt,
        "пересекается с"@ru,
        "空间重叠于"@zh ;
    rdfs:comment """This symmetric property allows the instances of E53 Place with overlapping geometric extents to be associated with each other. \r
It does not specify anything about the shared area. This property is purely spatial, in contrast to Allen operators, which are purely temporal.\r
"""@en ;
    rdfs:domain cidoc_crm:E53_Place ;
    rdfs:range cidoc_crm:E53_Place .

cidoc_crm:P122_borders_with a owl:ObjectProperty ;
    rdfs:label "grenzt an"@de,
        "συνορεύει με"@el,
        "borders with"@en,
        "jouxte"@fr,
        "fronteira com"@pt,
        "граничит с"@ru,
        "接壤于"@zh ;
    rdfs:comment """This symmetric property allows the instances of E53 Place which share common borders to be related as such. \r
This property is purely spatial, in contrast to Allen operators, which are purely temporal.\r
"""@en ;
    rdfs:domain cidoc_crm:E53_Place ;
    rdfs:range cidoc_crm:E53_Place .

cidoc_crm:P123_resulted_in a owl:ObjectProperty ;
    rdfs:label "ergab"@de,
        "είχε ως αποτέλεσμα"@el,
        "resulted in"@en,
        "a eu pour résultat"@fr,
        "resultou em"@pt,
        "повлек появление"@ru,
        "转变出"@zh ;
    rdfs:comment """This property identifies the E77 Persistent Item or items that are the result of an E81 Transformation. \r
New items replace the transformed item or items, which cease to exist as units of documentation. The physical continuity between the old and the new is expressed by the link to the common Transformation.\r
"""@en ;
    rdfs:domain cidoc_crm:E81_Transformation ;
    rdfs:range cidoc_crm:E77_Persistent_Item ;
    rdfs:subPropertyOf cidoc_crm:P92_brought_into_existence .

cidoc_crm:P123i_resulted_from a owl:ObjectProperty ;
    rdfs:label "ergab sich aus"@de,
        "προέκυψε από"@el,
        "resulted from"@en,
        "est le résultat de"@fr,
        "resultado de"@pt,
        "был результатом"@ru,
        "肇因於"@zh ;
    rdfs:domain cidoc_crm:E77_Persistent_Item ;
    rdfs:range cidoc_crm:E81_Transformation ;
    rdfs:subPropertyOf cidoc_crm:P92i_was_brought_into_existence_by .

cidoc_crm:P124_transformed a owl:ObjectProperty ;
    rdfs:label "wandelte um"@de,
        "μετέτρεψε"@el,
        "transformed"@en,
        "a transformé"@fr,
        "transformou"@pt,
        "трансформировал"@ru,
        "转变了"@zh ;
    rdfs:comment """This property identifies the E77 Persistent Item or items that cease to exist due to a E81 Transformation. \r
It is replaced by the result of the Transformation, which becomes a new unit of documentation. The continuity between both items, the new and the old, is expressed by the link to the common Transformation.\r
"""@en ;
    rdfs:domain cidoc_crm:E81_Transformation ;
    rdfs:range cidoc_crm:E77_Persistent_Item ;
    rdfs:subPropertyOf cidoc_crm:P93_took_out_of_existence .

cidoc_crm:P124i_was_transformed_by a owl:ObjectProperty ;
    rdfs:label "wurde umgewandelt durch"@de,
        "μετατράπηκε από"@el,
        "was transformed by"@en,
        "a été transformé par"@fr,
        "foi transformado por"@pt,
        "был трансформирован посредством"@ru,
        "被转变於"@zh ;
    rdfs:domain cidoc_crm:E77_Persistent_Item ;
    rdfs:range cidoc_crm:E81_Transformation ;
    rdfs:subPropertyOf cidoc_crm:P93i_was_taken_out_of_existence_by .

cidoc_crm:P126_employed a owl:ObjectProperty ;
    rdfs:label "verwendete"@de,
        "χρησιμοποίησε"@el,
        "employed"@en,
        "a employé"@fr,
        "empregou"@pt,
        "использовал"@ru,
        "采用了材料"@zh ;
    rdfs:comment """This property identifies E57 Material employed in an E11 Modification.\r
The E57 Material used during the E11 Modification does not necessarily become incorporated into the E24 Physical Man-Made Thing that forms the subject of the E11 Modification.\r
"""@en ;
    rdfs:domain cidoc_crm:E11_Modification ;
    rdfs:range cidoc_crm:E57_Material .

cidoc_crm:P126i_was_employed_in a owl:ObjectProperty ;
    rdfs:label "wurde verwendet bei"@de,
        "χρησιμοποιήθηκε σε"@el,
        "was employed in"@en,
        "a été employé dans"@fr,
        "foi empregado em"@pt,
        "использовался в"@ru,
        "被使用於"@zh ;
    rdfs:domain cidoc_crm:E57_Material ;
    rdfs:range cidoc_crm:E11_Modification .

cidoc_crm:P127_has_broader_term a owl:ObjectProperty ;
    rdfs:label "hat den Oberbegriff"@de,
        "έχει ευρύτερο όρο"@el,
        "has broader term"@en,
        "a pour terme générique"@fr,
        "tem termo genérico"@pt,
        "имеет вышестоящий термин"@ru,
        "有广义术语"@zh ;
    rdfs:comment """This property identifies a super-Type to which an E55 Type is related. \r
		It allows Types to be organised into hierarchies. This is the sense of "broader term generic  		(BTG)" as defined in ISO 2788\r
"""@en ;
    rdfs:domain cidoc_crm:E55_Type ;
    rdfs:range cidoc_crm:E55_Type .

cidoc_crm:P127i_has_narrower_term a owl:ObjectProperty ;
    rdfs:label "hat den Unterbegriff"@de,
        "έχει στενότερο όρο"@el,
        "has narrower term"@en,
        "a pour terme spécifique"@fr,
        "tem termo específico"@pt,
        "有狭义术语"@zh ;
    rdfs:domain cidoc_crm:E55_Type ;
    rdfs:range cidoc_crm:E55_Type .

cidoc_crm:P129_is_about a owl:ObjectProperty ;
    rdfs:label "handelt über"@de,
        "έχει ως θέμα"@el,
        "is about"@en,
        "est au sujet de"@fr,
        "é sobre"@pt,
        "касается"@ru,
        "陈述关於"@zh ;
    rdfs:comment """This property documents that an E89 Propositional Object has as subject an instance of E1 CRM Entity. \r
"""@en ;
    rdfs:domain cidoc_crm:E89_Propositional_Object ;
    rdfs:range cidoc_crm:E1_CRM_Entity ;
    rdfs:subPropertyOf cidoc_crm:P67_refers_to .

cidoc_crm:P129i_is_subject_of a owl:ObjectProperty ;
    rdfs:label "wird behandelt in"@de,
        "είναι θέμα  του/της"@el,
        "is subject of"@en,
        "est le sujet de"@fr,
        "é assunto de"@pt,
        "является предметом для"@ru,
        "被陈述於"@zh ;
    rdfs:domain cidoc_crm:E1_CRM_Entity ;
    rdfs:range cidoc_crm:E89_Propositional_Object ;
    rdfs:subPropertyOf cidoc_crm:P67i_is_referred_to_by .

cidoc_crm:P131_is_identified_by a owl:ObjectProperty ;
    rdfs:label "wird identifziert durch"@de,
        "αναγνωρίζεται ως"@el,
        "is identified by"@en,
        "est identifié par"@fr,
        "é identificado por"@pt,
        "идентифицируется посредством"@ru,
        "有称号"@zh ;
    rdfs:comment """This property identifies a name used specifically to identify an E39 Actor. \r
This property is a specialisation of P1 is identified by (identifies) is identified by.\r
"""@en ;
    rdfs:domain cidoc_crm:E39_Actor ;
    rdfs:range cidoc_crm:E82_Actor_Appellation ;
    rdfs:subPropertyOf cidoc_crm:P1_is_identified_by .

cidoc_crm:P131i_identifies a owl:ObjectProperty ;
    rdfs:label "identifiziert"@de,
        "είναι αναγνωριστικό"@el,
        "identifies"@en,
        "identifie"@fr,
        "identifica"@pt,
        "идентифицирует"@ru,
        "被用来识别"@zh ;
    rdfs:domain cidoc_crm:E82_Actor_Appellation ;
    rdfs:range cidoc_crm:E39_Actor ;
    rdfs:subPropertyOf cidoc_crm:P1i_identifies .

cidoc_crm:P132_overlaps_with a owl:ObjectProperty ;
    rdfs:label "überlappt mit"@de,
        "επικαλύπτεται με"@el,
        "overlaps with"@en,
        "chevauche"@fr,
        "sobrepõe"@pt,
        "пересекается с"@ru,
        "时空重叠于"@zh ;
    rdfs:comment """This symmetric property associates two instances of E92 Spacetime Volume that have some of their\r
extent in common.\r
"""@en ;
    rdfs:domain cidoc_crm:E92_Spacetime_Volume ;
    rdfs:range cidoc_crm:E92_Spacetime_Volume .

cidoc_crm:P133_is_separated_from a owl:ObjectProperty ;
    rdfs:label "getrennt von"@de,
        "διαχωρίζεται από"@el,
        "is separated from"@en,
        "est séparée de"@fr,
        "é separado de"@pt,
        "отделен от"@ru,
        "时空不重叠于"@zh ;
    rdfs:comment """This symmetric property associates two instances of E92 Spacetime Volume that have no extent in\r
common.\r
"""@en ;
    rdfs:domain cidoc_crm:E92_Spacetime_Volume ;
    rdfs:range cidoc_crm:E92_Spacetime_Volume .

cidoc_crm:P134_continued a owl:ObjectProperty ;
    rdfs:label "setzte sich fort in"@de,
        "συνέχισε"@el,
        "continued"@en,
        "est la suite de"@fr,
        "continuou"@pt,
        "продолжил"@ru,
        "延续了"@zh ;
    rdfs:comment """This property associates two instances of E7 Activity, where the domain is considered as an intentional continuation of the range. A continuation of an activity may happen when the continued activity is still ongoing or after the continued activity has completely ended. The continuing activity may have started already before it decided to continue the other one. Continuation implies a coherence of intentions and outcomes of the involved activities.\r
"""@en ;
    rdfs:domain cidoc_crm:E7_Activity ;
    rdfs:range cidoc_crm:E7_Activity ;
    rdfs:subPropertyOf cidoc_crm:P15_was_influenced_by .

cidoc_crm:P134i_was_continued_by a owl:ObjectProperty ;
    rdfs:label "wurde fortgesetzt durch"@de,
        "συνεχίστηκε από"@el,
        "was continued by"@en,
        "a été continuée par"@fr,
        "foi continuada por"@pt,
        "был продолжен"@ru,
        "有延续活动"@zh ;
    rdfs:domain cidoc_crm:E7_Activity ;
    rdfs:range cidoc_crm:E7_Activity ;
    rdfs:subPropertyOf cidoc_crm:P15i_influenced .

cidoc_crm:P135_created_type a owl:ObjectProperty ;
    rdfs:label "erschuf Typus"@de,
        "δημιούργησε τύπο"@el,
        "created type"@en,
        "a créé le type"@fr,
        "criou tipo"@pt,
        "создал тип"@ru,
        "创造了类型"@zh ;
    rdfs:comment "This property identifies the E55 Type, which is created in an E83Type Creation activity."@en ;
    rdfs:domain cidoc_crm:E83_Type_Creation ;
    rdfs:range cidoc_crm:E55_Type ;
    rdfs:subPropertyOf cidoc_crm:P94_has_created .

cidoc_crm:P135i_was_created_by a owl:ObjectProperty ;
    rdfs:label "wurde geschaffen durch"@de,
        "δημιουργήθηκε από"@el,
        "was created by"@en,
        "a été créé par"@fr,
        "foi criado por"@pt,
        "был создан посредством"@ru,
        "被创造於"@zh ;
    rdfs:domain cidoc_crm:E55_Type ;
    rdfs:range cidoc_crm:E83_Type_Creation ;
    rdfs:subPropertyOf cidoc_crm:P94i_was_created_by .

cidoc_crm:P136_was_based_on a owl:ObjectProperty ;
    rdfs:label "stützte sich auf"@de,
        "βασίστηκε σε"@el,
        "was based on"@en,
        "s’est fondée sur"@fr,
        "foi baseado em"@pt,
        "был основан на"@ru,
        "根据了"@zh ;
    rdfs:comment """This property identifies one or more items that were used as evidence to declare a new E55 Type.\r
The examination of these items is often the only objective way to understand the precise characteristics of a new Type. Such items should be deposited in a museum or similar institution for that reason. The taxonomic role renders the specific relationship of each item to the Type, such as "holotype" or "original element".\r
"""@en ;
    rdfs:domain cidoc_crm:E83_Type_Creation ;
    rdfs:range cidoc_crm:E1_CRM_Entity ;
    rdfs:subPropertyOf cidoc_crm:P15_was_influenced_by .

cidoc_crm:P136i_supported_type_creation a owl:ObjectProperty ;
    rdfs:label "belegte"@de,
        "υποστήριξε τη δημιουργία τύπου"@el,
        "supported type creation"@en,
        "a justifié la création de type"@fr,
        "suportou a criação de tipo"@pt,
        "поддержал создание типа"@ru,
        "提供證據给类型创造"@zh ;
    rdfs:domain cidoc_crm:E1_CRM_Entity ;
    rdfs:range cidoc_crm:E83_Type_Creation ;
    rdfs:subPropertyOf cidoc_crm:P15i_influenced .

cidoc_crm:P137_exemplifies a owl:ObjectProperty ;
    rdfs:label "erläutert"@de,
        "δειγματίζει"@el,
        "exemplifies"@en,
        "exemplifie"@fr,
        "é exemplificado por"@pt,
        "поясняет"@ru,
        "例示了"@zh ;
    rdfs:comment """This property allows an item to be declared as a particular example of an E55 Type or taxon\r
	The P137.1 in the taxonomic role property of P137 exemplifies (is exemplified by) allows differentiation of taxonomic roles. The taxonomic role renders the specific relationship of this example to the Type, such as "prototypical", "archetypical", "lectotype", etc. The taxonomic role "lectotype" is not associated with the Type Creation (E83) itself, but selected in a later phase.\r
"""@en ;
    rdfs:domain cidoc_crm:E1_CRM_Entity ;
    rdfs:range cidoc_crm:E55_Type ;
    rdfs:subPropertyOf cidoc_crm:P2_has_type .

cidoc_crm:P137i_is_exemplified_by a owl:ObjectProperty ;
    rdfs:label "erläutert durch Beispiel"@de,
        "δειγματίζεται από"@el,
        "is exemplified by"@en,
        "est exemplifié par"@fr,
        "exemplifica"@pt,
        "поясняется посредством"@ru,
        "有例示"@zh ;
    rdfs:domain cidoc_crm:E55_Type ;
    rdfs:range cidoc_crm:E1_CRM_Entity ;
    rdfs:subPropertyOf cidoc_crm:P2i_is_type_of .

cidoc_crm:P138_represents a owl:ObjectProperty ;
    rdfs:label "stellt dar"@de,
        "παριστάνει"@el,
        "represents"@en,
        "représente"@fr,
        "representa"@pt,
        "представляет"@ru,
        "描绘了"@zh ;
    rdfs:comment """This property establishes the relationship between an E36 Visual Item and the entity that it visually represents.\r
Any entity may be represented visually. This property is part of the fully developed path from E24 Physical Man-Made Thing through P65 shows visual item (is shown by), E36 Visual Item, P138 represents (has representation) to E1 CRM Entity, which is shortcut by P62depicts (is depicted by). P138.1 mode of representation allows the nature of the representation to be refined.\r
This property is also used for the relationship between an original and a digitisation of the original by the use of techniques such as digital photography, flatbed or infrared scanning. Digitisation is here seen as a process with a mechanical, causal component rendering the spatial distribution of structural and optical properties of the original and does not necessarily include any visual similarity identifiable by human observation.\r
"""@en ;
    rdfs:domain cidoc_crm:E36_Visual_Item ;
    rdfs:range cidoc_crm:E1_CRM_Entity ;
    rdfs:subPropertyOf cidoc_crm:P67_refers_to .

cidoc_crm:P138i_has_representation a owl:ObjectProperty ;
    rdfs:label "wird dargestellt durch"@de,
        "παριστάνεται από"@el,
        "has representation"@en,
        "est représentée par"@fr,
        "tem representação"@pt,
        "имеет представление"@ru,
        "有图像描绘"@zh ;
    rdfs:domain cidoc_crm:E1_CRM_Entity ;
    rdfs:range cidoc_crm:E36_Visual_Item ;
    rdfs:subPropertyOf cidoc_crm:P67i_is_referred_to_by .

cidoc_crm:P139_has_alternative_form a owl:ObjectProperty ;
    rdfs:label "hat alternative Form"@de,
        "έχει εναλλακτική μορφή"@el,
        "has alternative form"@en,
        "a pour autre forme"@fr,
        "tem forma alternativa"@pt,
        "имеет альтернативную форму"@ru,
        "有替代称号"@zh ;
    rdfs:comment """This property establishes a relationship of equivalence between two instances of E41 Appellation independent from any item identified by them. It is a dynamic asymmetric relationship, where the range expresses the derivative, if such a direction can be established. Otherwise, the relationship is symmetric. The relationship is not transitive.\r
The equivalence applies to all cases of use of an instance of E41 Appellation. Multiple names assigned to an object, which are not equivalent for all things identified with a specific instance of E41 Appellation, should be modelled as repeated values of P1 is identified by (identifies). \r
P139.1 has type allows the type of derivation, such as “transliteration from Latin 1 to ASCII” be refined..\r
"""@en ;
    rdfs:domain cidoc_crm:E41_Appellation ;
    rdfs:range cidoc_crm:E41_Appellation .

cidoc_crm:P13_destroyed a owl:ObjectProperty ;
    rdfs:label "zerstörte"@de,
        "κατέστρεψε"@el,
        "destroyed"@en,
        "a détruit"@fr,
        "destruiu"@pt,
        "уничтожил"@ru,
        "毁灭了"@zh ;
    rdfs:comment """This property allows specific instances of E18 Physical Thing that have been destroyed to be related to a destruction event. \r
Destruction implies the end of an item’s life as a subject of cultural documentation – the physical matter of which the item was composed may in fact continue to exist. A destruction event may be contiguous with a Production that brings into existence a derived object composed partly of matter from the destroyed object.\r
"""@en ;
    rdfs:domain cidoc_crm:E6_Destruction ;
    rdfs:range cidoc_crm:E18_Physical_Thing ;
    rdfs:subPropertyOf cidoc_crm:P93_took_out_of_existence .

cidoc_crm:P13i_was_destroyed_by a owl:ObjectProperty ;
    rdfs:label "wurde zerstört durch"@de,
        "καταστράφηκε από"@el,
        "was destroyed by"@en,
        "a été détruite par"@fr,
        "foi destruído por"@pt,
        "был уничтожен посредством"@ru,
        "被毁灭於"@zh ;
    rdfs:domain cidoc_crm:E18_Physical_Thing ;
    rdfs:range cidoc_crm:E6_Destruction ;
    rdfs:subPropertyOf cidoc_crm:P93i_was_taken_out_of_existence_by .

cidoc_crm:P142_used_constituent a owl:ObjectProperty ;
    rdfs:label "benutzte Bestandteil"@de,
        "used constituent"@en,
        "使用称号构成部分"@zh ;
    rdfs:comment """This property associates the event of assigning an instance of E42 Identifier to an entity, with  the instances of E41 Appellation that were used as elements of the identifier.\r
"""@en ;
    rdfs:domain cidoc_crm:E15_Identifier_Assignment ;
    rdfs:range cidoc_crm:E90_Symbolic_Object ;
    rdfs:subPropertyOf cidoc_crm:P16_used_specific_object .

cidoc_crm:P142i_was_used_in a owl:ObjectProperty ;
    rdfs:label "wurde benutzt in"@de,
        "was used in"@en,
        "被用来构成称号於"@zh ;
    rdfs:domain cidoc_crm:E90_Symbolic_Object ;
    rdfs:range cidoc_crm:E15_Identifier_Assignment ;
    rdfs:subPropertyOf cidoc_crm:P16i_was_used_for .

cidoc_crm:P143_joined a owl:ObjectProperty ;
    rdfs:label "verband"@de,
        "joined"@en,
        "加入了成员"@zh ;
    rdfs:comment """This property identifies the instance of E39 Actor that becomes member of a E74 Group in an E85 Joining.\r
 	Joining events allow for describing people becoming members of a group with a more detailed path from E74 Group through P144 joined with (gained member by), E85 Joining, P143 joined (was joined by) to E39 Actor, compared to the shortcut offered by P107 has current or former member (is current or former member of).\r
"""@en ;
    rdfs:domain cidoc_crm:E85_Joining ;
    rdfs:range cidoc_crm:E39_Actor ;
    rdfs:subPropertyOf cidoc_crm:P11_had_participant .

cidoc_crm:P143i_was_joined_by a owl:ObjectProperty ;
    rdfs:label "wurde verbunden durch"@de,
        "was joined by"@en,
        "被加入为成员於"@zh ;
    rdfs:domain cidoc_crm:E39_Actor ;
    rdfs:range cidoc_crm:E85_Joining ;
    rdfs:subPropertyOf cidoc_crm:P11i_participated_in .

cidoc_crm:P144_joined_with a owl:ObjectProperty ;
    rdfs:label "verband mit"@de,
        "joined with"@en,
        "加入成员到"@zh ;
    rdfs:comment """This property identifies the instance of E74 Group of which an instance of E39 Actor becomes a member through an instance of E85 Joining.\r
Although a Joining activity normally concerns only one instance of E74 Group, it is possible to imagine circumstances under which becoming member of one Group implies becoming member of another Group as well. \r
Joining events allow for describing people becoming members of a group with a more detailed path from E74 Group through P144 joined with (gained member by), E85 Joining, P143 joined (was joined by) to E39 Actor, compared to the shortcut offered by P107 has current or former member (is current or former member of).\r
The property P144.1 kind of member can be used to specify the type of membership or the role the member has in the group. \r
"""@en ;
    rdfs:domain cidoc_crm:E85_Joining ;
    rdfs:range cidoc_crm:E74_Group ;
    rdfs:subPropertyOf cidoc_crm:P11_had_participant .

cidoc_crm:P144i_gained_member_by a owl:ObjectProperty ;
    rdfs:label "erwarb Mitglied durch"@de,
        "gained member by"@en,
        "获得成员於"@zh ;
    rdfs:domain cidoc_crm:E74_Group ;
    rdfs:range cidoc_crm:E85_Joining ;
    rdfs:subPropertyOf cidoc_crm:P11i_participated_in .

cidoc_crm:P145_separated a owl:ObjectProperty ;
    rdfs:label "entließ"@de,
        "separated"@en,
        "分离了成员"@zh ;
    rdfs:comment "This property identifies the instance of E39 Actor that leaves an instance of E74 Group through an instance of E86 Leaving."@en ;
    rdfs:domain cidoc_crm:E86_Leaving ;
    rdfs:range cidoc_crm:E39_Actor ;
    rdfs:subPropertyOf cidoc_crm:P11_had_participant .

cidoc_crm:P145i_left_by a owl:ObjectProperty ;
    rdfs:label "wurde entlassen durch"@de,
        "left by"@en,
        "脱离群组於"@zh ;
    rdfs:domain cidoc_crm:E39_Actor ;
    rdfs:range cidoc_crm:E86_Leaving ;
    rdfs:subPropertyOf cidoc_crm:P11i_participated_in .

cidoc_crm:P146_separated_from a owl:ObjectProperty ;
    rdfs:label "entließ von"@de,
        "separated from"@en,
        "脱离了群组"@zh ;
    rdfs:comment """This property identifies the instance of E74 Group an instance of E39 Actor leaves through an instance of E86 Leaving.\r
Although a Leaving activity normally concerns only one instance of E74 Group, it is possible to imagine circumstances under which leaving one E74 Group implies leaving another E74 Group as well.\r
"""@en ;
    rdfs:domain cidoc_crm:E86_Leaving ;
    rdfs:range cidoc_crm:E74_Group ;
    rdfs:subPropertyOf cidoc_crm:P11_had_participant .

cidoc_crm:P146i_lost_member_by a owl:ObjectProperty ;
    rdfs:label "verlor Mitglied durch"@de,
        "lost member by"@en,
        "失去成员於"@zh ;
    rdfs:domain cidoc_crm:E74_Group ;
    rdfs:range cidoc_crm:E86_Leaving ;
    rdfs:subPropertyOf cidoc_crm:P11i_participated_in .

cidoc_crm:P147_curated a owl:ObjectProperty ;
    rdfs:label "betreute kuratorisch"@de,
        "curated"@en,
        "典藏管理了"@zh ;
    rdfs:comment """This property associates an instance of E87 Curation Activity with the instance of E78 Collection that is subject of that  curation activity.\r
"""@en ;
    rdfs:domain cidoc_crm:E87_Curation_Activity ;
    rdfs:range cidoc_crm:E78_Collection .

cidoc_crm:P147i_was_curated_by a owl:ObjectProperty ;
    rdfs:label "wurde kuratorisch betreut durch"@de,
        "was curated by"@en,
        "被典藏管理於"@zh ;
    rdfs:domain cidoc_crm:E78_Collection ;
    rdfs:range cidoc_crm:E87_Curation_Activity .

cidoc_crm:P148_has_component a owl:ObjectProperty ;
    rdfs:label "hat Bestandteil"@de,
        "has component"@en,
        "有组件"@zh ;
    rdfs:comment "This property associates an instance of E89 Propositional Object with a structural part of it that is by itself an instance of E89 Propositional Object."@en ;
    rdfs:domain cidoc_crm:E89_Propositional_Object ;
    rdfs:range cidoc_crm:E89_Propositional_Object .

cidoc_crm:P148i_is_component_of a owl:ObjectProperty ;
    rdfs:label "ist Bestandteil von"@de,
        "is component of"@en,
        "被用来组成"@zh ;
    rdfs:domain cidoc_crm:E89_Propositional_Object ;
    rdfs:range cidoc_crm:E89_Propositional_Object .

cidoc_crm:P149_is_identified_by a owl:ObjectProperty ;
    rdfs:label "is identified by"@en ;
    rdfs:comment "This property identifies an instance of E28 Conceptual Object using an instance of E75 Conceptual Object Appellation."@en ;
    rdfs:domain cidoc_crm:E28_Conceptual_Object ;
    rdfs:range cidoc_crm:E75_Conceptual_Object_Appellation ;
    rdfs:subPropertyOf cidoc_crm:P1_is_identified_by .

cidoc_crm:P149i_identifies a owl:ObjectProperty ;
    rdfs:label "identifies"@en ;
    rdfs:domain cidoc_crm:E75_Conceptual_Object_Appellation ;
    rdfs:range cidoc_crm:E28_Conceptual_Object ;
    rdfs:subPropertyOf cidoc_crm:P1i_identifies .

cidoc_crm:P150_defines_typical_parts_of a owl:ObjectProperty ;
    rdfs:label "defines typical parts of"@en ;
    rdfs:comment """This property associates an instance of E55 Type “A” with an instance of E55 Type “B”, when items\r
of type “A” typically form part of items of type “B”, such as “car motors” and “cars”.\r
It allows types to be organised into hierarchies based on one type describing a typical part of another.\r
This property is equivalent to "broader term partitive (BTP)" as defined in ISO 2788 and\r
“broaderPartitive” in SKOS.\r
"""@en ;
    rdfs:domain cidoc_crm:E55_Type ;
    rdfs:range cidoc_crm:E55_Type .

cidoc_crm:P150i_defines_typical_wholes_for a owl:ObjectProperty ;
    rdfs:label "defines typical wholes for"@en ;
    rdfs:domain cidoc_crm:E55_Type ;
    rdfs:range cidoc_crm:E55_Type .

cidoc_crm:P151_was_formed_from a owl:ObjectProperty ;
    rdfs:label "was formed from"@en ;
    rdfs:comment """This property associates an instance of E66 Formation with an instance of E74 Group from which the new group was formed preserving a sense of continuity such as in mission, membership or tradition.\r
	"""@en ;
    rdfs:domain cidoc_crm:E66_Formation ;
    rdfs:range cidoc_crm:E74_Group ;
    rdfs:subPropertyOf cidoc_crm:P11_had_participant .

cidoc_crm:P151i_participated_in a owl:ObjectProperty ;
    rdfs:label "participated in"@en ;
    rdfs:domain cidoc_crm:E74_Group ;
    rdfs:range cidoc_crm:E66_Formation ;
    rdfs:subPropertyOf cidoc_crm:P11i_participated_in .

cidoc_crm:P152_has_parent a owl:ObjectProperty ;
    rdfs:label "has parent"@en ;
    rdfs:comment """This property associates an instance of E21 Person with another instance of E21 Person who plays the role of the first instance’s parent, regardless of whether the relationship is biological parenthood, assumed or pretended biological parenthood or an equivalent legal status of rights and obligations obtained by a social or legal act. \r
	This property is, among others, a shortcut of the fully developed paths from ‘E21Person’ through ‘P98i was born’, ‘E67 Birth’, ‘P96 by mother’ to ‘E21 Person’, and from ‘E21Person’ through ‘P98i was born’, ‘E67 Birth’, ‘P97 from father’ to ‘E21 Person’.\r
	"""@en ;
    rdfs:domain cidoc_crm:E21_Person ;
    rdfs:range cidoc_crm:E21_Person .

cidoc_crm:P152i_is_parent_of a owl:ObjectProperty ;
    rdfs:label "is parent of"@en ;
    rdfs:domain cidoc_crm:E21_Person ;
    rdfs:range cidoc_crm:E21_Person .

cidoc_crm:P156_occupies a owl:ObjectProperty ;
    rdfs:label "occupies"@en ;
    rdfs:comment """This property describes the largest volume in space that an instance of E18 Physical Thing has occupied at any time during its existence, with respect to the reference space relative to itself. This allows you to describe the thing itself as a place that may contain other things, such as a box that may contain coins. In other words, it is the volume that contains all the points which the thing has covered at some time during its existence. In the case of an E26 Physical Feature the default reference space is the one in which the object that bears the feature or at least the surrounding matter of the feature is at rest. In this case there is a 1:1 relation of E26 Feature and E53 Place. For simplicity of implementation multiple inheritance (E26 Feature IsA E53 Place) may be a practical approach.\r
\r
For instances of E19 Physical Objects the default reference space is the one which is at rest to the object itself, i.e. which moves together with the object. We include in the occupied space the space filled by the matter of the physical thing and all its inner spaces. \r
\r
This property is a subproperty of P161 has spatial projection because it refers to its own domain as reference space for its range, whereas P161 has spatial projection may refer to a place in terms of any reference space. For some instances of E18 Physical Object the relative stability of form may not be sufficient to define a useful local reference space, for instance for an amoeba. In such cases the fully developed path to an external reference space and using a temporal validity component may be adequate to determine the place they have occupied.\r
\r
In contrast to P156  occupies, the property P53 has former or current location identifies an instance of E53 Place at which a thing is or has been for some unspecified time span.  Further it does not constrain the reference space of the referred instance of P53 Place.\r
	"""@en ;
    rdfs:domain cidoc_crm:E18_Physical_Thing ;
    rdfs:range cidoc_crm:E53_Place ;
    rdfs:subPropertyOf cidoc_crm:P161_has_spatial_projection .

cidoc_crm:P156i_is_occupied_by a owl:ObjectProperty ;
    rdfs:label "is occupied by"@en ;
    rdfs:domain cidoc_crm:E53_Place ;
    rdfs:range cidoc_crm:E18_Physical_Thing ;
    rdfs:subPropertyOf cidoc_crm:P161i_is_spatial_projection_of .

cidoc_crm:P157_is_at_rest_relative_to a owl:ObjectProperty ;
    rdfs:label "is at rest relative to"@en ;
    rdfs:comment """This property associates an instance of P53 Place with the instance of E18 Physical Thing that determines a reference space for this instance of P53 Place by being at rest with respect to this reference space. The relative stability of form of an E18 Physical Thing defines its default reference space. The reference space is not spatially limited to the referred thing. For example, a ship determines a reference space in terms of which other ships in its neighbourhood may be described. Larger constellations of matter, such as continental plates, may comprise many physical features that are at rest with them and define the same reference space.\r
	"""@en ;
    rdfs:domain cidoc_crm:E53_Place ;
    rdfs:range cidoc_crm:E18_Physical_Thing ;
    rdfs:subPropertyOf cidoc_crm:P59i_is_located_on_or_within .

cidoc_crm:P157i_provides_reference_space_for a owl:ObjectProperty ;
    rdfs:label "provides reference space for"@en ;
    rdfs:domain cidoc_crm:E18_Physical_Thing ;
    rdfs:range cidoc_crm:E53_Place ;
    rdfs:subPropertyOf cidoc_crm:P59_has_section .

cidoc_crm:P164_during a owl:ObjectProperty ;
    rdfs:label "during"@en ;
    rdfs:comment """This property relates an instance of E93 Presence with an arbitrary instance of E52 Time-Span that\r
defines the section of the spacetime volume that this instance of E93 Presence is related to by the property P166 was a presence of (had presence).\r
	"""@en ;
    rdfs:domain cidoc_crm:E93_Presence ;
    rdfs:range cidoc_crm:E52_Time-Span ;
    rdfs:subPropertyOf cidoc_crm:P160_has_temporal_projection .

cidoc_crm:P164i_was_time-span_of a owl:ObjectProperty ;
    rdfs:label "was time-span of"@en ;
    rdfs:domain cidoc_crm:E52_Time-Span ;
    rdfs:range cidoc_crm:E93_Presence ;
    rdfs:subPropertyOf cidoc_crm:P160i_is_temporal_projection_of .

cidoc_crm:P165_incorporates a owl:ObjectProperty ;
    rdfs:label "incorporates"@en ;
    rdfs:comment """This property associates an instance of E73 Information Object with an instance of E90 Symbolic Object (or any of its subclasses) that was included in it.\r
This property makes it possible to recognise the autonomous status of the incorporated signs, which were created in a distinct context, and can be incorporated in many distinct self-contained expressions, and to highlight the difference between structural and accidental whole-part relationships between conceptual entities.\r
It accounts for many cultural facts that are quite frequent and significant: the inclusion of a poem in an anthology, the re-use of an operatic aria in a new opera, the use of a reproduction of a painting for a book cover or a CD booklet, the integration of textual quotations, the presence of lyrics in a song that sets those lyrics to music, the presence of the text of a play in a movie based on that play, etc.\r
In particular, this property allows for modelling relationships of different levels of symbolic specificity, such as the natural language words making up a particular text, the characters making up the words and punctuation, the choice of fonts and page layout for the characters.\r
A digital photograph of a manuscript page incorporates the text of the manuscript page.\r
	"""@en ;
    rdfs:domain cidoc_crm:E73_Information_Object ;
    rdfs:range cidoc_crm:E90_Symbolic_Object ;
    rdfs:subPropertyOf cidoc_crm:P106_is_composed_of .

cidoc_crm:P165i_is_incorporated_in a owl:ObjectProperty ;
    rdfs:label "is incorporated in"@en ;
    rdfs:domain cidoc_crm:E90_Symbolic_Object ;
    rdfs:range cidoc_crm:E73_Information_Object ;
    rdfs:subPropertyOf cidoc_crm:P106i_forms_part_of .

cidoc_crm:P166_was_a_presence_of a owl:ObjectProperty ;
    rdfs:label "was a presence of"@en ;
    rdfs:comment """This property relates an E93 Presence with the STV it is part of… \r
	"""@en ;
    rdfs:domain cidoc_crm:E93_Presence ;
    rdfs:range cidoc_crm:E92_Spacetime_Volume .

cidoc_crm:P166i_had_presence a owl:ObjectProperty ;
    rdfs:label "had presence"@en ;
    rdfs:domain cidoc_crm:E92_Spacetime_Volume ;
    rdfs:range cidoc_crm:E93_Presence .

cidoc_crm:P167_at a owl:ObjectProperty ;
    rdfs:label "at"@en ;
    rdfs:comment """This property points to a wider area in which my thing /event was… \r
	"""@en ;
    rdfs:domain cidoc_crm:E93_Presence ;
    rdfs:range cidoc_crm:E53_Place .

cidoc_crm:P167i_was_place_of a owl:ObjectProperty ;
    rdfs:label "was place of"@en ;
    rdfs:domain cidoc_crm:E53_Place ;
    rdfs:range cidoc_crm:E93_Presence .

cidoc_crm:P168_place_is_defined_by a owl:DatatypeProperty ;
    rdfs:label "place is defined by "@en ;
    rdfs:comment """This property associates an instance of E53 Place with an instance of E94 Space Primitive that defines it. Syntactic variants or use of different scripts may result in multiple instances of E94 Space Primitive defining exactly the same place. Transformations between different reference systems in general result in new definitions of places approximating each other and not in alternative definitions. Note that it is possible for a place to be defined by phenomena causal to it or other forms of identification rather than by an instance of E94 Space Primitive. In this case, this property must not be used for approximating the respective instance of E53 Place with an instance of E94 Space Primitive. \r
	"""@en ;
    rdfs:domain cidoc_crm:E53_Place ;
    rdfs:range rdfs:Literal .

cidoc_crm:P17_was_motivated_by a owl:ObjectProperty ;
    rdfs:label "wurde angeregt durch"@de,
        "είχε ως αφορμή"@el,
        "was motivated by"@en,
        "a été motivée par"@fr,
        "foi motivado por"@pt,
        "был обусловлен посредством"@ru,
        "有促动事物"@zh ;
    rdfs:comment """This property describes an item or items that are regarded as a reason for carrying out the E7 Activity. \r
For example, the discovery of a large hoard of treasure may call for a celebration, an order from head quarters can start a military manoeuvre. \r
"""@en ;
    rdfs:domain cidoc_crm:E7_Activity ;
    rdfs:range cidoc_crm:E1_CRM_Entity ;
    rdfs:subPropertyOf cidoc_crm:P15_was_influenced_by .

cidoc_crm:P17i_motivated a owl:ObjectProperty ;
    rdfs:label "regte an"@de,
        "ήταν αφορμή"@el,
        "motivated"@en,
        "a motivé"@fr,
        "motivou"@pt,
        "обусловил"@ru,
        "促动了"@zh ;
    rdfs:domain cidoc_crm:E1_CRM_Entity ;
    rdfs:range cidoc_crm:E7_Activity ;
    rdfs:subPropertyOf cidoc_crm:P15i_influenced .

cidoc_crm:P19_was_intended_use_of a owl:ObjectProperty ;
    rdfs:label "war beabsichtigteter Gebrauch von "@de,
        "ήταν προορισμένη χρήση του"@el,
        "was intended use of"@en,
        "était l'utilisation prévue de"@fr,
        "era prevista a utilização de"@pt,
        "был предполагаемым использованием для"@ru,
        "特别使用了"@zh ;
    rdfs:comment """This property relates an E7 Activity with objects created specifically for use in the activity. \r
This is distinct from the intended use of an item in some general type of activity such as the book of common prayer which was intended for use in Church of England services (see P101 had as general use (was use of))."""@en ;
    rdfs:domain cidoc_crm:E7_Activity ;
    rdfs:range cidoc_crm:E71_Man-Made_Thing .

cidoc_crm:P19i_was_made_for a owl:ObjectProperty ;
    rdfs:label "wurde hergestellt für"@de,
        "έγινε για"@el,
        "was made for"@en,
        "a été fabriquée pour"@fr,
        "foi feito para"@pt,
        "был создан для"@ru,
        "被制造来用於"@zh ;
    rdfs:domain cidoc_crm:E71_Man-Made_Thing ;
    rdfs:range cidoc_crm:E7_Activity .

cidoc_crm:P20_had_specific_purpose a owl:ObjectProperty ;
    rdfs:label "hatte den bestimmten Zweck"@de,
        "είχε συγκεκριμένο σκοπό"@el,
        "had specific purpose"@en,
        "avait pour but spécifique"@fr,
        "tinha propósito específico"@pt,
        "имел конкретную цель"@ru,
        "有特定目地"@zh ;
    rdfs:comment """This property identifies the relationship between a preparatory activity and the event it is intended to be preparation for.\r
This includes activities, orders and other organisational actions, taken in preparation for other activities or events. \r
P20 had specific purpose (was purpose of) implies that an activity succeeded in achieving its aim. If it does not succeed, such as the setting of a trap that did not catch anything, one may document the unrealized intention using P21 had general purpose (was purpose of):E55 Type and/or  P33 used specific technique (was used by): E29 Design or Procedure."""@en ;
    rdfs:domain cidoc_crm:E7_Activity ;
    rdfs:range cidoc_crm:E5_Event .

cidoc_crm:P20i_was_purpose_of a owl:ObjectProperty ;
    rdfs:label "war Zweck von"@de,
        "ήταν σκοπός του/της"@el,
        "was purpose of"@en,
        "était le but de"@fr,
        "era o propósito de"@pt,
        "был целью для"@ru,
        "之準備活動是"@zh ;
    rdfs:domain cidoc_crm:E5_Event ;
    rdfs:range cidoc_crm:E7_Activity .

cidoc_crm:P21_had_general_purpose a owl:ObjectProperty ;
    rdfs:label "hatte den allgemeinen Zweck"@de,
        "είχε γενικό σκοπό"@el,
        "had general purpose"@en,
        "avait pour but général"@fr,
        "tinha propósito geral"@pt,
        "имел общую цель"@ru,
        "有通用目地"@zh ;
    rdfs:comment """This property describes an intentional relationship between an E7 Activity and some general goal or purpose. \r
This may involve activities intended as preparation for some type of activity or event. P21had general purpose (was purpose of) differs from P20 had specific purpose (was purpose of) in that no occurrence of an event is implied as the purpose. \r
"""@en ;
    rdfs:domain cidoc_crm:E7_Activity ;
    rdfs:range cidoc_crm:E55_Type .

cidoc_crm:P21i_was_purpose_of a owl:ObjectProperty ;
    rdfs:label "war Zweck von"@de,
        "ήταν σκοπός του/της"@el,
        "was purpose of"@en,
        "était le but de"@fr,
        "era o propósito de"@pt,
        "был целью для"@ru,
        "可利用"@zh ;
    rdfs:domain cidoc_crm:E55_Type ;
    rdfs:range cidoc_crm:E7_Activity .

cidoc_crm:P22_transferred_title_to a owl:ObjectProperty ;
    rdfs:label "übertrug Besitztitel auf"@de,
        "μετεβίβασε τον τίτλο σε"@el,
        "transferred title to"@en,
        "a fait passer le droit de propriété à"@fr,
        "transferiu os direitos de propriedade para"@pt,
        "передал право собственности"@ru,
        "转交所有权给"@zh ;
    rdfs:comment """This property identifies the E39 Actor that acquires the legal ownership of an object as a result of an E8 Acquisition. \r
The property will typically describe an Actor purchasing or otherwise acquiring an object from another Actor. However, title may also be acquired, without any corresponding loss of title by another Actor, through legal fieldwork such as hunting, shooting or fishing.\r
In reality the title is either transferred to or from someone, or both.\r
"""@en ;
    rdfs:domain cidoc_crm:E8_Acquisition ;
    rdfs:range cidoc_crm:E39_Actor ;
    rdfs:subPropertyOf cidoc_crm:P14_carried_out_by .

cidoc_crm:P22i_acquired_title_through a owl:ObjectProperty ;
    rdfs:label "erwarb Besitztitel durch"@de,
        "απέκτησε τον τίτλο μέσω"@el,
        "acquired title through"@en,
        "a acquis le droit de propriété du fait de"@fr,
        "adquiriu os direitos de propriedade por meio da"@pt,
        "получил право собственности через"@ru,
        "获取所有权於"@zh ;
    rdfs:domain cidoc_crm:E39_Actor ;
    rdfs:range cidoc_crm:E8_Acquisition ;
    rdfs:subPropertyOf cidoc_crm:P14i_performed .

cidoc_crm:P23_transferred_title_from a owl:ObjectProperty ;
    rdfs:label "übertrug Besitztitel von"@de,
        "μετεβίβασε τον τίτλο από"@el,
        "transferred title from"@en,
        "a fait passer le droit de propriété de"@fr,
        "transferiu os direitos de propriedade de"@pt,
        "передал право собственности от"@ru,
        "原所有权者是"@zh ;
    rdfs:comment """This property identifies the E39 Actor or Actors who relinquish legal ownership as the result of an E8 Acquisition.\r
The property will typically be used to describe a person donating or selling an object to a museum. In reality title is either transferred to or from someone, or both.\r
"""@en ;
    rdfs:domain cidoc_crm:E8_Acquisition ;
    rdfs:range cidoc_crm:E39_Actor ;
    rdfs:subPropertyOf cidoc_crm:P14_carried_out_by .

cidoc_crm:P23i_surrendered_title_through a owl:ObjectProperty ;
    rdfs:label "trat Besitztitel ab in"@de,
        "παρέδωσε τον τίτλο μέσω"@el,
        "surrendered title through"@en,
        "a perdu le droit de propriété du fait de"@fr,
        "perdeu os direitos de propriedade por meio da"@pt,
        "право собственности отдано через"@ru,
        "交出所有权於"@zh ;
    rdfs:domain cidoc_crm:E39_Actor ;
    rdfs:range cidoc_crm:E8_Acquisition ;
    rdfs:subPropertyOf cidoc_crm:P14i_performed .

cidoc_crm:P24_transferred_title_of a owl:ObjectProperty ;
    rdfs:label "übertrug Besitz über"@de,
        "μετεβίβασε τον τίτλο του/της"@el,
        "transferred title of"@en,
        "a fait passer le droit de propriété sur"@fr,
        "transferiu os direitos de propriedade sobre o"@pt,
        "передал право собственности на"@ru,
        "转移所有权的标的物是"@zh ;
    rdfs:comment """This property identifies the E18 Physical Thing or things involved in an E8 Acquisition. \r
In reality, an acquisition must refer to at least one transferred item.\r
"""@en ;
    rdfs:domain cidoc_crm:E8_Acquisition ;
    rdfs:range cidoc_crm:E18_Physical_Thing .

cidoc_crm:P24i_changed_ownership_through a owl:ObjectProperty ;
    rdfs:label "ging über in Besitz durch"@de,
        "άλλαξε ιδιοκτησία μέσω"@el,
        "changed ownership through"@en,
        "a changé de mains du fait de"@fr,
        "mudou de proprietário por meio de"@pt,
        "сменил владельца через"@ru,
        "转移了所有权於"@zh ;
    rdfs:domain cidoc_crm:E18_Physical_Thing ;
    rdfs:range cidoc_crm:E8_Acquisition .

cidoc_crm:P25_moved a owl:ObjectProperty ;
    rdfs:label "bewegte"@de,
        "μετεκίνησε"@el,
        "moved"@en,
        "a déplacé"@fr,
        "locomoveu"@pt,
        "переместил"@ru,
        "移动了"@zh ;
    rdfs:comment """This property identifies an instance of E19 Physical Object that was moved by a move event. A move must concern at least one object.\r
\r
The property implies the object's passive participation. For example, Monet's painting "Impression sunrise" was moved for the first Impressionist exhibition in 1874. \r
"""@en ;
    rdfs:domain cidoc_crm:E9_Move ;
    rdfs:range cidoc_crm:E19_Physical_Object ;
    rdfs:subPropertyOf cidoc_crm:P12_occurred_in_the_presence_of .

cidoc_crm:P25i_moved_by a owl:ObjectProperty ;
    rdfs:label "wurde bewegt durch"@de,
        "μετακινήθηκε από"@el,
        "moved by"@en,
        "a été déplacé par"@fr,
        "foi locomovido por"@pt,
        "перемещен посредством"@ru,
        "被移动於"@zh ;
    rdfs:domain cidoc_crm:E19_Physical_Object ;
    rdfs:range cidoc_crm:E9_Move ;
    rdfs:subPropertyOf cidoc_crm:P12i_was_present_at .

cidoc_crm:P26_moved_to a owl:ObjectProperty ;
    rdfs:label "bewegte bis zu"@de,
        "μετακινήθηκε προς"@el,
        "moved to"@en,
        "a déplacé vers"@fr,
        "locomoveu para"@pt,
        "перемещен в"@ru,
        "移入物件至"@zh ;
    rdfs:comment """This property identifies a destination of a E9 Move. \r
A move will be linked to a destination, such as the move of an artefact from storage to display. A move may be linked to many terminal instances of E53 Place by multiple instances of this property. In this case the move describes a distribution of a set of objects. The area of the move includes the origin(s), route and destination(s).\r
Therefore the described destination is an instance of E53 Place which P89 falls within (contains) the instance of E53 Place the move P7 took place at.\r
"""@en ;
    rdfs:domain cidoc_crm:E9_Move ;
    rdfs:range cidoc_crm:E53_Place .

cidoc_crm:P26i_was_destination_of a owl:ObjectProperty ;
    rdfs:label "war Zielort von"@de,
        "ήταν προορισμός του/της"@el,
        "was destination of"@en,
        "a été la destination de"@fr,
        "era destinação de"@pt,
        "был пунктом назначения для"@ru,
        "被作为移入地於"@zh ;
    rdfs:domain cidoc_crm:E53_Place ;
    rdfs:range cidoc_crm:E9_Move ;
    rdfs:subPropertyOf cidoc_crm:P7i_witnessed .

cidoc_crm:P27_moved_from a owl:ObjectProperty ;
    rdfs:label "bewegte weg von"@de,
        "μετακινήθηκε από"@el,
        "moved from"@en,
        "a retiré de"@fr,
        "locomoveu de"@pt,
        "перемещен из"@ru,
        "有移出地"@zh ;
    rdfs:comment """This property identifies a starting E53 Place of an E9 Move.\r
\r
A move will be linked to an origin, such as the move of an artefact from storage to display. A move may be linked to many starting instances of E53 Place by multiple instances of this property. In this case the move describes the picking up of a set of objects. The area of the move includes the origin(s), route and destination(s).\r
Therefore the described origin is an instance of E53 Place which P89 falls within (contains) the instance of E53 Place the move P7 took place at.\r
"""@en ;
    rdfs:domain cidoc_crm:E9_Move ;
    rdfs:range cidoc_crm:E53_Place .

cidoc_crm:P27i_was_origin_of a owl:ObjectProperty ;
    rdfs:label "war Ausgangsort von"@de,
        "ήταν αφετηρία του/της"@el,
        "was origin of"@en,
        "a été l'origine de"@fr,
        "era origem de"@pt,
        "был исходной точкой для"@ru,
        "被作为移出地於"@zh ;
    rdfs:domain cidoc_crm:E53_Place ;
    rdfs:range cidoc_crm:E9_Move ;
    rdfs:subPropertyOf cidoc_crm:P7i_witnessed .

cidoc_crm:P28_custody_surrendered_by a owl:ObjectProperty ;
    rdfs:label "übergab Gewahrsam an"@de,
        "μετεβίβασε κατοχή από"@el,
        "custody surrendered by"@en,
        "changement de détenteur au détriment de"@fr,
        "custódia concedida por"@pt,
        "опека отдана"@ru,
        "有原保管人"@zh ;
    rdfs:comment """This property identifies the E39 Actor or Actors who surrender custody of an instance of E18 Physical Thing in an E10 Transfer of Custody activity. \r
The property will typically describe an Actor surrendering custody of an object when it is handed over to someone else’s care. On occasion, physical custody may be surrendered involuntarily – through accident, loss or theft.\r
In reality, custody is either transferred to someone or from someone, or both.\r
"""@en ;
    rdfs:domain cidoc_crm:E10_Transfer_of_Custody ;
    rdfs:range cidoc_crm:E39_Actor ;
    rdfs:subPropertyOf cidoc_crm:P14_carried_out_by .

cidoc_crm:P28i_surrendered_custody_through a owl:ObjectProperty ;
    rdfs:label "wurde Gewahrsam übergeben durch"@de,
        "παρέδωσε κατοχή μέσω"@el,
        "surrendered custody through"@en,
        "a cessé d’être détenteur à cause de"@fr,
        "final da custódia por meio de"@pt,
        "опека отдана через"@ru,
        "交出保管作业於"@zh ;
    rdfs:domain cidoc_crm:E39_Actor ;
    rdfs:range cidoc_crm:E10_Transfer_of_Custody ;
    rdfs:subPropertyOf cidoc_crm:P14i_performed .

cidoc_crm:P29_custody_received_by a owl:ObjectProperty ;
    rdfs:label "übertrug Gewahrsam auf"@de,
        "μετεβίβασε κατοχή σε"@el,
        "custody received by"@en,
        "changement de détenteur au profit de"@fr,
        "custódia recebida por"@pt,
        "опека получена"@ru,
        "移转保管作业给"@zh ;
    rdfs:comment """This property identifies the E39 Actor or Actors who receive custody of an instance of E18 Physical Thing in an E10 Transfer of Custody activity. \r
The property will typically describe Actors receiving custody of an object when it is handed over from another Actor’s care. On occasion, physical custody may be received involuntarily or illegally – through accident, unsolicited donation, or theft.\r
In reality, custody is either transferred to someone or from someone, or both.\r
"""@en ;
    rdfs:domain cidoc_crm:E10_Transfer_of_Custody ;
    rdfs:range cidoc_crm:E39_Actor ;
    rdfs:subPropertyOf cidoc_crm:P14_carried_out_by .

cidoc_crm:P29i_received_custody_through a owl:ObjectProperty ;
    rdfs:label "erhielt Gewahrsam durch"@de,
        "παρέλαβε κατοχή μέσω"@el,
        "received custody through"@en,
        "est devenu détenteur grâce à"@fr,
        "início da custódia por meio de"@pt,
        "получил опеку через"@ru,
        "取得保管作业於"@zh ;
    rdfs:domain cidoc_crm:E39_Actor ;
    rdfs:range cidoc_crm:E10_Transfer_of_Custody ;
    rdfs:subPropertyOf cidoc_crm:P14i_performed .

cidoc_crm:P30_transferred_custody_of a owl:ObjectProperty ;
    rdfs:label "übertrug Gewahrsam über"@de,
        "μετεβίβασε κατοχή του/της/των"@el,
        "transferred custody of"@en,
        "changement de détenteur concernant"@fr,
        "transferida custódia de"@pt,
        "передало опеку на"@ru,
        "有保管标的物"@zh ;
    rdfs:comment """This property identifies an item or items of E18 Physical Thing concerned in an E10 Transfer of Custody activity. \r
The property will typically describe the object that is handed over by an E39 Actor to another Actor’s custody. On occasion, physical custody may be transferred involuntarily or illegally – through accident, unsolicited donation, or theft.\r
"""@en ;
    rdfs:domain cidoc_crm:E10_Transfer_of_Custody ;
    rdfs:range cidoc_crm:E18_Physical_Thing .

cidoc_crm:P30i_custody_transferred_through a owl:ObjectProperty ;
    rdfs:label "wechselte Gewahrsam durch"@de,
        "άλλαξε κατοχή μέσω"@el,
        "custody transferred through"@en,
        "a changé de détenteur du fait de"@fr,
        "custódia transferida por meio de"@pt,
        "опека передана через"@ru,
        "被移转了保管作业於"@zh ;
    rdfs:domain cidoc_crm:E18_Physical_Thing ;
    rdfs:range cidoc_crm:E10_Transfer_of_Custody .

cidoc_crm:P32_used_general_technique a owl:ObjectProperty ;
    rdfs:label "benutzte das allgemeine Verfahren"@de,
        "χρησιμοποίησε γενική τεχνική"@el,
        "used general technique"@en,
        "a employé comme technique générique"@fr,
        "usou técnica geral"@pt,
        "использовал общую технику"@ru,
        "使用通用技术"@zh ;
    rdfs:comment """This property identifies the technique or method that was employed in an activity.\r
These techniques should be drawn from an external E55 Type hierarchy of consistent terminology of general techniques or methods such as embroidery, oil-painting, carbon dating, etc. Specific documented techniques should be described as instances of E29 Design or Procedure. This property identifies the technique that was employed in an act of modification.\r
"""@en ;
    rdfs:domain cidoc_crm:E7_Activity ;
    rdfs:range cidoc_crm:E55_Type ;
    rdfs:subPropertyOf cidoc_crm:P125_used_object_of_type .

cidoc_crm:P32i_was_technique_of a owl:ObjectProperty ;
    rdfs:label "war Verfahren von"@de,
        "ήταν τεχνική του/της"@el,
        "was technique of"@en,
        "a été la technique mise en œuvre dans"@fr,
        "foi técnica da"@pt,
        "был техникой для"@ru,
        "被使用於"@zh ;
    rdfs:domain cidoc_crm:E55_Type ;
    rdfs:range cidoc_crm:E7_Activity ;
    rdfs:subPropertyOf cidoc_crm:P125i_was_type_of_object_used_in .

cidoc_crm:P33_used_specific_technique a owl:ObjectProperty ;
    rdfs:label "benutzte das bestimmte Verfahren"@de,
        "χρησιμοποίησε συγκεκριμένη τεχνική"@el,
        "used specific technique"@en,
        "a employé comme technique spécifique"@fr,
        "usou técnica específica"@pt,
        "использовал особую технику"@ru,
        "使用特定技术"@zh ;
    rdfs:comment """This property identifies a specific instance of E29 Design or Procedure in order to carry out an instance of E7 Activity or parts of it. \r
The property differs from P32 used general technique (was technique of) in that P33 refers to an instance of E29 Design or Procedure, which is a concrete information object in its own right rather than simply being a term or a method known by tradition. \r
Typical examples would include intervention plans for conservation or the construction plans of a building.\r
"""@en ;
    rdfs:domain cidoc_crm:E7_Activity ;
    rdfs:range cidoc_crm:E29_Design_or_Procedure ;
    rdfs:subPropertyOf cidoc_crm:P16_used_specific_object .

cidoc_crm:P33i_was_used_by a owl:ObjectProperty ;
    rdfs:label "wurde benutzt von"@de,
        "χρησιμοποιήθηκε για"@el,
        "was used by"@en,
        "a été employée par"@fr,
        "foi usada por"@pt,
        "был использован посредством"@ru,
        "被特别使用於"@zh ;
    rdfs:domain cidoc_crm:E29_Design_or_Procedure ;
    rdfs:range cidoc_crm:E7_Activity ;
    rdfs:subPropertyOf cidoc_crm:P16i_was_used_for .

cidoc_crm:P34_concerned a owl:ObjectProperty ;
    rdfs:label "betraf"@de,
        "αφορούσε σε"@el,
        "concerned"@en,
        "a concerné"@fr,
        "interessada"@pt,
        "имел дело с"@ru,
        "评估了"@zh ;
    rdfs:comment """This property identifies the E18 Physical Thing that was assessed during an E14 Condition Assessment activity. \r
Conditions may be assessed either by direct observation or using recorded evidence. In the latter case the E18 Physical Thing does not need to be present or extant.\r
"""@en ;
    rdfs:domain cidoc_crm:E14_Condition_Assessment ;
    rdfs:range cidoc_crm:E18_Physical_Thing ;
    rdfs:subPropertyOf cidoc_crm:P140_assigned_attribute_to .

cidoc_crm:P34i_was_assessed_by a owl:ObjectProperty ;
    rdfs:label "wurde beurteilt durch"@de,
        "εκτιμήθηκε από"@el,
        "was assessed by"@en,
        "expertisé par le biais de"@fr,
        "foi avaliada por"@pt,
        "был оценен посредством"@ru,
        "被评估於"@zh ;
    rdfs:domain cidoc_crm:E18_Physical_Thing ;
    rdfs:range cidoc_crm:E14_Condition_Assessment ;
    rdfs:subPropertyOf cidoc_crm:P140i_was_attributed_by .

cidoc_crm:P35_has_identified a owl:ObjectProperty ;
    rdfs:label "hat identifiziert"@de,
        "έχει διαπιστώσει"@el,
        "has identified"@en,
        "a identifié"@fr,
        "identificou"@pt,
        "идентифицировал"@ru,
        "评估认定了"@zh ;
    rdfs:comment "This property identifies the E3 Condition State that was observed in an E14 Condition Assessment activity."@en ;
    rdfs:domain cidoc_crm:E14_Condition_Assessment ;
    rdfs:range cidoc_crm:E3_Condition_State ;
    rdfs:subPropertyOf cidoc_crm:P141_assigned .

cidoc_crm:P35i_was_identified_by a owl:ObjectProperty ;
    rdfs:label "wurde identifiziert durch"@de,
        "έχει διαπιστωθεί από"@el,
        "was identified by"@en,
        "est identifié par"@fr,
        "foi identificado por"@pt,
        "идентифицирован посредством"@ru,
        "被评估认定於"@zh ;
    rdfs:domain cidoc_crm:E3_Condition_State ;
    rdfs:range cidoc_crm:E14_Condition_Assessment ;
    rdfs:subPropertyOf cidoc_crm:P141i_was_assigned_by .

cidoc_crm:P37_assigned a owl:ObjectProperty ;
    rdfs:label "wies zu"@de,
        "απέδωσε"@el,
        "assigned"@en,
        "a attribué"@fr,
        "atribuiu"@pt,
        "назначил"@ru,
        "指定标识符为"@zh ;
    rdfs:comment """This property records the identifier that was assigned to an item in an Identifier Assignment activity.\r
The same identifier may be assigned on more than one occasion.\r
An Identifier might be created prior to an assignment.\r
"""@en ;
    rdfs:domain cidoc_crm:E15_Identifier_Assignment ;
    rdfs:range cidoc_crm:E42_Identifier ;
    rdfs:subPropertyOf cidoc_crm:P141_assigned .

cidoc_crm:P37i_was_assigned_by a owl:ObjectProperty ;
    rdfs:label "wurde zugewiesen durch"@de,
        "αποδόθηκε ως ιδιότητα από"@el,
        "was assigned by"@en,
        "a été attribuée par"@fr,
        "foi atribuído por"@pt,
        "был присвоен посредством"@ru,
        "被指定为标识符於"@zh ;
    rdfs:domain cidoc_crm:E42_Identifier ;
    rdfs:range cidoc_crm:E15_Identifier_Assignment ;
    rdfs:subPropertyOf cidoc_crm:P141i_was_assigned_by .

cidoc_crm:P38_deassigned a owl:ObjectProperty ;
    rdfs:label " hob Zuweisung auf von"@de,
        "ακύρωσε"@el,
        "deassigned"@en,
        "a désattribué"@fr,
        "retirou a atribuição do"@pt,
        "отменил назначение"@ru,
        "取消标识符"@zh ;
    rdfs:comment """This property records the identifier that was deassigned from an instance of E1 CRM Entity.\r
Deassignment of an identifier may be necessary when an item is taken out of an inventory, a new numbering system is introduced or items are merged or split up. \r
The same identifier may be deassigned on more than one occasion.\r
"""@en ;
    rdfs:domain cidoc_crm:E15_Identifier_Assignment ;
    rdfs:range cidoc_crm:E42_Identifier ;
    rdfs:subPropertyOf cidoc_crm:P141_assigned .

cidoc_crm:P38i_was_deassigned_by a owl:ObjectProperty ;
    rdfs:label "wurde aufgehoben durch"@de,
        "ακυρώθηκε από"@el,
        "was deassigned by"@en,
        "a été désattribué par"@fr,
        "foi retirada a atribuição por"@pt,
        "был отменен посредством"@ru,
        "被取消标识符於"@zh ;
    rdfs:domain cidoc_crm:E42_Identifier ;
    rdfs:range cidoc_crm:E15_Identifier_Assignment ;
    rdfs:subPropertyOf cidoc_crm:P141i_was_assigned_by .

cidoc_crm:P39_measured a owl:ObjectProperty ;
    rdfs:label "vermaß"@de,
        "μέτρησε"@el,
        "measured"@en,
        "a mesuré"@fr,
        "mediu"@pt,
        "измерил"@ru,
        "测量了"@zh ;
    rdfs:comment """This property associates an instance of E16 Measurement with the instance of E1 CRM Entity to which it applied. An instance of E1 CRM Entity may be measured more than once. Material and immaterial things and processes may be measured, e.g. the number of words in a text, or the duration of an event.\r
"""@en ;
    rdfs:domain cidoc_crm:E16_Measurement ;
    rdfs:range cidoc_crm:E1_CRM_Entity ;
    rdfs:subPropertyOf cidoc_crm:P140_assigned_attribute_to .

cidoc_crm:P39i_was_measured_by a owl:ObjectProperty ;
    rdfs:label "wurde vermessen durch"@de,
        "μετρήθηκε από"@el,
        "was measured by"@en,
        "a été mesuré par"@fr,
        "foi medida por"@pt,
        "был измерен посредством"@ru,
        "被测量於"@zh ;
    rdfs:domain cidoc_crm:E1_CRM_Entity ;
    rdfs:range cidoc_crm:E16_Measurement ;
    rdfs:subPropertyOf cidoc_crm:P140i_was_attributed_by .

cidoc_crm:P40_observed_dimension a owl:ObjectProperty ;
    rdfs:label "beobachtete Dimension"@de,
        "παρατήρησε"@el,
        "observed dimension"@en,
        "a relevé comme dimension"@fr,
        "verificou a dimensão"@pt,
        "определил величину"@ru,
        "观察认定的规模是"@zh ;
    rdfs:comment """This property records the dimension that was observed in an E16 Measurement Event.\r
E54 Dimension can be any quantifiable aspect of E70 Thing. Weight, image colour depth and monetary value are dimensions in this sense. One measurement activity may determine more than one dimension of one object.\r
Dimensions may be determined either by direct observation or using recorded evidence. In the latter case the measured Thing does not need to be present or extant.\r
Even though knowledge of the value of a dimension requires measurement, the dimension may be an object of discourse prior to, or even without, any measurement being made.\r
"""@en ;
    rdfs:domain cidoc_crm:E16_Measurement ;
    rdfs:range cidoc_crm:E54_Dimension ;
    rdfs:subPropertyOf cidoc_crm:P141_assigned .

cidoc_crm:P40i_was_observed_in a owl:ObjectProperty ;
    rdfs:label "wurde beobachtet in"@de,
        "παρατηρήθηκε από"@el,
        "was observed in"@en,
        "a été relevée au cours de"@fr,
        "foi verificada durante"@pt,
        "наблюдался в"@ru,
        "被观察认定於"@zh ;
    rdfs:domain cidoc_crm:E54_Dimension ;
    rdfs:range cidoc_crm:E16_Measurement ;
    rdfs:subPropertyOf cidoc_crm:P141i_was_assigned_by .

cidoc_crm:P41_classified a owl:ObjectProperty ;
    rdfs:label "klassifizierte"@de,
        "χαρακτήρισε"@el,
        "classified"@en,
        "a classifié"@fr,
        "classificou"@pt,
        "классифицировал"@ru,
        "分类了"@zh ;
    rdfs:comment """This property records the item to which a type was assigned in an E17 Type Assignment activity.\r
Any instance of a CRM entity may be assigned a type through type assignment. Type assignment events allow a more detailed path from E1 CRM Entity through P41 classified (was classified), E17 Type Assignment, P42 assigned (was assigned by) to E55 Type for assigning types to objects compared to the shortcut offered by P2 has type (is type of).\r
"""@en ;
    rdfs:domain cidoc_crm:E17_Type_Assignment ;
    rdfs:range cidoc_crm:E1_CRM_Entity ;
    rdfs:subPropertyOf cidoc_crm:P140_assigned_attribute_to .

cidoc_crm:P41i_was_classified_by a owl:ObjectProperty ;
    rdfs:label "wurde klassifiziert durch"@de,
        "χαρακτηρίσθηκε από"@el,
        "was classified by"@en,
        "a été classifiée par le biais de"@fr,
        "foi classificada por"@pt,
        "был классифицирован посредством"@ru,
        "被分类於"@zh ;
    rdfs:domain cidoc_crm:E1_CRM_Entity ;
    rdfs:range cidoc_crm:E17_Type_Assignment ;
    rdfs:subPropertyOf cidoc_crm:P140i_was_attributed_by .

cidoc_crm:P42_assigned a owl:ObjectProperty ;
    rdfs:label "wies zu"@de,
        "απέδωσε ως ιδιότητα"@el,
        "assigned"@en,
        "a attribué"@fr,
        "atribuiu"@pt,
        "назначил"@ru,
        "指定类型为"@zh ;
    rdfs:comment """This property records the type that was assigned to an entity by an E17 Type Assignment activity. \r
Type assignment events allow a more detailed path from E1 CRM Entity through P41 classified (was classified by), E17 Type Assignment, P42 assigned (was assigned by) to E55 Type for assigning types to objects compared to the shortcut offered by P2 has type (is type of).\r
For example, a fragment of an antique vessel could be assigned the type “attic red figured belly handled amphora” by expert A. The same fragment could be assigned the type “shoulder handled amphora” by expert B.\r
A Type may be intellectually constructed independent from assigning an instance of it.\r
"""@en ;
    rdfs:domain cidoc_crm:E17_Type_Assignment ;
    rdfs:range cidoc_crm:E55_Type ;
    rdfs:subPropertyOf cidoc_crm:P141_assigned .

cidoc_crm:P42i_was_assigned_by a owl:ObjectProperty ;
    rdfs:label "wurde zugewiesen durch"@de,
        "αποδόθηκε από"@el,
        "was assigned by"@en,
        "a été attribué par"@fr,
        "foi atribuído por"@pt,
        "был присвоен посредством"@ru,
        "被指定类型於"@zh ;
    rdfs:domain cidoc_crm:E55_Type ;
    rdfs:range cidoc_crm:E17_Type_Assignment ;
    rdfs:subPropertyOf cidoc_crm:P141i_was_assigned_by .

cidoc_crm:P43_has_dimension a owl:ObjectProperty ;
    rdfs:label "hat Dimension"@de,
        "έχει μέγεθος"@el,
        "has dimension"@en,
        "a pour dimension"@fr,
        "tem dimensão"@pt,
        "имеет величину"@ru,
        "有规模数量"@zh ;
    rdfs:comment """This property records a E54 Dimension of some E70 Thing.\r
It is a shortcut of the more fully developed path from E70 Thing through P39 measured (was measured by), E16 Measurement P40 observed dimension (was observed in) to E54 Dimension. It offers no information about how and when an E54 Dimension was established, nor by whom.\r
An instance of E54 Dimension is specific to an instance of E70 Thing.\r
"""@en ;
    rdfs:domain cidoc_crm:E70_Thing ;
    rdfs:range cidoc_crm:E54_Dimension .

cidoc_crm:P43i_is_dimension_of a owl:ObjectProperty ;
    rdfs:label "ist Dimension von"@de,
        "είναι μέγεθος του"@el,
        "is dimension of"@en,
        "est dimension de"@fr,
        "é dimensão de"@pt,
        "является величиной для"@ru,
        "估量的标的物是"@zh ;
    rdfs:domain cidoc_crm:E54_Dimension ;
    rdfs:range cidoc_crm:E70_Thing .

cidoc_crm:P44_has_condition a owl:ObjectProperty ;
    rdfs:label "hat Zustand"@de,
        "έχει κατάσταση"@el,
        "has condition"@en,
        "a pour état matériel"@fr,
        "tem estado material "@pt,
        "имеет условие"@ru,
        "有状态"@zh ;
    rdfs:comment """This property records an E3 Condition State for some E18 Physical Thing.\r
It is a shortcut of the more fully developed path from E18 Physical Thing through P34 concerned (was assessed by), E14 Condition Assessment P35 has identified (was identified by) to E3 Condition State. It offers no information about how and when the E3 Condition State was established, nor by whom. \r
An instance of Condition State is specific to an instance of Physical Thing.\r
"""@en ;
    rdfs:domain cidoc_crm:E18_Physical_Thing ;
    rdfs:range cidoc_crm:E3_Condition_State .

cidoc_crm:P44i_is_condition_of a owl:ObjectProperty ;
    rdfs:label "ist Zustand von"@de,
        "είναι κατάσταση του"@el,
        "is condition of"@en,
        "état matériel de"@fr,
        "estado material de"@pt,
        "является условием для"@ru,
        "描述的标的物是"@zh ;
    rdfs:domain cidoc_crm:E3_Condition_State ;
    rdfs:range cidoc_crm:E18_Physical_Thing .

cidoc_crm:P45_consists_of a owl:ObjectProperty ;
    rdfs:label "besteht aus"@de,
        "αποτελείται από"@el,
        "consists of"@en,
        "consiste en"@fr,
        "consiste de"@pt,
        "составлен из"@ru,
        "有构成材料"@zh ;
    rdfs:comment """This property identifies the instances of E57 Materials of which an instance of E18 Physical Thing is composed.\r
All physical things consist of physical materials. P45 consists of (is incorporated in) allows the different Materials to be recorded. P45 consists of (is incorporated in) refers here to observed Material as opposed to the consumed raw material.\r
A Material, such as a theoretical alloy, may not have any physical instances"""@en ;
    rdfs:domain cidoc_crm:E18_Physical_Thing ;
    rdfs:range cidoc_crm:E57_Material .

cidoc_crm:P45i_is_incorporated_in a owl:ObjectProperty ;
    rdfs:label "ist enthalten in"@de,
        "είναι ενσωματωμένος/η/ο σε"@el,
        "is incorporated in"@en,
        "est présent dans"@fr,
        "está presente em"@pt,
        "входит в состав"@ru,
        "被用来构成"@zh ;
    rdfs:domain cidoc_crm:E57_Material ;
    rdfs:range cidoc_crm:E18_Physical_Thing .

cidoc_crm:P48_has_preferred_identifier a owl:ObjectProperty ;
    rdfs:label "hat bevorzugtes Kennzeichen"@de,
        "έχει προτιμώμενο αναγνωριστικό"@el,
        "has preferred identifier"@en,
        "a pour identificateur retenu"@fr,
        "tem identificador preferido"@pt,
        "имеет предпочтительный идентификатор"@ru,
        "有首选标识符"@zh ;
    rdfs:comment """This property records the preferred E42 Identifier that was used to identify an instance of E1 CRM Entity at the time this property was recorded.\r
More than one preferred identifier may have been assigned to an item over time.\r
Use of this property requires an external mechanism for assigning temporal validity to the respective CRM instance.\r
P48 has preferred identifier (is preferred identifier of), is a shortcut for the path from E1 CRM Entity through P140 assigned attribute to (was attributed by), E15 Identifier Assignment, P37 assigned (was assigned by) to E42 Identifier. The fact that an identifier is a preferred one for an organisation can be better expressed in a context independent form by assigning a suitable E55 Type to the respective instance of E15 Identifier Assignment using the P2 has type property.\r
"""@en ;
    rdfs:domain cidoc_crm:E1_CRM_Entity ;
    rdfs:range cidoc_crm:E42_Identifier ;
    rdfs:subPropertyOf cidoc_crm:P1_is_identified_by .

cidoc_crm:P48i_is_preferred_identifier_of a owl:ObjectProperty ;
    rdfs:label "ist bevorzugtes Kennzeichen für"@de,
        "είναι προτιμώμενο αναγνωριστικό"@el,
        "is preferred identifier of"@en,
        "est l’identificateur retenu de"@fr,
        "é o identificador preferido de"@pt,
        "является предпочтительным идентификатором для"@ru,
        "首选标识符的标的物是"@zh ;
    rdfs:domain cidoc_crm:E42_Identifier ;
    rdfs:range cidoc_crm:E1_CRM_Entity ;
    rdfs:subPropertyOf cidoc_crm:P1i_identifies .

cidoc_crm:P4_has_time-span a owl:ObjectProperty ;
    rdfs:label "hat Zeitspanne"@de,
        "βρισκόταν σε εξέλιξη"@el,
        "has time-span"@en,
        "a pour durée"@fr,
        "tem período de tempo"@pt,
        "имеет временной отрезок"@ru,
        "发生时段是"@zh ;
    rdfs:comment """This property describes the temporal confinement of an instance of an E2 Temporal Entity.\r
The related E52 Time-Span is understood as the real Time-Span during which the phenomena were active, which make up the temporal entity instance. It does not convey any other meaning than a positioning on the “time-line” of chronology. The Time-Span in turn is approximated by a set of dates (E61 Time Primitive). A temporal entity can have in reality only one Time-Span, but there may exist alternative opinions about it, which we would express by assigning multiple Time-Spans. Related temporal entities may share a Time-Span. Time-Spans may have completely unknown dates but other descriptions by which we can infer knowledge.\r
"""@en ;
    rdfs:domain cidoc_crm:E2_Temporal_Entity ;
    rdfs:range cidoc_crm:E52_Time-Span .

cidoc_crm:P4i_is_time-span_of a owl:ObjectProperty ;
    rdfs:label "ist Zeitspanne von"@de,
        "είναι χρονικό διάστημα του/της"@el,
        "is time-span of"@en,
        "est la durée de"@fr,
        "é o período de tempo de"@pt,
        "является временным отрезком для"@ru,
        "开始并完成了"@zh ;
    rdfs:domain cidoc_crm:E52_Time-Span ;
    rdfs:range cidoc_crm:E2_Temporal_Entity .

cidoc_crm:P50_has_current_keeper a owl:ObjectProperty ;
    rdfs:label "hat derzeitigen Betreuer"@de,
        "είναι στην κατοχή του"@el,
        "has current keeper"@en,
        "est actuellement détenu par"@fr,
        "é guardada por"@pt,
        "имеет текущего смотрителя"@ru,
        "有现任保管者"@zh ;
    rdfs:comment """This property identifies the E39 Actor or Actors who had custody of an instance of E18 Physical Thing at the time of validity of the record or database containing the statement that uses this property.\r
	P50 has current keeper (is current keeper of) is a shortcut for the more detailed path from E18 Physical Thing through P30 transferred custody of (custody transferred through), E10 Transfer of Custody, P29 custody received by (received custody through) to E39 Actor.\r
"""@en ;
    rdfs:domain cidoc_crm:E18_Physical_Thing ;
    rdfs:range cidoc_crm:E39_Actor ;
    rdfs:subPropertyOf cidoc_crm:P49_has_former_or_current_keeper .

cidoc_crm:P50i_is_current_keeper_of a owl:ObjectProperty ;
    rdfs:label "ist derzeitiger Betreuer von"@de,
        "κατέχει"@el,
        "is current keeper of"@en,
        "est actuel détenteur de"@fr,
        "é guardador de"@pt,
        "является текущим смотрителем для"@ru,
        "目前保管"@zh ;
    rdfs:domain cidoc_crm:E39_Actor ;
    rdfs:range cidoc_crm:E18_Physical_Thing ;
    rdfs:subPropertyOf cidoc_crm:P49i_is_former_or_current_keeper_of .

cidoc_crm:P52_has_current_owner a owl:ObjectProperty ;
    rdfs:label "hat derzeitigen Besitzer"@de,
        "έχει ιδιοκτήτη"@el,
        "has current owner"@en,
        "est actuellement possédée par"@fr,
        "é propriedade de"@pt,
        "имеет текущего владельца"@ru,
        "有现任物主"@zh ;
    rdfs:comment """This property identifies the E21 Person, E74 Group or E40 Legal Body that was the owner of an instance of E18 Physical Thing at the time of validity of the record or database containing the statement that uses this property.\r
P52 has current owner (is current owner of) is a shortcut for the more detailed path from E18 Physical Thing through P24 transferred title of (changed ownership through), E8 Acquisition, P22 transferred title to (acquired title through) to E39 Actor, if and only if this acquisition event is the most recent.\r
"""@en ;
    rdfs:domain cidoc_crm:E18_Physical_Thing ;
    rdfs:range cidoc_crm:E39_Actor ;
    rdfs:subPropertyOf cidoc_crm:P105_right_held_by,
        cidoc_crm:P51_has_former_or_current_owner .

cidoc_crm:P52i_is_current_owner_of a owl:ObjectProperty ;
    rdfs:label "ist derzeitiger Besitzer von"@de,
        "είναι ιδιοκτήτης του"@el,
        "is current owner of"@en,
        "est le propriétaire actuel de"@fr,
        "é proprietário de"@pt,
        "является текущим владельцем для"@ru,
        "目前拥有"@zh ;
    rdfs:domain cidoc_crm:E39_Actor ;
    rdfs:range cidoc_crm:E18_Physical_Thing ;
    rdfs:subPropertyOf cidoc_crm:P105i_has_right_on,
        cidoc_crm:P51i_is_former_or_current_owner_of .

cidoc_crm:P54_has_current_permanent_location a owl:ObjectProperty ;
    rdfs:label "hat derzeitigen permanenten Standort"@de,
        "έχει μόνιμη θέση"@el,
        "has current permanent location"@en,
        "a actuellement pour localisation à demeure"@fr,
        "é localizado permanentemente em"@pt,
        "имеет текущее постоянное местоположение"@ru,
        "目前的永久位置位於"@zh ;
    rdfs:comment """This property records the foreseen permanent location of an instance of E19 Physical Object at the time of validity of the record or database containing the statement that uses this property.\r
P54 has current permanent location (is current permanent location of) is similar to P55 has current location (currently holds). However, it indicates the E53 Place currently reserved for an object, such as the permanent storage location or a permanent exhibit location. The object may be temporarily removed from the permanent location, for example when used in temporary exhibitions or loaned to another institution. The object may never actually be located at its permanent location.\r
"""@en ;
    rdfs:domain cidoc_crm:E19_Physical_Object ;
    rdfs:range cidoc_crm:E53_Place .

cidoc_crm:P54i_is_current_permanent_location_of a owl:ObjectProperty ;
    rdfs:label "ist derzeitiger permanenter Standort von"@de,
        "είναι μόνιμη θέση του/της"@el,
        "is current permanent location of"@en,
        "est actuellement localisation à demeure de"@fr,
        "é localização permanente de"@pt,
        "является текущим постоянным местоположением для"@ru,
        "目前被用来永久置放"@zh ;
    rdfs:domain cidoc_crm:E53_Place ;
    rdfs:range cidoc_crm:E19_Physical_Object .

cidoc_crm:P55_has_current_location a owl:ObjectProperty ;
    rdfs:label "hat derzeitigen Standort"@de,
        "βρίσκεται σε"@el,
        "has current location"@en,
        "a pour localisation actuelle"@fr,
        "é localizado em"@pt,
        "в данный момент находится в"@ru,
        "目前被置放於"@zh ;
    rdfs:comment """This property records the location of an E19 Physical Object at the time of validity of the record or database containing the statement that uses this property. \r
	This property is a specialisation of P53 has former or current location (is former or current location of). It indicates that the E53 Place associated with the E19 Physical Object is the current location of the object. The property does not allow any indication of how long the Object has been at the current location. \r
P55 has current location (currently holds) is a shortcut. A more detailed representation can make use of the fully developed (i.e. indirect) path from E19 Physical Object through P25 moved (moved by), E9 Move P26 moved to (was destination of) to E53 Place if and only if this Move is the most recent.\r
"""@en ;
    rdfs:domain cidoc_crm:E19_Physical_Object ;
    rdfs:range cidoc_crm:E53_Place ;
    rdfs:subPropertyOf cidoc_crm:P53_has_former_or_current_location .

cidoc_crm:P55i_currently_holds a owl:ObjectProperty ;
    rdfs:label "hält derzeitig"@de,
        "είναι θέση του"@el,
        "currently holds"@en,
        "est localisation actuelle de"@fr,
        "é localização atual de"@pt,
        "в данный момент содержит"@ru,
        "目前置放了"@zh ;
    rdfs:domain cidoc_crm:E53_Place ;
    rdfs:range cidoc_crm:E19_Physical_Object ;
    rdfs:subPropertyOf cidoc_crm:P53i_is_former_or_current_location_of .

cidoc_crm:P56_bears_feature a owl:ObjectProperty ;
    rdfs:label "trägt Merkmal"@de,
        "φέρει μόρφωμα"@el,
        "bears feature"@en,
        "présente pour caractéristique"@fr,
        "possui característica"@pt,
        "несет признак"@ru,
        "有外貌表征"@zh ;
    rdfs:comment """This property links an instance of E19 Physical Object to an instance of E26 Physical Feature that it bears.\r
An E26 Physical Feature can only exist on one object. One object may bear more than one E26 Physical Feature. An E27 Site should be considered as an E26 Physical Feature on the surface of the Earth.\r
An instance B of E26 Physical Feature being a detail of the structure of another instance A of E26 Physical Feature can be linked to B by use of the property P46 is composed of (forms part of). This implies that the subfeature B is P56i found on the same E19 Physical Object as A.\r
P56 bears feature (is found on) is a shortcut. A more detailed representation can make use of the fully developed (i.e. indirect) path from E19 Physical Object through P59 has section (is located on or\r
Definition of the CIDOC Conceptual Reference Model 149 within), E53 Place, P53 has former or current location (is former or current location of) to E26 Physical Feature.\r
"""@en ;
    rdfs:domain cidoc_crm:E19_Physical_Object ;
    rdfs:range cidoc_crm:E26_Physical_Feature ;
    rdfs:subPropertyOf cidoc_crm:P46_is_composed_of .

cidoc_crm:P56i_is_found_on a owl:ObjectProperty ;
    rdfs:label "wird gefunden auf"@de,
        "βρίσκεται σε"@el,
        "is found on"@en,
        "se trouve sur"@fr,
        "é encontrada em"@pt,
        "найден на"@ru,
        "被见於"@zh ;
    rdfs:domain cidoc_crm:E26_Physical_Feature ;
    rdfs:range cidoc_crm:E19_Physical_Object ;
    rdfs:subPropertyOf cidoc_crm:P46i_forms_part_of .

cidoc_crm:P57_has_number_of_parts a owl:DatatypeProperty ;
    rdfs:label "hat Anzahl Teile"@de,
        "έχει αριθμό μερών"@el,
        "has number of parts"@en,
        "a pour nombre de parties"@fr,
        "tem número de partes"@pt,
        "имеет число частей"@ru,
        "有组件数目"@zh ;
    rdfs:comment """This property documents the E60 Number of parts of which an instance of E19 Physical Object is composed.\r
This may be used as a method of checking inventory counts with regard to aggregate or collective objects. What constitutes a part or component depends on the context and requirements of the documentation. Normally, the parts documented in this way would not be considered as worthy of individual attention.\r
For a more complete description, objects may be decomposed into their components and constituents using P46 is composed of (forms parts of) and P45 consists of (is incorporated in). This allows each element to be described individually.\r
"""@en ;
    rdfs:domain cidoc_crm:E19_Physical_Object ;
    rdfs:range rdfs:Literal .

cidoc_crm:P58_has_section_definition a owl:ObjectProperty ;
    rdfs:label "hat Abschittsdefinition"@de,
        "έχει ορισμό τμήματος"@el,
        "has section definition"@en,
        "a pour désignation de section"@fr,
        "tem designação de seção"@pt,
        "имеет определение района"@ru,
        "有区域定义"@zh ;
    rdfs:comment """This property links an area (section) named by a E46 Section Definition to the instance of E18 Physical Thing upon which it is found.\r
The CRM handles sections as locations (instances of E53 Place) within or on E18 Physical Thing that are identified by E46 Section Definitions. Sections need not be discrete and separable components or parts of an object.\r
This is part of a more developed path from E18 Physical Thing through P58, E46 Section Definition, P87 is identified by (identifies) that allows a more precise definition of a location found on an object than the shortcut P59 has section (is located on or within).\r
A particular instance of a Section Definition only applies to one instance of Physical Thing."""@en ;
    rdfs:domain cidoc_crm:E18_Physical_Thing ;
    rdfs:range cidoc_crm:E46_Section_Definition .

cidoc_crm:P58i_defines_section a owl:ObjectProperty ;
    rdfs:label "definiert Abschitt auf oder von"@de,
        "ορίζει τμήμα σε"@el,
        "defines section"@en,
        "définit une section de"@fr,
        "define uma seção de"@pt,
        "определяет район"@ru,
        "界定了区域於"@zh ;
    rdfs:domain cidoc_crm:E46_Section_Definition ;
    rdfs:range cidoc_crm:E18_Physical_Thing .

cidoc_crm:P5_consists_of a owl:ObjectProperty ;
    rdfs:label "besteht aus"@de,
        "αποτελείται από"@el,
        "consists of"@en,
        "consiste en"@fr,
        "consiste de"@pt,
        "состоит из"@ru,
        "包含"@zh ;
    rdfs:comment """This property describes the decomposition of an E3 Condition State into discrete, subsidiary states. \r
It is assumed that the sub-states into which the condition state is analysed form a logical whole - although the entire story may not be completely known – and that the sub-states are in fact constitutive of the general condition state. For example, a general condition state of “in ruins” may be decomposed into the individual stages of decay"""@en ;
    rdfs:domain cidoc_crm:E3_Condition_State ;
    rdfs:range cidoc_crm:E3_Condition_State .

cidoc_crm:P5i_forms_part_of a owl:ObjectProperty ;
    rdfs:label "bildet Teil von"@de,
        "αποτελεί μέρος του/της"@el,
        "forms part of"@en,
        "fait partie de"@fr,
        "faz parte de"@pt,
        "формирует часть"@ru,
        "组成了"@zh ;
    rdfs:domain cidoc_crm:E3_Condition_State ;
    rdfs:range cidoc_crm:E3_Condition_State .

cidoc_crm:P62_depicts a owl:ObjectProperty ;
    rdfs:label "bildet ab"@de,
        "απεικονίζει"@el,
        "depicts"@en,
        "figure"@fr,
        "retrata"@pt,
        "описывает"@ru,
        "描绘"@zh ;
    rdfs:comment """This property identifies something that is depicted by an instance of E24 Physical Man-Made Thing. Depicting is meant in the sense that the surface of the E24 Physical Man-Made Thing shows, through its passive optical qualities or form, a representation of the entity depicted. It does not pertain to inscriptions or any other information encoding.\r
\r
This property is a shortcut of the more fully developed path from E24 Physical Man-Made Thing through P65 shows visual item (is shown by), E36 Visual Item, P138 represents (has representation) to E1 CRM Entity. P62.1 mode of depiction allows the nature of the depiction to be refined.\r
"""@en ;
    rdfs:domain cidoc_crm:E24_Physical_Man-Made_Thing ;
    rdfs:range cidoc_crm:E1_CRM_Entity .

cidoc_crm:P62i_is_depicted_by a owl:ObjectProperty ;
    rdfs:label "wird abgebildet durch"@de,
        "απεικονίζεται σε"@el,
        "is depicted by"@en,
        "est figurée sur"@fr,
        "é retratada por"@pt,
        "описан посредством"@ru,
        "被描绘於"@zh ;
    rdfs:domain cidoc_crm:E1_CRM_Entity ;
    rdfs:range cidoc_crm:E24_Physical_Man-Made_Thing .

cidoc_crm:P65_shows_visual_item a owl:ObjectProperty ;
    rdfs:label "zeigt Bildliches"@de,
        "εμφανίζει οπτικό στοιχείο"@el,
        "shows visual item"@en,
        "présente l'item visuel"@fr,
        "apresenta item visual"@pt,
        "показывает визуальный предмет"@ru,
        "显示视觉项目"@zh ;
    rdfs:comment """This property documents an E36 Visual Item shown by an instance of E24 Physical Man-Made Thing.\r
This property is similar to P62 depicts (is depicted by) in that it associates an item of E24 Physical Man-Made Thing with a visual representation. However, P65 shows visual item (is shown by) differs from the P62 depicts (is depicted by) property in that it makes no claims about what the E36 Visual Item is deemed to represent. E36 Visual Item identifies a recognisable image or visual symbol, regardless of what this image may or may not represent.\r
For example, all recent British coins bear a portrait of Queen Elizabeth II, a fact that is correctly documented using P62 depicts (is depicted by). Different portraits have been used at different periods, however. P65 shows visual item (is shown by) can be used to refer to a particular portrait.\r
P65 shows visual item (is shown by) may also be used for Visual Items such as signs, marks and symbols, for example the 'Maltese Cross' or the 'copyright symbol’ that have no particular representational content. \r
This property is part of the fully developed path from E24 Physical Man-Made Thing through P65 shows visual item (is shown by), E36 Visual Item, P138 represents (has representation) to E1 CRM Entity which is shortcut by, P62 depicts (is depicted by).\r
"""@en ;
    rdfs:domain cidoc_crm:E24_Physical_Man-Made_Thing ;
    rdfs:range cidoc_crm:E36_Visual_Item ;
    rdfs:subPropertyOf cidoc_crm:P128_carries .

cidoc_crm:P65i_is_shown_by a owl:ObjectProperty ;
    rdfs:label "wird gezeigt durch"@de,
        "εμφανίζεται σε"@el,
        "is shown by"@en,
        "est présenté par"@fr,
        "é apresentado por"@pt,
        "показан посредством"@ru,
        "被显示於"@zh ;
    rdfs:domain cidoc_crm:E36_Visual_Item ;
    rdfs:range cidoc_crm:E24_Physical_Man-Made_Thing ;
    rdfs:subPropertyOf cidoc_crm:P128i_is_carried_by .

cidoc_crm:P68_foresees_use_of a owl:ObjectProperty ;
    rdfs:label " sieht den Gebrauch vor von"@de,
        "συνήθως χρησιμοποιεί"@el,
        "foresees use of"@en,
        "utilise habituellement"@fr,
        "normalmente emprega"@pt,
        "обычно применяет"@ru,
        "指定使用材料"@zh ;
    rdfs:comment """This property identifies an E57 Material foreseeen to be used by an E29 Design or Procedure. \r
E29 Designs and procedures commonly foresee the use of particular E57 Materials. The fabrication of adobe bricks, for example, requires straw, clay and water. This property enables this to be documented.\r
This property is not intended for the documentation of E57 Materials that were used on a particular occasion when an instance of E29 Design or Procedure was executed.\r
"""@en ;
    rdfs:domain cidoc_crm:E29_Design_or_Procedure ;
    rdfs:range cidoc_crm:E57_Material ;
    rdfs:subPropertyOf cidoc_crm:P67_refers_to .

cidoc_crm:P68i_use_foreseen_by a owl:ObjectProperty ;
    rdfs:label "vorgesehen für Gebrauch durch defined"@de,
        "συνήθως χρησιμοποιείται από"@el,
        "use foreseen by"@en,
        "est habituellement utilisé par"@fr,
        "é empregado por"@pt,
        "обычно используется посредством"@ru,
        "被指定使用於"@zh ;
    rdfs:domain cidoc_crm:E57_Material ;
    rdfs:range cidoc_crm:E29_Design_or_Procedure ;
    rdfs:subPropertyOf cidoc_crm:P67i_is_referred_to_by .

cidoc_crm:P69_is_associated_with a owl:ObjectProperty ;
    rdfs:label "ist verbunden mit"@de,
        "σχετίζεται με"@el,
        "is associated with"@en,
        "est associée à"@fr,
        "é associado com"@pt,
        "ассоциирован с"@ru,
        "相关於"@zh ;
    rdfs:comment """This property generalises relationships like whole-part, sequence, prerequisite or inspired by between instances of E29 Design or Procedure. Any instance of E29 Design or Procedure may be associated with other designs or procedures. The property is considered to be symmetrical unless otherwise indicated by P69.1 has type.\r
The P69.1 has type property of P69 has association with allows the nature of the association to be specified reading from domain to range; examples of types of association between instances of E29 Design or Procedure include: has part, follows, requires, etc.\r
The property can typically be used to model the decomposition of the description of a complete workflow into a series of separate procedures.\r
"""@en ;
    rdfs:domain cidoc_crm:E29_Design_or_Procedure ;
    rdfs:range cidoc_crm:E29_Design_or_Procedure .

cidoc_crm:P70_documents a owl:ObjectProperty ;
    rdfs:label "belegt"@de,
        "τεκμηριώνει"@el,
        "documents"@en,
        "mentionne"@fr,
        "documenta"@pt,
        "документирует"@ru,
        "记录了"@zh ;
    rdfs:comment """This property describes the CRM Entities documented by instances of E31 Document.\r
Documents may describe any conceivable entity, hence the link to the highest-level entity in the CRM hierarchy. This property is intended for cases where a reference is regarded as being of a documentary character, in the scholarly or scientific sense.\r
"""@en ;
    rdfs:domain cidoc_crm:E31_Document ;
    rdfs:range cidoc_crm:E1_CRM_Entity ;
    rdfs:subPropertyOf cidoc_crm:P67_refers_to .

cidoc_crm:P70i_is_documented_in a owl:ObjectProperty ;
    rdfs:label "wird belegt in"@de,
        "τεκμηριώνεται σε"@el,
        "is documented in"@en,
        "est mentionnée dans"@fr,
        "é documentado em"@pt,
        "документирован в"@ru,
        "被记录於"@zh ;
    rdfs:domain cidoc_crm:E1_CRM_Entity ;
    rdfs:range cidoc_crm:E31_Document ;
    rdfs:subPropertyOf cidoc_crm:P67i_is_referred_to_by .

cidoc_crm:P71_lists a owl:ObjectProperty ;
    rdfs:label "listet"@de,
        "περιλαμβάνει"@el,
        "lists"@en,
        "définit"@fr,
        "define"@pt,
        "перечисляет"@ru,
        "条列出"@zh ;
    rdfs:comment """This property documents a source E32 Authority Document for an instance of an E1 CRM Entity.\r
"""@en ;
    rdfs:domain cidoc_crm:E32_Authority_Document ;
    rdfs:range cidoc_crm:E1_CRM_Entity ;
    rdfs:subPropertyOf cidoc_crm:P67_refers_to .

cidoc_crm:P71i_is_listed_in a owl:ObjectProperty ;
    rdfs:label "wird aufgelistet in"@de,
        "περιλαμβάνεται σε"@el,
        "is listed in"@en,
        "est défini par"@fr,
        "é definido por"@pt,
        "перечислен в"@ru,
        "被条列於"@zh ;
    rdfs:domain cidoc_crm:E1_CRM_Entity ;
    rdfs:range cidoc_crm:E32_Authority_Document ;
    rdfs:subPropertyOf cidoc_crm:P67i_is_referred_to_by .

cidoc_crm:P72_has_language a owl:ObjectProperty ;
    rdfs:label "hat Sprache"@de,
        "έχει γλώσσα"@el,
        "has language"@en,
        "est en langue"@fr,
        "é da língua "@pt,
        "имеет язык"@ru,
        "使用语言"@zh ;
    rdfs:comment """This property describes the E56 Language of an E33 Linguistic Object. \r
Linguistic Objects are composed in one or more human Languages. This property allows these languages to be documented.\r
"""@en ;
    rdfs:domain cidoc_crm:E33_Linguistic_Object ;
    rdfs:range cidoc_crm:E56_Language .

cidoc_crm:P72i_is_language_of a owl:ObjectProperty ;
    rdfs:label "ist Sprache von"@de,
        "είναι γλώσσα του/της"@el,
        "is language of"@en,
        "est la langue de"@fr,
        "é a língua de"@pt,
        "является языком для"@ru,
        "被用来撰写"@zh ;
    rdfs:domain cidoc_crm:E56_Language ;
    rdfs:range cidoc_crm:E33_Linguistic_Object .

cidoc_crm:P73_has_translation a owl:ObjectProperty ;
    rdfs:label "hat Übersetzung"@de,
        "έχει μετάφραση"@el,
        "has translation"@en,
        "a pour traduction"@fr,
        "tem tradução"@pt,
        "имеет перевод"@ru,
        "有译文"@zh ;
    rdfs:comment """This property describes the source and target of instances of E33Linguistic Object involved in a translation.\r
When a Linguistic Object is translated into a new language it becomes a new Linguistic Object, despite being conceptually similar to the source object.\r
"""@en ;
    rdfs:domain cidoc_crm:E33_Linguistic_Object ;
    rdfs:range cidoc_crm:E33_Linguistic_Object ;
    rdfs:subPropertyOf cidoc_crm:P130i_features_are_also_found_on .

cidoc_crm:P73i_is_translation_of a owl:ObjectProperty ;
    rdfs:label "ist Übersetzung von"@de,
        "είναι μετάφραση του/της"@el,
        "is translation of"@en,
        "est la traduction de"@fr,
        "é tradução de"@pt,
        "является переводом"@ru,
        "翻译自"@zh ;
    rdfs:domain cidoc_crm:E33_Linguistic_Object ;
    rdfs:range cidoc_crm:E33_Linguistic_Object ;
    rdfs:subPropertyOf cidoc_crm:P130_shows_features_of .

cidoc_crm:P74_has_current_or_former_residence a owl:ObjectProperty ;
    rdfs:label "hat derzeitigen oder früheren Sitz"@de,
        "έχει ή είχε κατοικία"@el,
        "has current or former residence"@en,
        "réside ou a résidé à"@fr,
        "reside ou residiu em"@pt,
        "имеет текущее или бывшее местожительства"@ru,
        "目前或曾经居住於"@zh ;
    rdfs:comment """This property describes the current or former E53 Place of residence of an E39 Actor. \r
The residence may be either the Place where the Actor resides, or a legally registered address of any kind.\r
"""@en ;
    rdfs:domain cidoc_crm:E39_Actor ;
    rdfs:range cidoc_crm:E53_Place .

cidoc_crm:P74i_is_current_or_former_residence_of a owl:ObjectProperty ;
    rdfs:label "ist derzeitiger oder früherer Sitz von"@de,
        "είναι ή ήταν κατοικία του/της"@el,
        "is current or former residence of"@en,
        "est ou a été la résidence de"@fr,
        "é ou foi residência de"@pt,
        "является текущим или бывшим местом жительства для"@ru,
        "历年来的居住者包括"@zh ;
    rdfs:domain cidoc_crm:E53_Place ;
    rdfs:range cidoc_crm:E39_Actor .

cidoc_crm:P75_possesses a owl:ObjectProperty ;
    rdfs:label "besitzt"@de,
        "κατέχει"@el,
        "possesses"@en,
        "est détenteur de"@fr,
        "é detentor de"@pt,
        "владеет"@ru,
        "拥有"@zh ;
    rdfs:comment "This property identifies former or current instances of E30 Rights held by an E39 Actor."@en ;
    rdfs:domain cidoc_crm:E39_Actor ;
    rdfs:range cidoc_crm:E30_Right .

cidoc_crm:P75i_is_possessed_by a owl:ObjectProperty ;
    rdfs:label "sind im Besitz von"@de,
        "κατέχεται από"@el,
        "is possessed by"@en,
        "est détenu par"@fr,
        "são detidos por"@pt,
        "принадлежит"@ru,
        "有拥有者"@zh ;
    rdfs:domain cidoc_crm:E30_Right ;
    rdfs:range cidoc_crm:E39_Actor .

cidoc_crm:P76_has_contact_point a owl:ObjectProperty ;
    rdfs:label "hat Kontaktpunkt"@de,
        "έχει σημείο επικοινωνίας"@el,
        "has contact point"@en,
        "a pour coordonnées individuelles"@fr,
        "possui ponto de contato"@pt,
        "имеет контакт"@ru,
        "有联系方式"@zh ;
    rdfs:comment """This property identifies an E51 Contact Point of any type that provides access to an E39 Actor by any communication method, such as e-mail or fax.\r
"""@en ;
    rdfs:domain cidoc_crm:E39_Actor ;
    rdfs:range cidoc_crm:E51_Contact_Point .

cidoc_crm:P76i_provides_access_to a owl:ObjectProperty ;
    rdfs:label "bietet Zugang zu"@de,
        "παρέχει πρόσβαση σε"@el,
        "provides access to"@en,
        "permettent de contacter"@fr,
        "é ponto de contado de"@pt,
        "предоставляет доступ к"@ru,
        "被用来联系"@zh ;
    rdfs:domain cidoc_crm:E51_Contact_Point ;
    rdfs:range cidoc_crm:E39_Actor .

cidoc_crm:P78_is_identified_by a owl:ObjectProperty ;
    rdfs:label "wird bezeichnet als"@de,
        "αναγνωρίζεται ως"@el,
        "is identified by"@en,
        "est identifiée par"@fr,
        "é identificado por "@pt,
        "идентифицируется посредством"@ru,
        "有识别称号"@zh ;
    rdfs:comment "This property identifies an E52 Time-Span using an E49Time Appellation."@en ;
    rdfs:domain cidoc_crm:E52_Time-Span ;
    rdfs:range cidoc_crm:E49_Time_Appellation ;
    rdfs:subPropertyOf cidoc_crm:P1_is_identified_by .

cidoc_crm:P78i_identifies a owl:ObjectProperty ;
    rdfs:label "bezeichnet"@de,
        "είναι αναγνωριστικό"@el,
        "identifies"@en,
        "identifie"@fr,
        "identifica"@pt,
        "идентифицирует"@ru,
        "被用来识别"@zh ;
    rdfs:domain cidoc_crm:E49_Time_Appellation ;
    rdfs:range cidoc_crm:E52_Time-Span ;
    rdfs:subPropertyOf cidoc_crm:P1i_identifies .

cidoc_crm:P79_beginning_is_qualified_by a owl:DatatypeProperty ;
    rdfs:label "hat Anfangsbegründung"@de,
        "αρχή προσδιορίζεται από"@el,
        "beginning is qualified by"@en,
        "début est qualifié par"@fr,
        "início é qualificado por"@pt,
        "начало ограничено"@ru,
        "起点认定的性质是"@zh ;
    rdfs:comment """This property qualifies the beginning of an E52 Time-Span in some way. \r
The nature of the qualification may be certainty, precision, source etc.\r
"""@en ;
    rdfs:domain cidoc_crm:E52_Time-Span ;
    rdfs:range rdfs:Literal ;
    rdfs:subPropertyOf cidoc_crm:P3_has_note .

cidoc_crm:P7_took_place_at a owl:ObjectProperty ;
    rdfs:label "fand statt in"@de,
        "έλαβε χώρα σε"@el,
        "took place at"@en,
        "a eu lieu dans"@fr,
        "ocorreu em"@pt,
        "совершался на"@ru,
        "发生地在"@zh ;
    rdfs:comment """This property describes the spatial location of an instance of E4 Period. \r
\r
The related E53 Place should be seen as an approximation of the geographical area within which the phenomena that characterise the period in question occurred. P7took place at (witnessed) does not convey any meaning other than spatial positioning (generally on the surface of the earth).  For example, the period "Révolution française" can be said to have taken place in “France”, the “Victorian” period, may be said to have taken place in “Britain” and its colonies, as well as other parts of Europe and north America.\r
A period can take place at multiple locations.\r
It is a shortcut of the more fully developed path from E4 Period through P161 has spatial projection, E53 Place, P89 falls within (contains) to E53 Place. \r
"""@en ;
    rdfs:domain cidoc_crm:E4_Period ;
    rdfs:range cidoc_crm:E53_Place .

cidoc_crm:P80_end_is_qualified_by a owl:DatatypeProperty ;
    rdfs:label "hat Begründung des Endes"@de,
        "τέλος προσδιορίζεται από"@el,
        "end is qualified by"@en,
        "fin est qualifiée par"@fr,
        "final é qualificado por"@pt,
        "конец ограничен"@ru,
        "终点认定的性质是"@zh ;
    rdfs:comment """This property qualifies the end of an E52 Time-Span in some way. \r
The nature of the qualification may be certainty, precision, source etc.\r
"""@en ;
    rdfs:domain cidoc_crm:E52_Time-Span ;
    rdfs:range rdfs:Literal ;
    rdfs:subPropertyOf cidoc_crm:P3_has_note .

cidoc_crm:P81a_end_of_the_begin a owl:DatatypeProperty ;
    rdfs:label "Ende des Anfangs"@de,
        "τέλος της αρχής"@el,
        "end of the begin"@en,
        "fin du début"@fr,
        "fim do início"@pt,
        "конец начала"@ru ;
    rdfs:comment "This is defined as the first boundary of the property P81"@en ;
    rdfs:domain cidoc_crm:E52_Time-Span ;
    rdfs:range xsd:dateTime ;
    rdfs:subPropertyOf cidoc_crm:P81_ongoing_throughout .

cidoc_crm:P81b_begin_of_the_end a owl:DatatypeProperty ;
    rdfs:label "Anfang vom Ende"@de,
        "αρχή του τέλους"@el,
        "begin of the end"@en,
        "début de la fin"@fr,
        "começar do fim"@pt,
        "начать в конце"@ru ;
    rdfs:comment "This is defined as the second boundary of the property P81"@en ;
    rdfs:domain cidoc_crm:E52_Time-Span ;
    rdfs:range xsd:dateTime ;
    rdfs:subPropertyOf cidoc_crm:P81_ongoing_throughout .

cidoc_crm:P82a_begin_of_the_begin a owl:DatatypeProperty ;
    rdfs:label "Anfang des Anfangs"@de,
        "αρχή της αρχής"@el,
        "begin of the begin"@en,
        "début du début"@fr,
        "começar do início"@pt,
        "начать с начала"@ru ;
    rdfs:comment "This is defined as the first boundary of the property P82"@en ;
    rdfs:domain cidoc_crm:E52_Time-Span ;
    rdfs:range xsd:dateTime ;
    rdfs:subPropertyOf cidoc_crm:P82_at_some_time_within .

cidoc_crm:P82b_end_of_the_end a owl:DatatypeProperty ;
    rdfs:label "Ende vom Ende"@de,
        "τέλος του τέλους"@el,
        "end of the end"@en,
        "fin de la fin"@fr,
        "fim do fim"@pt,
        "конец конец"@ru ;
    rdfs:comment "This is defined as the second boundary of the property P82"@en ;
    rdfs:domain cidoc_crm:E52_Time-Span ;
    rdfs:range xsd:dateTime ;
    rdfs:subPropertyOf cidoc_crm:P82_at_some_time_within .

cidoc_crm:P83_had_at_least_duration a owl:ObjectProperty ;
    rdfs:label "hatte Mindestdauer"@de,
        "είχε ελάχιστη διάρκεια"@el,
        "had at least duration"@en,
        "a duré au moins"@fr,
        "durou no mínimo"@pt,
        "имеет длительность по крайней мере больше чем"@ru,
        "时间最少持续了"@zh ;
    rdfs:comment """This property describes the minimum length of time covered by an E52 Time-Span. \r
It allows an E52 Time-Span to be associated with an E54 Dimension representing it’s minimum duration (i.e. it’s inner boundary) independent from the actual beginning and end.\r
"""@en ;
    rdfs:domain cidoc_crm:E52_Time-Span ;
    rdfs:range cidoc_crm:E54_Dimension .

cidoc_crm:P83i_was_minimum_duration_of a owl:ObjectProperty ;
    rdfs:label "war Mindestdauer von"@de,
        "είναι ελάχιστη διάρκεια του/της"@el,
        "was minimum duration of"@en,
        "a été la durée minimum de"@fr,
        "foi a duração mínima de"@pt,
        "был минимальной длительностью для"@ru ;
    rdfs:domain cidoc_crm:E54_Dimension ;
    rdfs:range cidoc_crm:E52_Time-Span .

cidoc_crm:P84_had_at_most_duration a owl:ObjectProperty ;
    rdfs:label "hatte Höchstdauer"@de,
        "είχε μέγιστη διάρκεια"@el,
        "had at most duration"@en,
        "a duré au plus"@fr,
        "durou no máximo"@pt,
        "имеет длительность меньше чем"@ru,
        "时间最多持续了"@zh ;
    rdfs:comment """This property describes the maximum length of time covered by an E52 Time-Span. \r
It allows an E52 Time-Span to be associated with an E54 Dimension representing it’s maximum duration (i.e. it’s outer boundary) independent from the actual beginning and end.\r
"""@en ;
    rdfs:domain cidoc_crm:E52_Time-Span ;
    rdfs:range cidoc_crm:E54_Dimension .

cidoc_crm:P84i_was_maximum_duration_of a owl:ObjectProperty ;
    rdfs:label "war längste Dauer von"@de,
        "είναι μέγιστη διάρκεια του/της"@el,
        "was maximum duration of"@en,
        "a été la durée maximum de"@fr,
        "foi a duração máxima de"@pt,
        "был максимальной длительностью для"@ru,
        ""@zh ;
    rdfs:domain cidoc_crm:E54_Dimension ;
    rdfs:range cidoc_crm:E52_Time-Span .

cidoc_crm:P86_falls_within a owl:ObjectProperty ;
    rdfs:label "fällt in"@de,
        "περιέχεται σε"@el,
        "falls within"@en,
        "s’insère dans"@fr,
        "está contido em"@pt,
        "содержится в"@ru,
        "时间上被涵盖於"@zh ;
    rdfs:comment """This property describes the inclusion relationship between two instances of E52 Time-Span.\r
This property supports the notion that a Time-Span’s temporal extent falls within the temporal extent of another Time-Span. It addresses temporal containment only, and no contextual link between the two instances of Time-Span is implied.\r
"""@en ;
    rdfs:domain cidoc_crm:E52_Time-Span ;
    rdfs:range cidoc_crm:E52_Time-Span .

cidoc_crm:P86i_contains a owl:ObjectProperty ;
    rdfs:label "enthält"@de,
        "περιέχει"@el,
        "contains"@en,
        "inclut"@fr,
        "contém"@pt,
        "содержит"@ru,
        "时间上涵盖了"@zh ;
    rdfs:domain cidoc_crm:E52_Time-Span ;
    rdfs:range cidoc_crm:E52_Time-Span .

cidoc_crm:P87_is_identified_by a owl:ObjectProperty ;
    rdfs:label "wird bezeichnet als"@de,
        "αναγνωρίζεται ως"@el,
        "is identified by"@en,
        "est identifié par"@fr,
        "é identificado por"@pt,
        "идентифицируется посредством"@ru,
        "有辨认码"@zh ;
    rdfs:comment """This property identifies an E53 Place using an E44 Place Appellation. \r
Examples of Place Appellations used to identify Places include instances of E48 Place Name, addresses, E47 Spatial Coordinates etc.\r
"""@en ;
    rdfs:domain cidoc_crm:E53_Place ;
    rdfs:range cidoc_crm:E44_Place_Appellation ;
    rdfs:subPropertyOf cidoc_crm:P1_is_identified_by .

cidoc_crm:P87i_identifies a owl:ObjectProperty ;
    rdfs:label "bezeichnet"@de,
        "είναι αναγνωριστικό"@el,
        "identifies"@en,
        "identifie"@fr,
        "identifica"@pt,
        "идентифицирует"@ru,
        "被用来辨认"@zh ;
    rdfs:domain cidoc_crm:E44_Place_Appellation ;
    rdfs:range cidoc_crm:E53_Place ;
    rdfs:subPropertyOf cidoc_crm:P1i_identifies .

cidoc_crm:P89_falls_within a owl:ObjectProperty ;
    rdfs:label "fällt in"@de,
        "περιέχεται σε"@el,
        "falls within"@en,
        "s’insère dans"@fr,
        "está contido em"@pt,
        "содержится в"@ru,
        "空间上被包围於"@zh ;
    rdfs:comment """This property identifies an instance of E53 Place that falls wholly within the extent of another E53 Place.\r
It addresses spatial containment only, and does not imply any relationship between things or phenomena occupying these places.\r
"""@en ;
    rdfs:domain cidoc_crm:E53_Place ;
    rdfs:range cidoc_crm:E53_Place .

cidoc_crm:P89i_contains a owl:ObjectProperty ;
    rdfs:label "enthält"@de,
        "περιέχει"@el,
        "contains"@en,
        "inclut"@fr,
        "contém"@pt,
        "содержит"@ru,
        "空间上包含了"@zh ;
    rdfs:domain cidoc_crm:E53_Place ;
    rdfs:range cidoc_crm:E53_Place .

cidoc_crm:P8_took_place_on_or_within a owl:ObjectProperty ;
    rdfs:label "fand statt auf oder innerhalb von "@de,
        "έλαβε χώρα σε ή εντός"@el,
        "took place on or within"@en,
        "a eu lieu sur ou dans"@fr,
        "ocorreu em ou dentro"@pt,
        "имел место на или в"@ru,
        "发生所在物件是"@zh ;
    rdfs:comment """This property describes the location of an instance of E4 Period with respect to an E19 Physical Object. \r
P8 took place on or within (witnessed) is a shortcut of the more fully developed path from E4 Period through P7 took place at, E53 Place, P156 occupies (is occupied by) to E18 Physical Thing.\r
\r
It describes a period that can be located with respect to the space defined by an E19 Physical Object such as a ship or a building. The precise geographical location of the object during the period in question may be unknown or unimportant. \r
For example, the French and German armistice of 22 June 1940 was signed in the same railway carriage as the armistice of 11 November 1918.\r
"""@en ;
    rdfs:domain cidoc_crm:E4_Period ;
    rdfs:range cidoc_crm:E18_Physical_Thing .

cidoc_crm:P8i_witnessed a owl:ObjectProperty ;
    rdfs:label "bezeugte"@de,
        "υπήρξε τόπος του"@el,
        "witnessed"@en,
        "a été témoin de"@fr,
        "testemunhou"@pt,
        "являлся местом для"@ru,
        "发生过"@zh ;
    rdfs:domain cidoc_crm:E18_Physical_Thing ;
    rdfs:range cidoc_crm:E4_Period .

cidoc_crm:P90_has_value a owl:DatatypeProperty ;
    rdfs:label "hat Wert"@de,
        "έχει τιμή"@el,
        "has value"@en,
        "a la valeur"@fr,
        "tem valor"@pt,
        "имеет значение"@ru,
        "有数值"@zh ;
    rdfs:comment "This property allows an E54 Dimension to be approximated by an E60 Number primitive."@en ;
    rdfs:domain cidoc_crm:E54_Dimension ;
    rdfs:range rdfs:Literal .

cidoc_crm:P91_has_unit a owl:ObjectProperty ;
    rdfs:label "hat Einheit"@de,
        "έχει μονάδα μέτρησης"@el,
        "has unit"@en,
        "a pour unité"@fr,
        "tem unidade"@pt,
        "имеет единицу"@ru,
        "有单位"@zh ;
    rdfs:comment "This property shows the type of unit an E54 Dimension was expressed in."@en ;
    rdfs:domain cidoc_crm:E54_Dimension ;
    rdfs:range cidoc_crm:E58_Measurement_Unit .

cidoc_crm:P91i_is_unit_of a owl:ObjectProperty ;
    rdfs:label "ist Einheit von"@de,
        "αποτελεί μονάδα μέτρησης του/της"@el,
        "is unit of"@en,
        "est l'unité de"@fr,
        "é unidade de"@pt,
        "является единицей для"@ru,
        "被当做单位来表示"@zh ;
    rdfs:domain cidoc_crm:E58_Measurement_Unit ;
    rdfs:range cidoc_crm:E54_Dimension .

cidoc_crm:P95_has_formed a owl:ObjectProperty ;
    rdfs:label "hat gebildet"@de,
        "σχημάτισε"@el,
        "has formed"@en,
        "a fondé"@fr,
        "formou"@pt,
        "сформировал"@ru,
        "组成了"@zh ;
    rdfs:comment "This property links the founding or E66 Formation for an E74 Group with the Group itself."@en ;
    rdfs:domain cidoc_crm:E66_Formation ;
    rdfs:range cidoc_crm:E74_Group ;
    rdfs:subPropertyOf cidoc_crm:P92_brought_into_existence .

cidoc_crm:P95i_was_formed_by a owl:ObjectProperty ;
    rdfs:label "wurde gebildet von"@de,
        "σχηματίστηκε από"@el,
        "was formed by"@en,
        "a été fondé par"@fr,
        "foi formado por"@pt,
        "была сформирована посредством"@ru,
        "被组成於"@zh ;
    rdfs:domain cidoc_crm:E74_Group ;
    rdfs:range cidoc_crm:E66_Formation ;
    rdfs:subPropertyOf cidoc_crm:P92i_was_brought_into_existence_by .

cidoc_crm:P96_by_mother a owl:ObjectProperty ;
    rdfs:label "durch Mutter"@de,
        "είχε μητέρα"@el,
        "by mother"@en,
        "de mère"@fr,
        "pela mãe"@pt,
        "посредством матери"@ru,
        "来自生母"@zh ;
    rdfs:comment """This property links an E67 Birth event to an E21 Person as a participant in the role of birth-giving mother.\r
\r
Note that biological fathers are not necessarily participants in the Birth (see P97 from father (was father for)). The Person being born is linked to the Birth with the property P98 brought into life (was born). This is not intended for use with general natural history material, only people. There is no explicit method for modelling conception and gestation except by using extensions. This is a sub-property of P11 had participant (participated in).\r
"""@en ;
    rdfs:domain cidoc_crm:E67_Birth ;
    rdfs:range cidoc_crm:E21_Person ;
    rdfs:subPropertyOf cidoc_crm:P11_had_participant .

cidoc_crm:P96i_gave_birth a owl:ObjectProperty ;
    rdfs:label "gebar"@de,
        "ήταν μητέρα του/της"@el,
        "gave birth"@en,
        "a donné naissance à"@fr,
        "deu nascimento"@pt,
        "дал рождение"@ru,
        "成为生母於"@zh ;
    rdfs:domain cidoc_crm:E21_Person ;
    rdfs:range cidoc_crm:E67_Birth ;
    rdfs:subPropertyOf cidoc_crm:P11i_participated_in .

cidoc_crm:P97_from_father a owl:ObjectProperty ;
    rdfs:label "gab Vaterschaft"@de,
        "είχε πατέρα"@el,
        "from father"@en,
        "de père"@fr,
        "pelo pai"@pt,
        "от отца"@ru,
        "来自父亲"@zh ;
    rdfs:comment """This property links an E67 Birth event to an E21 Person in the role of biological father.\r
Note that biological fathers are not seen as necessary participants in the Birth, whereas birth-giving mothers are (see P96 by mother (gave birth)). The Person being born is linked to the Birth with the property P98 brought into life (was born).\r
This is not intended for use with general natural history material, only people. There is no explicit method for modelling conception and gestation except by using extensions. \r
A Birth event is normally (but not always) associated with one biological father.\r
"""@en ;
    rdfs:domain cidoc_crm:E67_Birth ;
    rdfs:range cidoc_crm:E21_Person .

cidoc_crm:P97i_was_father_for a owl:ObjectProperty ;
    rdfs:label "war Vater für"@de,
        "ήταν πατέρας του/της"@el,
        "was father for"@en,
        "a été père dans"@fr,
        "foi pai para"@pt,
        "был отцом для"@ru,
        "成为生父於"@zh ;
    rdfs:domain cidoc_crm:E21_Person ;
    rdfs:range cidoc_crm:E67_Birth .

cidoc_crm:P98_brought_into_life a owl:ObjectProperty ;
    rdfs:label "brachte zur Welt"@de,
        "έφερε στη ζωή"@el,
        "brought into life"@en,
        "a donné vie à"@fr,
        "trouxe à vida"@pt,
        "породил"@ru,
        "诞生了"@zh ;
    rdfs:comment """This property links an E67Birth event to an E21 Person in the role of offspring.\r
Twins, triplets etc. are brought into life by the same Birth event. This is not intended for use with general Natural History material, only people. There is no explicit method for modelling conception and gestation except by using extensions.\r
"""@en ;
    rdfs:domain cidoc_crm:E67_Birth ;
    rdfs:range cidoc_crm:E21_Person ;
    rdfs:subPropertyOf cidoc_crm:P92_brought_into_existence .

cidoc_crm:P98i_was_born a owl:ObjectProperty ;
    rdfs:label "wurde geboren durch"@de,
        "γεννήθηκε"@el,
        "was born"@en,
        "est né"@fr,
        "veio à vida pelo"@pt,
        "был рожден"@ru,
        "诞生於"@zh ;
    rdfs:domain cidoc_crm:E21_Person ;
    rdfs:range cidoc_crm:E67_Birth ;
    rdfs:subPropertyOf cidoc_crm:P92i_was_brought_into_existence_by .

cidoc_crm:P99_dissolved a owl:ObjectProperty ;
    rdfs:label "löste auf"@de,
        "διέλυσε"@el,
        "dissolved"@en,
        "a dissous"@fr,
        "dissolveu"@pt,
        "распустил"@ru,
        "解散了"@zh ;
    rdfs:comment "This property links the disbanding or E68 Dissolution of an E74 Group to the Group itself."@en ;
    rdfs:domain cidoc_crm:E68_Dissolution ;
    rdfs:range cidoc_crm:E74_Group ;
    rdfs:subPropertyOf cidoc_crm:P11_had_participant,
        cidoc_crm:P93_took_out_of_existence .

cidoc_crm:P99i_was_dissolved_by a owl:ObjectProperty ;
    rdfs:label "wurde aufgelöst durch"@de,
        "διαλύθηκε από"@el,
        "was dissolved by"@en,
        "a été dissous par"@fr,
        "foi dissolvido por"@pt,
        "был распущен посредством"@ru,
        "被解散於"@zh ;
    rdfs:domain cidoc_crm:E74_Group ;
    rdfs:range cidoc_crm:E68_Dissolution ;
    rdfs:subPropertyOf cidoc_crm:P11i_participated_in,
        cidoc_crm:P93i_was_taken_out_of_existence_by .

cidoc_crm:P9_consists_of a owl:ObjectProperty ;
    rdfs:label "setzt sich zusammen aus"@de,
        "αποτελείται από"@el,
        "consists of"@en,
        "consiste en"@fr,
        "consiste de"@pt,
        "состоит из"@ru,
        "包含子时期"@zh ;
    rdfs:comment """This property associates an instance of E4 Period with another instance of E4 Period that is defined by a subset of the phenomena that define the former. Therefore the spacetime volume of the latter must fall within the spacetime volume of the former.\r
"""@en ;
    rdfs:domain cidoc_crm:E4_Period ;
    rdfs:range cidoc_crm:E4_Period ;
    rdfs:subPropertyOf cidoc_crm:P10i_contains .

cidoc_crm:P9i_forms_part_of a owl:ObjectProperty ;
    rdfs:label "bildet Teil von"@de,
        "αποτελεί μέρος του/της"@el,
        "forms part of"@en,
        "fait partie de"@fr,
        "faz parte de"@pt,
        "формирует часть"@ru,
        "附属於"@zh ;
    rdfs:domain cidoc_crm:E4_Period ;
    rdfs:range cidoc_crm:E4_Period ;
    rdfs:subPropertyOf cidoc_crm:P10_falls_within .

<https://purl.org/bdot10k#bdot10k_entity> rdfs:subClassOf cidoc_crm:E70_Thing .

<https://purl.org/urbanonto> a owl:Ontology ;
    owl:imports <https://purl.org/bdot10k>,
        <https://raw.githubusercontent.com/ontogeohist/ontology/master/ontohgis_pure.ttl> .

urbanonto:object_type_0 a owl:Class ;
    rdfs:label "Town"@en,
        "Miasto"@pl ;
    rdfs:comment "Przynamniej w okresie od XIII do XVIII w. funkcjonowały równolegle dwa pojęcia miasta: ogólne, obejmujące cały zespół osadniczy o odrębności społecznej, gospodarczej i urbanistycznej, postrzegane przede wszystkim intuicyjnie oraz miasto w sensie polityczno-prawnym, obdarzona względnie szeroką autonomią gmina. W konsekwencji mogły istnieć miasta w mieście i obiekty leżące jednocześnie w mieście i poza nim. Dla takich złożonych struktur w niniejszym projekcie należy się posługiwać pierwszym znaczeniem miasta."@en,
        "Przynamniej w okresie od XIII do XVIII w. funkcjonowały równolegle dwa pojęcia miasta: ogólne, obejmujące cały zespół osadniczy o odrębności społecznej, gospodarczej i urbanistycznej, postrzegane przede wszystkim intuicyjnie oraz miasto w sensie polityczno-prawnym, obdarzona względnie szeroką autonomią gmina. W konsekwencji mogły istnieć miasta w mieście i obiekty leżące jednocześnie w mieście i poza nim. Dla takich złożonych struktur w niniejszym projekcie należy się posługiwać pierwszym znaczeniem miasta."@pl ;
    rdfs:isDefinedBy "Miasto jest to miejscowość wyższego rzędu, odróżniająca się od otaczających je podstawowych wielkością (liczoną według miary właściwej dla danej epoki i regionu), stopniem złożoności i funkcjami centralnymi względem nich."@en,
        "Miasto jest to miejscowość wyższego rzędu, odróżniająca się od otaczających je podstawowych wielkością (liczoną według miary właściwej dla danej epoki i regionu), stopniem złożoności i funkcjami centralnymi względem nich."@pl ;
    rdfs:seeAlso """#EncPWN1962: "Skupisko ludności, odróżniające się od innych swymi głównie nierolniczymi funkcjami, znaczną wielkością oraz intensywnością zabudowy. Definicja ta musi być jednak interpretowana elastycznie i zawsze na tle aktualnej sieci osadniczej"(Wacław Ostrowski)
#SPXVIw, t. 13, s. 37: "Wytyczony i najczęściej otoczony murem teren, pokryty gęstą i planową zabudową tworzącą place i ulice, stanowiący mniej lub więcej samodzielną jednostkę administracyjną, samorządową, a czasem polityczną"
#Irsigler 2001, s. 63: "Miasto jest osadą różniącą się od wsi i nierolniczych osad monofunkcyjnych względną wielkością z zagęszczoną i rozczłonkowaną zabudową, z ludnością wyspecjalizowaną zawodowo i rozwarstwioną społecznie oraz funkcjami centralnymi pełnionymi wobec określonego regionu lub lokalnej ludności w sferze polityki, panowania, obronności, gospodarki, kultu i kultury" [Stadt ist eine vom Dorf und nichtagrarischen Einzwecksiedlungen unterschiedene Siedlung relativer Größe mit verdichteter, gegliederter Bebauung, beruflich spezialisierter und sozial geschichteter Bevölkerung und zentralen Funktionen politisch-herrschaftlich-militärischer, wirtschaftlicher und kultisch-kultureller Art für eine bestimmte Region oder regionale Bevölkerung.]
#wiki.ru: główny punkt osadniczy, którego mieszkańcy z reguły nie zajmują się rolnictwem; ma rozwiniętą gospodarkę, charakteryzuje się zagęszczeniem obiektów architektonicznych i inżynierskich zaspokajających potrzeby życiowe miejscowej ludności." [крупный населённый пункт, жители которого заняты, как правило, не сельским хозяйством. Имеет развитый комплекс хозяйства и экономики, является скоплением архитектурных и инженерных сооружений, обеспечивающих жизнеобеспечение населения.]
#wiki.fr: ośrodek materialny - ośrodek miejski - w którym koncentruje się znaczna ludność i gdzie przestrzeń jest ukształtowana celem ułatwienia i skoncentrowania jego aktywności: mieszkania, handlu, przemysłu, edukacji, polityki, dróg, transportu, kultury etc." [un milieu physique — le milieu urbain — où se concentre une forte population humaine, et dont l'espace est aménagé pour faciliter et concentrer ces activités : habitat, commerce, industrie, éducation, politique, voie de circulation, transports, culture, etc.]"""@en,
        """#EncPWN1962: "Skupisko ludności, odróżniające się od innych swymi głównie nierolniczymi funkcjami, znaczną wielkością oraz intensywnością zabudowy. Definicja ta musi być jednak interpretowana elastycznie i zawsze na tle aktualnej sieci osadniczej"(Wacław Ostrowski)
#SPXVIw, t. 13, s. 37: "Wytyczony i najczęściej otoczony murem teren, pokryty gęstą i planową zabudową tworzącą place i ulice, stanowiący mniej lub więcej samodzielną jednostkę administracyjną, samorządową, a czasem polityczną"
#Irsigler 2001, s. 63: "Miasto jest osadą różniącą się od wsi i nierolniczych osad monofunkcyjnych względną wielkością z zagęszczoną i rozczłonkowaną zabudową, z ludnością wyspecjalizowaną zawodowo i rozwarstwioną społecznie oraz funkcjami centralnymi pełnionymi wobec określonego regionu lub lokalnej ludności w sferze polityki, panowania, obronności, gospodarki, kultu i kultury" [Stadt ist eine vom Dorf und nichtagrarischen Einzwecksiedlungen unterschiedene Siedlung relativer Größe mit verdichteter, gegliederter Bebauung, beruflich spezialisierter und sozial geschichteter Bevölkerung und zentralen Funktionen politisch-herrschaftlich-militärischer, wirtschaftlicher und kultisch-kultureller Art für eine bestimmte Region oder regionale Bevölkerung.]
#wiki.ru: główny punkt osadniczy, którego mieszkańcy z reguły nie zajmują się rolnictwem; ma rozwiniętą gospodarkę, charakteryzuje się zagęszczeniem obiektów architektonicznych i inżynierskich zaspokajających potrzeby życiowe miejscowej ludności." [крупный населённый пункт, жители которого заняты, как правило, не сельским хозяйством. Имеет развитый комплекс хозяйства и экономики, является скоплением архитектурных и инженерных сооружений, обеспечивающих жизнеобеспечение населения.]
#wiki.fr: ośrodek materialny - ośrodek miejski - w którym koncentruje się znaczna ludność i gdzie przestrzeń jest ukształtowana celem ułatwienia i skoncentrowania jego aktywności: mieszkania, handlu, przemysłu, edukacji, polityki, dróg, transportu, kultury etc." [un milieu physique — le milieu urbain — où se concentre une forte population humaine, et dont l'espace est aménagé pour faciliter et concentrer ces activités : habitat, commerce, industrie, éducation, politique, voie de circulation, transports, culture, etc.]"""@pl,
        "https://www.wikidata.org/wiki/Q515"^^xsd:url ;
    rdfs:subClassOf <https://purl.org/bdot10k#class_29> ;
    ns1:altLabel "Stadt"@de,
        "city"@en,
        "town"@en,
        "cité"@fr,
        "ville"@fr,
        "civitas"@la,
        "oppidum"@la,
        "miasteczko"@pl,
        "gorod"@ru ;
    ns1:hiddenLabel "aglomeracja"@en,
        "miasteczko"@en,
        "osada miejska"@en,
        "aglomeracja"@pl,
        "miasteczko"@pl,
        "osada miejska"@pl .

urbanonto:object_type_1 a owl:Class ;
    rdfs:label "Urban plot"@en,
        "Działka miejska"@pl ;
    rdfs:comment "Działki różnią się pod względem wielkości. Mają różne typy zabudowy lub brak zabudowy. Pełnią różne funkcje."@en,
        "Działki różnią się pod względem wielkości. Mają różne typy zabudowy lub brak zabudowy. Pełnią różne funkcje."@pl ;
    rdfs:isDefinedBy "Jest to część terenu miasta oddzielona od innych na podstawie własności lub pełnionej funkcji. Granica działki widoczna jest w terenie lub w rejestrach własności lub w materiale kartograficznym."@en,
        "Jest to część terenu miasta oddzielona od innych na podstawie własności lub pełnionej funkcji. Granica działki widoczna jest w terenie lub w rejestrach własności lub w materiale kartograficznym."@pl ;
    ns1:altLabel "Stadtgrundstück"@de,
        "urban plot"@en,
        "parcela"@pl .

urbanonto:object_type_2 a owl:Class ;
    rdfs:label "Street"@en,
        "Ulica"@pl ;
    rdfs:comment "Ulice różnią się pod wzgledem długości i szerokości. Mają różne typy nawierzchni. Mogą być wykorzystywane jak plac lub targowisko."@en,
        "Ulice różnią się pod wzgledem długości i szerokości. Mają różne typy nawierzchni. Mogą być wykorzystywane jak plac lub targowisko."@pl ;
    rdfs:isDefinedBy "Jest to droga lub część drogi w terenie zabudowanym, do której budynki, budowle, urządzenia lub inne obiekty przylegają lub nie. "@en,
        "Jest to droga lub część drogi w terenie zabudowanym, do której budynki, budowle, urządzenia lub inne obiekty przylegają lub nie. "@pl ;
    rdfs:seeAlso "USTAWA z dnia 21 marca 1985 r. o drogach publicznych: Art. 4 [Słowniczek] Użyte w ustawie określenia oznaczają [...] 3)  ulica - drogę na terenie zabudowy lub przeznaczonym do zabudowy zgodnie z przepisami o planowaniu i zagospodarowaniu przestrzennym, w której ciągu może być zlokalizowane torowisko tramwajowe."@en,
        "USTAWA z dnia 21 marca 1985 r. o drogach publicznych: Art. 4 [Słowniczek] Użyte w ustawie określenia oznaczają [...] 3)  ulica - drogę na terenie zabudowy lub przeznaczonym do zabudowy zgodnie z przepisami o planowaniu i zagospodarowaniu przestrzennym, w której ciągu może być zlokalizowane torowisko tramwajowe."@pl,
        "https://www.wikidata.org/wiki/Q79007"^^xsd:url ;
    rdfs:subClassOf <https://purl.org/bdot10k#class_5> ;
    ns1:altLabel "Strasse"@de,
        "street"@en,
        "rue"@fr,
        "via"@la,
        "ulitsa"@ru ;
    ns1:hiddenLabel "aleja"@en,
        "bulwar"@en,
        "droga"@en,
        "jezdnia"@en,
        "pasaż"@en,
        "trakt"@en,
        "uliczka"@en,
        "zaułek"@en,
        "ścieżka"@en,
        "aleja"@pl,
        "bulwar"@pl,
        "droga"@pl,
        "jezdnia"@pl,
        "pasaż"@pl,
        "trakt"@pl,
        "uliczka"@pl,
        "zaułek"@pl,
        "ścieżka"@pl .

urbanonto:object_type_3 a owl:Class ;
    rdfs:label "School"@en,
        "Szkoła"@pl ;
    rdfs:comment "Szkoły publiczne istnieją przez cały okres XIX w., ich istnienie reguluje ustawodawstwo, które mówi o ich tworzeniu, normach, jakie powinny spełniać, o ich rodzajach i stopniach. Ich liczba jest dużo niższa od prywatnych. Szkoły prywatne istnieją także przez cały okres, wpierw głównie jako szkoły wyznaniowe (które potem włączane w sieć placówek publicznych utrzymywanych przez państwo), potem rośnie liczba laickich szkół prywatnych, których właściciele wynajmują przestrzeń w kamienicach czynszowych na cele szkolne."@en,
        "Szkoły publiczne istnieją przez cały okres XIX w., ich istnienie reguluje ustawodawstwo, które mówi o ich tworzeniu, normach, jakie powinny spełniać, o ich rodzajach i stopniach. Ich liczba jest dużo niższa od prywatnych. Szkoły prywatne istnieją także przez cały okres, wpierw głównie jako szkoły wyznaniowe (które potem włączane w sieć placówek publicznych utrzymywanych przez państwo), potem rośnie liczba laickich szkół prywatnych, których właściciele wynajmują przestrzeń w kamienicach czynszowych na cele szkolne."@pl ;
    rdfs:isDefinedBy "Jest to budynek mieszczący instytucję wychowawczo-edukacyjną."@en,
        "Jest to budynek mieszczący instytucję wychowawczo-edukacyjną."@pl ;
    rdfs:seeAlso "https://www.wikidata.org/wiki/Q3914"^^xsd:url ;
    rdfs:subClassOf <https://purl.org/bdot10k#object_120> ;
    ns1:altLabel "Lehranstalt"@de,
        "Schule"@de,
        "school"@en,
        "école"@fr,
        "scholae"@la,
        "ucziliszcze"@ru ;
    ns1:hiddenLabel "szkoła wyższa"@en,
        "uniwersytet"@en,
        "szkoła wyższa"@pl,
        "uniwersytet"@pl .

urbanonto:object_type_4 a owl:Class ;
    rdfs:label "kompleks szkolny"@en,
        "Kompleks szkolny"@pl ;
    rdfs:comment "Szkoły publiczne istnieją przez cały okres XIX w., ich istnienie reguluje ustawodawstwo, które mówi o ich tworzeniu, normach, jakie powinny spełniać, o ich rodzajach i stopniach. Ich liczba jest dużo niższa od prywatnych. Szkoły prywatne istnieją także przez cały okres, wpierw głównie jako szkoły wyznaniowe (które potem włączane w sieć placówek publicznych utrzymywanych przez państwo), potem rośnie liczba laickich szkół prywatnych, których właściciele wynajmują przestrzeń w kamienicach czynszowych na cele szkolne."@en,
        "Szkoły publiczne istnieją przez cały okres XIX w., ich istnienie reguluje ustawodawstwo, które mówi o ich tworzeniu, normach, jakie powinny spełniać, o ich rodzajach i stopniach. Ich liczba jest dużo niższa od prywatnych. Szkoły prywatne istnieją także przez cały okres, wpierw głównie jako szkoły wyznaniowe (które potem włączane w sieć placówek publicznych utrzymywanych przez państwo), potem rośnie liczba laickich szkół prywatnych, których właściciele wynajmują przestrzeń w kamienicach czynszowych na cele szkolne."@pl ;
    rdfs:isDefinedBy "Jest to kompleks budynków i obiektów użytkowania terenu mieszczący instytucję wychowawczo-edukacyjną."@en,
        "Jest to kompleks budynków i obiektów użytkowania terenu mieszczący instytucję wychowawczo-edukacyjną."@pl ;
    rdfs:seeAlso "https://www.wikidata.org/wiki/Q3914"^^xsd:url ;
    rdfs:subClassOf <https://purl.org/bdot10k#class_48> ;
    ns1:altLabel "Lehranstalt"@de,
        "Schule"@de,
        "school"@en,
        "école"@fr,
        "scholae"@la,
        "kompleks oświatowy"@pl,
        "ucziliszcze"@ru ;
    ns1:hiddenLabel "ochronka"@en,
        "przedszkole"@en,
        "szkoła wyższa"@en,
        "uniwersytet"@en,
        "zespół szkół"@en,
        "ochronka"@pl,
        "przedszkole"@pl,
        "szkoła wyższa"@pl,
        "uniwersytet"@pl,
        "zespół szkół"@pl .

urbanonto:object_type_5 a owl:Class ;
    rdfs:label "Chapel"@en,
        "Kaplica wolnostojąca"@pl ;
    rdfs:comment "Kaplice wolnostrojące są widoczne na planach miast, w przestrzeni miejskiej wyróżnia je forma architektoniczna charakterystyczna dla budynków sakralnych."@en,
        "Kaplice wolnostrojące są widoczne na planach miast, w przestrzeni miejskiej wyróżnia je forma architektoniczna charakterystyczna dla budynków sakralnych."@pl ;
    rdfs:isDefinedBy "Jest to niewielka chrześcijańska budowla sakralna służąca do odprawiania kultu (np. celebracja mszy, modlitwa) lub będąca (rzadko) miejscem pochówku, zawierająca ołtarz lub ołtarze."@en,
        "Jest to niewielka chrześcijańska budowla sakralna służąca do odprawiania kultu (np. celebracja mszy, modlitwa) lub będąca (rzadko) miejscem pochówku, zawierająca ołtarz lub ołtarze."@pl ;
    rdfs:seeAlso """#SJP PWN on-line: 1.  niewielka budowla sakralna; 
#Słownik języka polskiego pod red. W. Doroszewskiego: mały kościółek; boczna część kościoła mająca ołtarz i tworząca oddzielną całość; oddzielny pokój z ołtarzem do odprawiania nabożeństwa; 
#Encyklopedia PWN on-line: kaplica [czes. < łac.], arch. niewielka budowla sakralna, wolno stojąca lub połączona z większym kompleksem architektonicznym (głównie kościołem), bądź też wydzielone pomieszczenie z ołtarzem, stanowiące część większej budowli; 
#Prawo kanoniczne (katolicyzm): Kan. 1223 – Przez kaplicę rozumie się miejsce przeznaczone, za zezwoleniem ordynariusza, do sprawowania kultu Bożego, dla pożytku jakiejś wspólnoty lub grupy wiernych, którzy się w nim zbierają, do którego za zgodą kompetentnego przełożonego mogą przychodzić także inni wierni."""@en,
        """#SJP PWN on-line: 1.  niewielka budowla sakralna; 
#Słownik języka polskiego pod red. W. Doroszewskiego: mały kościółek; boczna część kościoła mająca ołtarz i tworząca oddzielną całość; oddzielny pokój z ołtarzem do odprawiania nabożeństwa; 
#Encyklopedia PWN on-line: kaplica [czes. < łac.], arch. niewielka budowla sakralna, wolno stojąca lub połączona z większym kompleksem architektonicznym (głównie kościołem), bądź też wydzielone pomieszczenie z ołtarzem, stanowiące część większej budowli; 
#Prawo kanoniczne (katolicyzm): Kan. 1223 – Przez kaplicę rozumie się miejsce przeznaczone, za zezwoleniem ordynariusza, do sprawowania kultu Bożego, dla pożytku jakiejś wspólnoty lub grupy wiernych, którzy się w nim zbierają, do którego za zgodą kompetentnego przełożonego mogą przychodzić także inni wierni."""@pl,
        "https://www.wikidata.org/wiki/Q108325"^^xsd:url ;
    rdfs:subClassOf <https://purl.org/bdot10k#class_30> ;
    ns1:altLabel "Kapelle"@de,
        "chapel"@en,
        "capella"@la,
        "oratorium"@la,
        "kaplica"@pl,
        "kapliczka"@pl ;
    ns1:hiddenLabel "kapliczka"@en,
        "kościół"@en,
        "kościółek"@en,
        "świątynia"@en,
        "kapliczka"@pl,
        "kościół"@pl,
        "kościółek"@pl,
        "świątynia"@pl .

cidoc_crm:E20_Biological_Object a owl:Class ;
    rdfs:label "Biologischer Gegenstand"@de,
        "Βιολογικό Ακτικείμενο"@el,
        "Biological Object"@en,
        "Objet biologique"@fr,
        "Objeto Biológico"@pt,
        "Биологический Объект"@ru,
        "生物体"@zh ;
    rdfs:comment """This class comprises individual items of a material nature, which live, have lived or are natural products of or from living organisms. \r
Artificial objects that incorporate biological elements, such as Victorian butterfly frames, can be documented as both instances of E20 Biological Object and E22 Man-Made Object. \r
"""@en ;
    rdfs:subClassOf cidoc_crm:E19_Physical_Object .

cidoc_crm:E37_Mark a owl:Class ;
    rdfs:label "Marke"@de,
        "Σήμανση"@el,
        "Mark"@en,
        "Marque"@fr,
        "Marca"@pt,
        "Пометка"@ru,
        "标志"@zh ;
    rdfs:comment """This class comprises symbols, signs, signatures or short texts applied to instances of E24 Physical Man-Made Thing by arbitrary techniques in order to indicate the creator, owner, dedications, purpose, etc. \r
This class specifically excludes features that have no semantic significance, such as scratches or tool marks. These should be documented as instances of E25 Man-Made Feature. \r
"""@en ;
    rdfs:subClassOf cidoc_crm:E36_Visual_Item .

cidoc_crm:E48_Place_Name a owl:Class ;
    rdfs:label "Orts- oder Flurname"@de,
        "Τοπωνύμιο"@el,
        "Place Name"@en,
        "Toponyme"@fr,
        "Nome de Local"@pt,
        "Название Места"@ru,
        "地名"@zh ;
    rdfs:comment """This class comprises particular and common forms of E44 Place Appellation. \r
Place Names may change their application over time: the name of an E53 Place may change, and a name may be reused for a different E53 Place. Instances of E48 Place Name are typically subject to place name gazetteers."""@en ;
    rdfs:subClassOf cidoc_crm:E44_Place_Appellation .

cidoc_crm:P105_right_held_by a owl:ObjectProperty ;
    rdfs:label "Rechte stehen zu"@de,
        "δικαίωμα κατέχεται από"@el,
        "right held by"@en,
        "droit détenu par"@fr,
        "são direitos de "@pt,
        "право принадлежит"@ru,
        "有权限持有者"@zh ;
    rdfs:comment """This property identifies the E39 Actor who holds the instances of E30 Right to an E72 Legal Object.\r
	It is a superproperty of P52 has current owner (is current owner of) because ownership is a right that is held on the owned object.\r
P105 right held by (has right on) is a shortcut of the fully developed path from E72 Legal Object through P104 is subject to (applies to), E30 Right, P75 possesses (is possessed by) to E39 Actor.\r
"""@en ;
    rdfs:domain cidoc_crm:E72_Legal_Object ;
    rdfs:range cidoc_crm:E39_Actor .

cidoc_crm:P105i_has_right_on a owl:ObjectProperty ;
    rdfs:label "hat Rechte an"@de,
        "έχει δικαίωμα σε"@el,
        "has right on"@en,
        "détient un droit sur"@fr,
        "possui direitos sobre"@pt,
        "владеет правом на"@ru,
        "持有权限来管制"@zh ;
    rdfs:domain cidoc_crm:E39_Actor ;
    rdfs:range cidoc_crm:E72_Legal_Object .

cidoc_crm:P106_is_composed_of a owl:ObjectProperty ;
    rdfs:label " ist zusammengesetzt aus"@de,
        "αποτελείται από"@el,
        "is composed of"@en,
        "est composé de"@fr,
        "é composto de"@pt,
        "составлен из"@ru,
        "有组成元素"@zh ;
    rdfs:comment """This property associates an instance of E90 Symbolic Object with a part of it that is by itself an instance of E90 Symbolic Object, such as fragments of texts or clippings from an image.\r
"""@en ;
    rdfs:domain cidoc_crm:E90_Symbolic_Object ;
    rdfs:range cidoc_crm:E90_Symbolic_Object .

cidoc_crm:P106i_forms_part_of a owl:ObjectProperty ;
    rdfs:label "bildet Teil von"@de,
        "αποτελεί μέρος του/της"@el,
        "forms part of"@en,
        "fait partie de"@fr,
        "faz parte de"@pt,
        "формирует часть"@ru,
        "组成了"@zh ;
    rdfs:domain cidoc_crm:E90_Symbolic_Object ;
    rdfs:range cidoc_crm:E90_Symbolic_Object .

cidoc_crm:P10_falls_within a owl:ObjectProperty ;
    rdfs:label "fällt in"@de,
        "εμπίπτει"@el,
        "falls within"@en,
        "s’insère dans le cours de"@fr,
        "está contido em"@pt,
        "находится в пределах"@ru,
        "发生时间涵盖於"@zh ;
    rdfs:comment """This property associates an instance of E92 Spacetime Volume with another instance of E92 Spacetime Volume that falls within the latter. In other words, all points in the former are also points in the latter.\r
"""@en ;
    rdfs:domain cidoc_crm:E92_Spacetime_Volume ;
    rdfs:range cidoc_crm:E92_Spacetime_Volume .

cidoc_crm:P10i_contains a owl:ObjectProperty ;
    rdfs:label "enthält"@de,
        "περιλαμβάνει"@el,
        "contains"@en,
        "contient"@fr,
        "contém"@pt,
        "содержит"@ru,
        "时间上涵盖"@zh ;
    rdfs:domain cidoc_crm:E92_Spacetime_Volume ;
    rdfs:range cidoc_crm:E92_Spacetime_Volume .

cidoc_crm:P125_used_object_of_type a owl:ObjectProperty ;
    rdfs:label "benutzte Objekt des Typus"@de,
        "χρησιμοποίησε αντικείμενο τύπου"@el,
        "used object of type"@en,
        "a employé un objet du type"@fr,
        "usou objeto do tipo"@pt,
        "использовал объект типа"@ru,
        "有使用物件类型"@zh ;
    rdfs:comment """This property defines the kind of objects used in an E7 Activity, when the specific instance is either unknown or not of interest, such as use of "a hammer".\r
"""@en ;
    rdfs:domain cidoc_crm:E7_Activity ;
    rdfs:range cidoc_crm:E55_Type .

cidoc_crm:P125i_was_type_of_object_used_in a owl:ObjectProperty ;
    rdfs:label "Objekt des Typus ... wurde benutzt in"@de,
        "ήταν o τύπος αντικείμενου που χρησιμοποιήθηκε σε"@el,
        "was type of object used in"@en,
        "était le type d’objet employé par"@fr,
        "foi tipo do objeto usado em"@pt,
        "был типом объекта использованного в"@ru,
        "被使用於"@zh ;
    rdfs:domain cidoc_crm:E55_Type ;
    rdfs:range cidoc_crm:E7_Activity .

cidoc_crm:P128_carries a owl:ObjectProperty ;
    rdfs:label "trägt"@de,
        "φέρει"@el,
        "carries"@en,
        "est le support de"@fr,
        "é o suporte de"@pt,
        "несет"@ru,
        "承载信息"@zh ;
    rdfs:comment """This property identifies an E90 Symbolic Object carried by an instance of E18 Physical Thing.\r
"""@en ;
    rdfs:domain cidoc_crm:E18_Physical_Thing ;
    rdfs:range cidoc_crm:E90_Symbolic_Object ;
    rdfs:subPropertyOf cidoc_crm:P130_shows_features_of .

cidoc_crm:P128i_is_carried_by a owl:ObjectProperty ;
    rdfs:label "wird getragen von"@de,
        "φέρεται από"@el,
        "is carried by"@en,
        "a pour support"@fr,
        "é suportado por"@pt,
        "переносится посредством"@ru,
        "被承载于"@zh ;
    rdfs:domain cidoc_crm:E90_Symbolic_Object ;
    rdfs:range cidoc_crm:E18_Physical_Thing ;
    rdfs:subPropertyOf cidoc_crm:P130i_features_are_also_found_on .

cidoc_crm:P160_has_temporal_projection a owl:ObjectProperty ;
    rdfs:label "has temporal projection"@en ;
    rdfs:comment """This property describes the temporal projection of an instance of an E92 Spacetime Volume. The property P4 has time-span is the same as P160 has temporal projection if it is used to document an instance of E4 Period or any subclass of it. \r
	"""@en ;
    rdfs:domain cidoc_crm:E92_Spacetime_Volume ;
    rdfs:range cidoc_crm:E52_Time-Span .

cidoc_crm:P160i_is_temporal_projection_of a owl:ObjectProperty ;
    rdfs:label "is temporal projection of"@en ;
    rdfs:domain cidoc_crm:E52_Time-Span ;
    rdfs:range cidoc_crm:E92_Spacetime_Volume .

cidoc_crm:P161_has_spatial_projection a owl:ObjectProperty ;
    rdfs:label "has spatial projection"@en ;
    rdfs:comment """This property associates an instance of a E92 Spacetime Volume with an instance of E53 Place that is the result of the spatial projection of the instance of a E92 Spacetime Volume on a reference space. In general there can be more than one useful reference space to describe the spatial projection of a spacetime volume, such as that of a battle ship versus that of the seafloor. Therefore the projection is not unique.\r
This is part of the fully developed path that is shortcut by P7took place at (witnessed).The more fully developed path from E4 Period through P161 has spatial projection, E53 Place, P89 falls within (contains) to E53 Place. \r
	"""@en ;
    rdfs:domain cidoc_crm:E92_Spacetime_Volume ;
    rdfs:range cidoc_crm:E53_Place .

cidoc_crm:P161i_is_spatial_projection_of a owl:ObjectProperty ;
    rdfs:label "is spatial projection of"@en ;
    rdfs:domain cidoc_crm:E53_Place ;
    rdfs:range cidoc_crm:E92_Spacetime_Volume .

cidoc_crm:P2_has_type a owl:ObjectProperty ;
    rdfs:label "hat den Typus"@de,
        "έχει τύπο"@el,
        "has type"@en,
        "est de type"@fr,
        "é do tipo"@pt,
        "имеет тип"@ru,
        "有类型"@zh ;
    rdfs:comment """This property allows sub typing of CRM entities - a form of specialisation – through the use of a terminological hierarchy, or thesaurus. \r
The CRM is intended to focus on the high-level entities and relationships needed to describe data structures. Consequently, it does not specialise entities any further than is required for this immediate purpose. However, entities in the isA hierarchy of the CRM may by specialised into any number of sub entities, which can be defined in the E55 Type hierarchy. E51 Contact Point, for example, may be specialised into “e-mail address”, “telephone number”, “post office box”, “URL” etc. none of which figures explicitly in the CRM hierarchy. Sub typing obviously requires consistency between the meaning of the terms assigned and the more general intent of the CRM entity in question.\r
"""@en ;
    rdfs:domain cidoc_crm:E1_CRM_Entity ;
    rdfs:range cidoc_crm:E55_Type .

cidoc_crm:P2i_is_type_of a owl:ObjectProperty ;
    rdfs:label "ist Typus von"@de,
        "είναι ο τύπος του/της"@el,
        "is type of"@en,
        "est le type de"@fr,
        "é o tipo de"@pt,
        "является типом для"@ru,
        "被用来分类"@zh ;
    rdfs:domain cidoc_crm:E55_Type ;
    rdfs:range cidoc_crm:E1_CRM_Entity .

cidoc_crm:P46_is_composed_of a owl:ObjectProperty ;
    rdfs:label "ist zusammengesetzt aus"@de,
        "αποτελείται από"@el,
        "is composed of"@en,
        "est composée de"@fr,
        "é composto de"@pt,
        "составлен из"@ru,
        "有组件"@zh ;
    rdfs:comment """This property allows instances of E18 Physical Thing to be analysed into component elements.\r
\r
Component elements, since they are themselves instances of E18 Physical Thing, may be further analysed into sub-components, thereby creating a hierarchy of part decomposition. An instance of E18 Physical Thing may be shared between multiple wholes, for example two buildings may share a common wall. This property does not specify when and for how long a component element resided in the respective whole. If  a component is not part of a whole from the beginning of existence or until the end of existence of the whole, the classes E79 Part Addition and E90 Part Removal can be used to document when a component became part of a particular whole and/or when it stopped being a part of it. For the time-span of being part of the respective whole, the component is completely contained in the place the whole occupies.\r
\r
This property is intended to describe specific components that are individually documented, rather than general aspects. Overall descriptions of the structure of an instance of E18 Physical Thing are captured by the P3 has note property.\r
\r
The instances of E57 Material of which an item of E18 Physical Thing is composed should be documented using P45 consists of (is incorporated in).\r
"""@en ;
    rdfs:domain cidoc_crm:E18_Physical_Thing ;
    rdfs:range cidoc_crm:E18_Physical_Thing .

cidoc_crm:P46i_forms_part_of a owl:ObjectProperty ;
    rdfs:label "bildet Teil von"@de,
        "αποτελεί μέρος του/της"@el,
        "forms part of"@en,
        "fait partie de"@fr,
        "faz parte de"@pt,
        "формирует часть"@ru,
        "被用来组成"@zh ;
    rdfs:domain cidoc_crm:E18_Physical_Thing ;
    rdfs:range cidoc_crm:E18_Physical_Thing .

cidoc_crm:P51_has_former_or_current_owner a owl:ObjectProperty ;
    rdfs:label "hat früheren oder derzeitigen Besitzer "@de,
        "έχει ή είχε ιδιοκτήτη"@el,
        "has former or current owner"@en,
        "est ou a été possédée par"@fr,
        "é ou foi propriedade de"@pt,
        "имеет бывшего или текущего владельца"@ru,
        "有前任或现任物主"@zh ;
    rdfs:comment """This property identifies the E39 Actor that is or has been the legal owner (i.e. title holder) of an instance of E18 Physical Thing at some time.\r
The distinction with P52 has current owner (is current owner of) is that P51 has former or current owner (is former or current owner of) does not indicate whether the specified owners are current. P51 has former or current owner (is former or current owner of) is a shortcut for the more detailed path from E18 Physical Thing through P24 transferred title of (changed ownership through), E8 Acquisition, P23 transferred title from (surrendered title through), or P22 transferred title to (acquired title through) to E39 Actor.\r
"""@en ;
    rdfs:domain cidoc_crm:E18_Physical_Thing ;
    rdfs:range cidoc_crm:E39_Actor .

cidoc_crm:P51i_is_former_or_current_owner_of a owl:ObjectProperty ;
    rdfs:label "ist früherer oder derzeitiger Besitzer von"@de,
        "είναι ή ήταν ιδιοκτήτης του/της"@el,
        "is former or current owner of"@en,
        "est ou a été propriétaire de"@fr,
        "é ou foi proprietário de"@pt,
        "является бывшим или текущим владельцем для"@ru,
        "目前或曾经拥有"@zh ;
    rdfs:domain cidoc_crm:E39_Actor ;
    rdfs:range cidoc_crm:E18_Physical_Thing .

cidoc_crm:P53_has_former_or_current_location a owl:ObjectProperty ;
    rdfs:label "hat früheren oder derzeitigen Standort"@de,
        "βρίσκεται ή βρισκόταν σε"@el,
        "has former or current location"@en,
        "a ou a eu pour localisation"@fr,
        "é ou foi localizada em"@pt,
        "имеет текущее или бывшее местоположение"@ru,
        "目前或曾经被置放於"@zh ;
    rdfs:comment """This property allows an instance of E53 Place to be associated as the former or current location of an instance of E18 Physical Thing.\r
In the case of E19 Physical Objects, the property does not allow any indication of the Time-Span during which the Physical Object was located at this Place, nor if this is the current location.\r
In the case of immobile objects, the Place would normally correspond to the Place of creation.\r
P53 has former or current location (is former or current location of) is a shortcut. A more detailed representation can make use of the fully developed (i.e. indirect) path from E19 Physical Object through P25 moved (moved by), E9 Move, P26 moved to (was destination of) or P27 moved from (was origin of) to E53 Place.\r
"""@en ;
    rdfs:domain cidoc_crm:E18_Physical_Thing ;
    rdfs:range cidoc_crm:E53_Place .

cidoc_crm:P53i_is_former_or_current_location_of a owl:ObjectProperty ;
    rdfs:label "ist früherer oder derzeitiger Standort von"@de,
        "είναι ή ήταν θέση του"@el,
        "is former or current location of"@en,
        "est ou a été localisation de"@fr,
        "é ou foi localização de"@pt,
        "является текущим или бывшим местоположением для"@ru,
        "目前或曾经被置放了"@zh ;
    rdfs:domain cidoc_crm:E53_Place ;
    rdfs:range cidoc_crm:E18_Physical_Thing .

cidoc_crm:P59_has_section a owl:ObjectProperty ;
    rdfs:label "hat Bereich"@de,
        "έχει τομέα"@el,
        "has section"@en,
        "a pour section"@fr,
        "tem seção"@pt,
        "имеет район"@ru,
        "有区域"@zh ;
    rdfs:comment """This property links an area to the instance of E18 Physical Thing upon which it is found.\r
It is typically used when a named E46 Section Definition is not appropriate.\r
E18 Physical Thing may be subdivided into arbitrary regions. \r
P59 has section (is located on or within) is a shortcut. If the E53 Place is identified by a Section Definition, a more detailed representation can make use of the fully developed (i.e. indirect) path from E18 Physical Thing through P58 has section definition (defines section), E46 Section Definition, P87 is identified by (identifies) to E53 Place. A Place can only be located on or within one Physical Object.\r
"""@en ;
    rdfs:domain cidoc_crm:E18_Physical_Thing ;
    rdfs:range cidoc_crm:E53_Place .

cidoc_crm:P59i_is_located_on_or_within a owl:ObjectProperty ;
    rdfs:label "befindet sich auf oder in"@de,
        "βρίσκεται σε ή εντός"@el,
        "is located on or within"@en,
        "se situe sur ou dans"@fr,
        "está localizada sobre ou dentro de"@pt,
        "находится на или внутри"@ru,
        "位於"@zh ;
    rdfs:domain cidoc_crm:E53_Place ;
    rdfs:range cidoc_crm:E18_Physical_Thing .

cidoc_crm:P94_has_created a owl:ObjectProperty ;
    rdfs:label "hat erschaffen"@de,
        "δημιούργησε"@el,
        "has created"@en,
        "a créé"@fr,
        "criou"@pt,
        "создал"@ru,
        "创造了"@zh ;
    rdfs:comment """This property allows a conceptual E65 Creation to be linked to the E28 Conceptual Object created by it. \r
It represents the act of conceiving the intellectual content of the E28 Conceptual Object. It does not represent the act of creating the first physical carrier of the E28 Conceptual Object. As an example, this is the composition of a poem, not its commitment to paper.\r
"""@en ;
    rdfs:domain cidoc_crm:E65_Creation ;
    rdfs:range cidoc_crm:E28_Conceptual_Object ;
    rdfs:subPropertyOf cidoc_crm:P92_brought_into_existence .

cidoc_crm:P94i_was_created_by a owl:ObjectProperty ;
    rdfs:label "wurde erschaffen durch"@de,
        "δημιουργήθηκε από"@el,
        "was created by"@en,
        "a été créé par"@fr,
        "foi criado por"@pt,
        "был создан посредством"@ru,
        "被创造於"@zh ;
    rdfs:domain cidoc_crm:E28_Conceptual_Object ;
    rdfs:range cidoc_crm:E65_Creation ;
    rdfs:subPropertyOf cidoc_crm:P92i_was_brought_into_existence_by .

cidoc_crm:E12_Production a owl:Class ;
    rdfs:label "Herstellung"@de,
        "Παραγωγή"@el,
        "Production"@en,
        "Production"@fr,
        "Produção"@pt,
        "Событие Производства"@ru,
        "生产"@zh ;
    rdfs:comment """This class comprises activities that are designed to, and succeed in, creating one or more new items. \r
It specializes the notion of modification into production. The decision as to whether or not an object is regarded as new is context sensitive. Normally, items are considered “new” if there is no obvious overall similarity between them and the consumed items and material used in their production. In other cases, an item is considered “new” because it becomes relevant to documentation by a modification. For example, the scribbling of a name on a potsherd may make it a voting token. The original potsherd may not be worth documenting, in contrast to the inscribed one. \r
This entity can be collective: the printing of a thousand books, for example, would normally be considered a single event. \r
An event should also be documented using E81 Transformation if it results in the destruction of one or more objects and the simultaneous production of others using parts or material from the originals. In this case, the new items have separate identities and matter is preserved, but identity is not.\r
"""@en ;
    rdfs:subClassOf cidoc_crm:E11_Modification,
        cidoc_crm:E63_Beginning_of_Existence .

cidoc_crm:E25_Man-Made_Feature a owl:Class ;
    rdfs:label "Hergestelltes Merkmal"@de,
        "Ανθρωπογενές Μόρφωμα"@el,
        "Man-Made Feature"@en,
        "Caractéristique fabriquée"@fr,
        "Característica Fabricada"@pt,
        "Искусственный Признак"@ru,
        "人造外貌表征"@zh ;
    rdfs:comment """This class comprises physical features that are purposely created by human activity, such as scratches, artificial caves, artificial water channels, etc. \r
No assumptions are made as to the extent of modification required to justify regarding a feature as man-made. For example, rock art or even “cup and ring” carvings on bedrock a regarded as types of E25 Man-Made Feature.\r
"""@en ;
    rdfs:subClassOf cidoc_crm:E24_Physical_Man-Made_Thing,
        cidoc_crm:E26_Physical_Feature .

cidoc_crm:E32_Authority_Document a owl:Class ;
    rdfs:label "Referenzdokument"@de,
        "Πηγή Καθιερωμένων Όρων"@el,
        "Authority Document"@en,
        "Document de référence"@fr,
        "Documento de Referência"@pt,
        "Официальный Документ"@ru,
        "权威文献"@zh ;
    rdfs:comment """This class comprises encyclopaedia, thesauri, authority lists and other documents that define terminology or conceptual systems for consistent use.\r
"""@en ;
    rdfs:subClassOf cidoc_crm:E31_Document .

cidoc_crm:E35_Title a owl:Class ;
    rdfs:label "Titel"@de,
        " Τίτλος"@el,
        "Title"@en,
        "Titre"@fr,
        "Título"@pt,
        "Заголовок"@ru,
        "题目"@zh ;
    rdfs:comment """This class comprises the names assigned to works, such as texts, artworks or pieces of music. \r
Titles are proper noun phrases or verbal phrases, and should not be confused with generic object names such as “chair”, “painting” or “book” (the latter are common nouns that stand for instances of E55 Type). Titles may be assigned by the creator of the work itself, or by a social group. \r
This class also comprises the translations of titles that are used as surrogates for the original titles in different social contexts.\r
"""@en ;
    rdfs:subClassOf cidoc_crm:E33_Linguistic_Object,
        cidoc_crm:E41_Appellation .

cidoc_crm:E46_Section_Definition a owl:Class ;
    rdfs:label "Abschnittsdefinition"@de,
        "Ονομασία Τμήματος"@el,
        "Section Definition"@en,
        "Désignation de section"@fr,
        "Designação de Seção"@pt,
        "Определение Района"@ru,
        "区域定义"@zh ;
    rdfs:comment """This class comprises areas of objects referred to in terms specific to the general geometry or structure of its kind. \r
The 'prow' of the boat, the 'frame' of the picture, the 'front' of the building are all instances of E46 Section Definition. The class highlights the fact that parts of objects can be treated as locations. This holds in particular for features without natural boundaries, such as the “head” of a marble statue made out of one block (cf. E53 Place). In answer to the question 'where is the signature?' one might reply 'on the lower left corner'. (Section Definition is closely related to the term “segment” in Gerstl, P.& Pribbenow, S, 1996 “ A conceptual theory of part – whole relations and its applications”, Data & Knowledge 	Engineering 20 305-322, North Holland- Elsevier ).\r
"""@en ;
    rdfs:subClassOf cidoc_crm:E44_Place_Appellation .

cidoc_crm:E56_Language a owl:Class ;
    rdfs:label "Sprache"@de,
        "Γλώσσα"@el,
        "Language"@en,
        "Langue"@fr,
        "Língua"@pt,
        "Язык"@ru,
        "语言"@zh ;
    rdfs:comment """This class is a specialization of E55 Type and comprises the natural languages in the sense of concepts. \r
This type is used categorically in the model without reference to instances of it, i.e. the Model does not foresee the description of instances of instances of E56 Language, e.g.: “instances of  Mandarin Chinese”.\r
It is recommended that internationally or nationally agreed codes and terminology are used to denote instances of E56 Language, such as those defined in ISO 639:1988. \r
"""@en ;
    rdfs:subClassOf cidoc_crm:E55_Type .

cidoc_crm:E58_Measurement_Unit a owl:Class ;
    rdfs:label "Maßeinheit"@de,
        "Μονάδα Μέτρησης"@el,
        "Measurement Unit"@en,
        "Unité de mesure"@fr,
        "Unidade de Medida"@pt,
        "Единица Измерения"@ru,
        "测量单位"@zh ;
    rdfs:comment """This class is a specialization of E55 Type and comprises the types of measurement units: feet, inches, centimetres, litres, lumens, etc. \r
This type is used categorically in the model without reference to instances of it, i.e. the Model does not foresee the description of instances of instances of E58 Measurement Unit, e.g.: “instances of cm”.\r
Syst?me International (SI) units or internationally recognized non-SI terms should be used whenever possible. (ISO 1000:1992). Archaic Measurement Units used in historical records should be preserved.\r
"""@en ;
    rdfs:subClassOf cidoc_crm:E55_Type .

cidoc_crm:E68_Dissolution a owl:Class ;
    rdfs:label "Gruppenauflösung"@de,
        "Διάλυση Ομάδας"@el,
        "Dissolution"@en,
        "Dissolution"@fr,
        "Dissolução"@pt,
        "Роспуск"@ru,
        "解散"@zh ;
    rdfs:comment """This class comprises the events that result in the formal or informal termination of an E74 Group of people. \r
If the dissolution was deliberate, the Dissolution event should also be instantiated as an E7 Activity.\r
"""@en ;
    rdfs:subClassOf cidoc_crm:E64_End_of_Existence .

cidoc_crm:E69_Death a owl:Class ;
    rdfs:label "Tod"@de,
        "Θάνατος"@el,
        "Death"@en,
        "Mort"@fr,
        "Morte"@pt,
        "Смерть"@ru,
        "死亡"@zh ;
    rdfs:comment """This class comprises the deaths of human beings. \r
If a person is killed, their death should be instantiated as E69 Death and as E7 Activity. The death or perishing of other living beings should be documented using E64 End of Existence.\r
"""@en ;
    rdfs:subClassOf cidoc_crm:E64_End_of_Existence .

cidoc_crm:E6_Destruction a owl:Class ;
    rdfs:label "Zerstörung"@de,
        "Καταστροφή"@el,
        "Destruction"@en,
        "Destruction"@fr,
        "Destruição"@pt,
        "Разрушение"@ru,
        "摧毁"@zh ;
    rdfs:comment """This class comprises events that destroy one or more instances of E18 Physical Thing such that they lose their identity as the subjects of documentation.  \r
Some destruction events are intentional, while others are independent of human activity. Intentional destruction may be documented by classifying the event as both an E6 Destruction and E7 Activity. \r
The decision to document an object as destroyed, transformed or modified is context sensitive: \r
1.  If the matter remaining from the destruction is not documented, the event is modelled solely as E6 Destruction. \r
2. An event should also be documented using E81 Transformation if it results in the destruction of one or more objects and the simultaneous production of others using parts or material from the original. In this case, the new items have separate identities. Matter is preserved, but identity is not.\r
3. When the initial identity of the changed instance of E18 Physical Thing is preserved, the event should be documented as E11 Modification. \r
"""@en ;
    rdfs:subClassOf cidoc_crm:E64_End_of_Existence .

cidoc_crm:E75_Conceptual_Object_Appellation a owl:Class ;
    rdfs:label "Begriff- oder Konzeptbenennung "@de,
        "Ονομασία Νοητικού Αντικειμένου"@el,
        "Conceptual Object Appellation"@en,
        "Appellation d'objet conceptuel"@fr,
        "Designação de Objeto Conceitual"@pt,
        "Обозначение Концептуального Объекта"@ru,
        "概念物件称号"@zh ;
    rdfs:comment "This class comprises appellations that are by their form or syntax specific to identifying instances of E28 Conceptual Object, such as intellectual products, standardized patterns etc."@en ;
    rdfs:subClassOf cidoc_crm:E41_Appellation .

cidoc_crm:E82_Actor_Appellation a owl:Class ;
    rdfs:label "Akteurbenennung"@de,
        "Ονομασία Δράστη"@el,
        "Actor Appellation"@en,
        "Appellation d'agent"@fr,
        "Designação de Agente"@pt,
        "Обозначение Агента"@ru,
        "角色称号"@zh ;
    rdfs:comment """This class comprises any sort of name, number, code or symbol characteristically used to identify an E39 Actor. \r
An E39 Actor will typically have more than one E82 Actor Appellation, and instances of E82 Actor Appellation in turn may have alternative representations. The distinction between corporate and personal names, which is particularly important in library applications, should be made by explicitly linking the E82 Actor Appellation to an instance of either E21 Person or E74 Group/E40 Legal Body. If this is not possible, the distinction can be made through the use of the P2 has type mechanism. \r
"""@en ;
    rdfs:subClassOf cidoc_crm:E41_Appellation .

cidoc_crm:E87_Curation_Activity a owl:Class ;
    rdfs:label "Kuratorische Tätigkeit"@de,
        "Curation Activity"@en,
        "典藏管理"@zh ;
    rdfs:comment """This class comprises the activities that result in the continuity of management and the preservation and evolution of instances of E78 Collection, following an implicit or explicit curation plan. \r
It specializes the notion of activity into the curation of a collection and allows the history of curation to be recorded.\r
Items are accumulated and organized following criteria like subject, chronological period, material type, style of art etc. and can be added or removed from an E78 Collection for a specific purpose and/or audience. The initial aggregation of items of a collection is regarded as an instance of E12 Production Event while the activity of evolving, preserving and promoting a collection is regarded as an instance of E87 Curation Activity.\r
"""@en ;
    rdfs:subClassOf cidoc_crm:E7_Activity .

cidoc_crm:P130_shows_features_of a owl:ObjectProperty ;
    rdfs:label "zeigt Merkmale von"@de,
        "παρουσιάζει χαρακτηριστικά του/της"@el,
        "shows features of"@en,
        "présente des caractéristiques de"@fr,
        "apresenta características de"@pt,
        "демонстрирует признаки"@ru,
        "外观特征原出现於"@zh ;
    rdfs:comment """This property generalises the notions of "copy of" and "similar to" into a directed relationship, where\r
the domain expresses the derivative, if such a direction can be established.\r
Otherwise, the relationship is symmetric. If the reason for similarity is a sort of derivation process, i.e.,\r
that the creator has used or had in mind the form of a particular thing during the creation or production,\r
this process should be explicitly modelled. Moreover it expresses similarity in cases that can be stated\r
between two objects only, without historical knowledge about its reasons.\r
	"""@en ;
    rdfs:domain cidoc_crm:E70_Thing ;
    rdfs:range cidoc_crm:E70_Thing .

cidoc_crm:P130i_features_are_also_found_on a owl:ObjectProperty ;
    rdfs:label "Merkmale auch auf"@de,
        "χαρακτηριστικά του βρίσκονται επίσης σε"@el,
        "features are also found on"@en,
        "a des caractéristiques se trouvant aussi sur"@fr,
        "características são também encontradas em"@pt,
        "признаки также найдены на"@ru,
        "外观特征被复制於"@zh ;
    rdfs:domain cidoc_crm:E70_Thing ;
    rdfs:range cidoc_crm:E70_Thing .

cidoc_crm:P3_has_note a owl:DatatypeProperty ;
    rdfs:label "hat Anmerkung"@de,
        "έχει επεξήγηση"@el,
        "has note"@en,
        "a pour note"@fr,
        "tem nota"@pt,
        "имеет примечание"@ru,
        "有说明"@zh ;
    rdfs:comment """This property is a container for all informal descriptions about an object that have not been expressed in terms of CRM constructs. \r
In particular it captures the characterisation of the item itself, its internal structures, appearance etc.\r
Like property P2 has type (is type of), this property is a consequence of the restricted focus of the CRM. The aim is not to capture, in a structured form, everything that can be said about an item; indeed, the CRM formalism is not regarded as sufficient to express everything that can be said. Good practice requires use of distinct note fields for different aspects of a characterisation. The P3.1 has type property of P3 has note allows differentiation of specific notes, e.g. “construction”, “decoration” etc. \r
An item may have many notes, but a note is attached to a specific item.\r
"""@en ;
    rdfs:domain cidoc_crm:E1_CRM_Entity ;
    rdfs:range rdfs:Literal .

cidoc_crm:P49_has_former_or_current_keeper a owl:ObjectProperty ;
    rdfs:label "hat früheren oder derzeitigen Betreuer"@de,
        "είναι ή ήταν στην κατοχή του"@el,
        "has former or current keeper"@en,
        "est ou a été détenu par"@fr,
        "é ou foi guardada por"@pt,
        "имеет бывшего или текущего смотрителя"@ru,
        "有前任或现任保管者"@zh ;
    rdfs:comment """\r
This property identifies the E39 Actor or Actors who have or have had custody of an instance of E18 Physical Thing at\r
some time. This property leaves open the question if parts of this physical thing have\r
been added or removed during the time-spans it has been under the custody of this\r
actor, but it is required that at least a part which can unambiguously be identified as\r
representing the whole has been under this custody for its whole time. The way, in\r
which a representative part is defined, should ensure that it is unambiguous who keeps\r
a part and who the whole and should be consistent with the identity criteria of the kept\r
instance of E18 Physical Thing.\r
The distinction with P50 has current keeper (is current keeper of) is that P49 has former or current\r
keeper (is former or current keeper of) leaves open the question as to whether the specified keepers are\r
current.\r
P49 has former or current keeper (is former or current keeper of) is a shortcut for the more detailed\r
path from E18 Physical Thing through P30 transferred custody of (custody transferred through), E10\r
Transfer of Custody, P28 custody surrendered by (surrendered custody through) or P29 custody\r
received by (received custody through) to E39 Actor.\r
"""@en ;
    rdfs:domain cidoc_crm:E18_Physical_Thing ;
    rdfs:range cidoc_crm:E39_Actor .

cidoc_crm:P49i_is_former_or_current_keeper_of a owl:ObjectProperty ;
    rdfs:label "ist früherer oder derzeitiger Betreuer von"@de,
        "κατέχει ή κατείχε"@el,
        "is former or current keeper of"@en,
        "est ou a été détenteur de"@fr,
        "é ou foi guardador de"@pt,
        "является бывшим или текущим смотрителем для"@ru,
        "目前或曾经保管"@zh ;
    rdfs:domain cidoc_crm:E39_Actor ;
    rdfs:range cidoc_crm:E18_Physical_Thing .

cidoc_crm:P7i_witnessed a owl:ObjectProperty ;
    rdfs:label "bezeugte"@de,
        "υπήρξε τόπος του"@el,
        "witnessed"@en,
        "a été témoin de"@fr,
        "testemunhou"@pt,
        "был местом совершения"@ru,
        "发生过"@zh ;
    rdfs:domain cidoc_crm:E53_Place ;
    rdfs:range cidoc_crm:E4_Period .

cidoc_crm:P81_ongoing_throughout a owl:DatatypeProperty ;
    rdfs:label "andauernd während"@de,
        "καθόλη τη διάρκεια του/της"@el,
        "ongoing throughout"@en,
        "couvre au moins"@fr,
        "abrange no mínimo"@pt,
        "длится в течение"@ru,
        "时段的数值至少涵盖"@zh ;
    rdfs:comment """This property describes the minimum period of time covered by an E52 Time-Span.\r
Since Time-Spans may not have precisely known temporal extents, the CRM supports statements about the minimum and maximum temporal extents of Time-Spans. This property allows a Time-Span’s minimum temporal extent (i.e. its inner boundary) to be assigned an E61 Time Primitive value. Time Primitives are treated by the CRM as application or system specific date intervals, and are not further analysed.\r
"""@en ;
    rdfs:domain cidoc_crm:E52_Time-Span ;
    rdfs:range rdfs:Literal .

cidoc_crm:P82_at_some_time_within a owl:DatatypeProperty ;
    rdfs:label "irgendwann innerhalb von"@de,
        "κάποτε εντός"@el,
        "at some time within"@en,
        "couvre au plus"@fr,
        "abrange no máximo"@pt,
        "некоторое время в течение"@ru,
        "时段的数值不会超越"@zh ;
    rdfs:comment """This property describes the maximum period of time within which an E52 Time-Span falls.\r
Since Time-Spans may not have precisely known temporal extents, the CRM supports statements about the minimum and maximum temporal extents of Time-Spans. This property allows a Time-Span’s maximum temporal extent (i.e. its outer boundary) to be assigned an E61 Time Primitive value. Time Primitives are treated by the CRM as application or system specific date intervals, and are not further analysed.\r
"""@en ;
    rdfs:domain cidoc_crm:E52_Time-Span ;
    rdfs:range rdfs:Literal .

cidoc_crm:E49_Time_Appellation a owl:Class ;
    rdfs:label "Zeitbenennung"@de,
        "Ονομασία Χρόνου"@el,
        "Time Appellation"@en,
        "Appellation temporelle"@fr,
        "Designação de Tempo"@pt,
        "Обозначение Времени"@ru,
        "时间称号"@zh ;
    rdfs:comment """This class comprises all forms of names or codes, such as historical periods, and dates, which are characteristically used to refer to a specific E52 Time-Span. \r
The instances of E49 Time Appellation may vary in their degree of precision, and they may be relative to other time frames, “Before Christ” for example. Instances of E52 Time-Span are often defined by reference to a cultural period or an event e.g. ‘the duration of the Ming Dynasty’."""@en ;
    rdfs:subClassOf cidoc_crm:E41_Appellation .

cidoc_crm:E51_Contact_Point a owl:Class ;
    rdfs:label "Kontaktpunkt"@de,
        "Στοιχείο Επικοινωνίας"@el,
        "Contact Point"@en,
        "Coordonnées individuelles"@fr,
        "Ponto de Contato"@pt,
        "Контакт"@ru,
        "联系方式"@zh ;
    rdfs:comment """This class comprises identifiers employed, or understood, by communication services to direct communications to an instance of E39 Actor. These include E-mail addresses, telephone numbers, post office boxes, Fax numbers, URLs etc. Most postal addresses can be considered both as instances of E44 Place Appellation and E51 Contact Point. In such cases the subclass E45 Address should be used. \r
URLs are addresses used by machines to access another machine through an http request. Since the accessed machine acts on behalf of the E39 Actor providing the machine, URLs are considered as instances of E51 Contact Point to that E39 Actor.\r
"""@en ;
    rdfs:subClassOf cidoc_crm:E41_Appellation .

cidoc_crm:E65_Creation a owl:Class ;
    rdfs:label "Begriffliche Schöpfung"@de,
        "Δημιουργία"@el,
        "Creation"@en,
        "Création"@fr,
        "Criação"@pt,
        "Событие Творения"@ru,
        "创造"@zh ;
    rdfs:comment """This class comprises events that result in the creation of conceptual items or immaterial products, such as legends, poems, texts, music, images, movies, laws, types etc.\r
"""@en ;
    rdfs:subClassOf cidoc_crm:E63_Beginning_of_Existence,
        cidoc_crm:E7_Activity .

cidoc_crm:P140_assigned_attribute_to a owl:ObjectProperty ;
    rdfs:label "wies Merkmal zu"@de,
        "απέδωσε ιδιότητα σε"@el,
        "assigned attribute to"@en,
        "a affecté un attribut à"@fr,
        "atribuiu atributo para"@pt,
        "присвоил атрибут для"@ru,
        "指定属性给"@zh ;
    rdfs:comment "This property indicates the item to which an attribute or relation is assigned. "@en ;
    rdfs:domain cidoc_crm:E13_Attribute_Assignment ;
    rdfs:range cidoc_crm:E1_CRM_Entity .

cidoc_crm:P140i_was_attributed_by a owl:ObjectProperty ;
    rdfs:label "bekam Merkmal zugewiesen durch"@de,
        "χαρακτηρίστηκε από"@el,
        "was attributed by"@en,
        "a reçu un attribut par"@fr,
        "foi atribuído por"@pt,
        "получил атрибут посредством"@ru,
        "被指定属性於"@zh ;
    rdfs:domain cidoc_crm:E1_CRM_Entity ;
    rdfs:range cidoc_crm:E13_Attribute_Assignment .

cidoc_crm:P16_used_specific_object a owl:ObjectProperty ;
    rdfs:label "benutzte das bestimmte Objekt"@de,
        "χρησιμοποίησε αντικείμενο"@el,
        "used specific object"@en,
        "a utilisé l'objet spécifique"@fr,
        "usou objeto específico"@pt,
        "использовал особый объект"@ru,
        "使用特定物"@zh ;
    rdfs:comment """This property describes the use of material or immaterial things in a way essential to the performance or the outcome of an E7 Activity. \r
This property typically applies to tools, instruments, moulds, raw materials and items embedded in a product. It implies that the presence of the object in question was a necessary condition for the action. For example, the activity of writing this text required the use of a computer. An immaterial thing can be used if at least one of its carriers is present. For example, the software tools on a computer.\r
Another example is the use of a particular name by a particular group of people over some span to identify a thing, such as a settlement. In this case, the physical carriers of this name are at least the people understanding its use.\r
"""@en ;
    rdfs:domain cidoc_crm:E7_Activity ;
    rdfs:range cidoc_crm:E70_Thing ;
    rdfs:subPropertyOf cidoc_crm:P12_occurred_in_the_presence_of,
        cidoc_crm:P15_was_influenced_by .

cidoc_crm:P16i_was_used_for a owl:ObjectProperty ;
    rdfs:label "wurde benutzt für"@de,
        "χρησιμοποιήθηκε για"@el,
        "was used for"@en,
        "a été utilisé pour"@fr,
        "foi usado por"@pt,
        "был использован для"@ru,
        "被用於"@zh ;
    rdfs:domain cidoc_crm:E70_Thing ;
    rdfs:range cidoc_crm:E7_Activity ;
    rdfs:subPropertyOf cidoc_crm:P12i_was_present_at,
        cidoc_crm:P15i_influenced .

cidoc_crm:P31_has_modified a owl:ObjectProperty ;
    rdfs:label "veränderte"@de,
        "τροποποίησε"@el,
        "has modified"@en,
        "a modifié"@fr,
        "modificou"@pt,
        "изменил"@ru,
        "修改了"@zh ;
    rdfs:comment """This property identifies the E24 Physical Man-Made Thing modified in an E11 Modification.\r
If a modification is applied to a non-man-made object, it is regarded as an E22 Man-Made Object from that time onwards. \r
"""@en ;
    rdfs:domain cidoc_crm:E11_Modification ;
    rdfs:range cidoc_crm:E24_Physical_Man-Made_Thing ;
    rdfs:subPropertyOf cidoc_crm:P12_occurred_in_the_presence_of .

cidoc_crm:P31i_was_modified_by a owl:ObjectProperty ;
    rdfs:label "wurde verändert durch"@de,
        "τροποποιήθηκε από"@el,
        "was modified by"@en,
        "a été modifié par"@fr,
        "foi modificada por"@pt,
        "был изменен посредством"@ru,
        "被修改於"@zh ;
    rdfs:domain cidoc_crm:E24_Physical_Man-Made_Thing ;
    rdfs:range cidoc_crm:E11_Modification ;
    rdfs:subPropertyOf cidoc_crm:P12i_was_present_at .

cidoc_crm:E14_Condition_Assessment a owl:Class ;
    rdfs:label "Zustandsfeststellung"@de,
        "Εκτίμηση Κατάστασης"@el,
        "Condition Assessment"@en,
        "Expertise de l'état matériel"@fr,
        "Avaliação do Estado Material"@pt,
        "Оценка Состояния"@ru,
        "状态评估"@zh ;
    rdfs:comment """This class describes the act of assessing the state of preservation of an object during a particular period. \r
The condition assessment may be carried out by inspection, measurement or through historical research. This class is used to document circumstances of the respective assessment that may be relevant to interpret its quality at a later stage, or to continue research on related documents. \r
"""@en ;
    rdfs:subClassOf cidoc_crm:E13_Attribute_Assignment .

cidoc_crm:E16_Measurement a owl:Class ;
    rdfs:label "Messung"@de,
        "Μέτρηση"@el,
        "Measurement"@en,
        "Mesurage"@fr,
        "Medição"@pt,
        "Событие Измерения"@ru,
        "测量"@zh ;
    rdfs:comment """This class comprises actions measuring physical properties and other values that can be determined by a systematic procedure. \r
Examples include measuring the monetary value of a collection of coins or the running time of a specific video cassette. \r
The E16 Measurement may use simple counting or tools, such as yardsticks or radiation detection devices. The interest is in the method and care applied, so that the reliability of the result may be judged at a later stage, or research continued on the associated documents. The date of the event is important for dimensions, which may change value over time, such as the length of an object subject to shrinkage. Details of methods and devices are best handled as free text, whereas basic techniques such as "carbon 14 dating" should be encoded using P2 has type (is type of:) E55 Type.\r
"""@en ;
    rdfs:subClassOf cidoc_crm:E13_Attribute_Assignment .

cidoc_crm:E17_Type_Assignment a owl:Class ;
    rdfs:label "Typuszuweisung"@de,
        "Απόδοση Τύπου"@el,
        "Type Assignment"@en,
        "Attribution de type"@fr,
        "Atribuição de Tipo"@pt,
        "Присвоение Типа"@ru,
        "类型指定"@zh ;
    rdfs:comment """This class comprises the actions of classifying items of whatever kind. Such items include objects, specimens, people, actions and concepts. \r
This class allows for the documentation of the context of classification acts in cases where the value of the classification depends on the personal opinion of the classifier, and the date that the classification was made. This class also encompasses the notion of "determination," i.e. the systematic and molecular identification of a specimen in biology. \r
"""@en ;
    rdfs:subClassOf cidoc_crm:E13_Attribute_Assignment .

cidoc_crm:E26_Physical_Feature a owl:Class ;
    rdfs:label "Materielles Merkmal"@de,
        "Υλικό Μόρφωμα"@el,
        "Physical Feature"@en,
        "Caractéristique matérielle"@fr,
        "Característica Material"@pt,
        "Физический Признак"@ru,
        "实体外貌表征"@zh ;
    rdfs:comment """This class comprises identifiable features that are physically attached in an integral way to particular physical objects. \r
Instances of E26 Physical Feature share many of the attributes of instances of E19 Physical Object. They may have a one-, two- or three-dimensional geometric extent, but there are no natural borders that separate them completely in an objective way from the carrier objects. For example, a doorway is a feature but the door itself, being attached by hinges, is not. \r
Instances of E26 Physical Feature can be features in a narrower sense, such as scratches, holes, reliefs, surface colours, reflection zones in an opal crystal or a density change in a piece of wood. In the wider sense, they are portions of particular objects with partially imaginary borders, such as the core of the Earth, an area of property on the surface of the Earth, a landscape or the head of a contiguous marble statue. They can be measured and dated, and it is sometimes possible to state who or what is or was responsible for them. They cannot be separated from the carrier object, but a segment of the carrier object may be identified (or sometimes removed) carrying the complete feature. \r
This definition coincides with the definition of "fiat objects" (Smith & Varzi, 2000, pp.401-420), with the exception of aggregates of “bona fide objects”. \r
"""@en ;
    rdfs:subClassOf cidoc_crm:E18_Physical_Thing .

cidoc_crm:E30_Right a owl:Class ;
    rdfs:label "Recht"@de,
        "Δικαίωμα"@el,
        "Right"@en,
        "Droit"@fr,
        "Direitos"@pt,
        "Право"@ru,
        "权限"@zh ;
    rdfs:comment """This class comprises legal privileges concerning material and immaterial things or their derivatives. \r
These include reproduction and property rights"""@en ;
    rdfs:subClassOf cidoc_crm:E89_Propositional_Object .

cidoc_crm:E31_Document a owl:Class ;
    rdfs:label "Dokument"@de,
        "Τεκμήριο"@el,
        "Document"@en,
        "Document"@fr,
        "Documento"@pt,
        "Документ"@ru,
        "文献"@zh ;
    rdfs:comment """This class comprises identifiable immaterial items that make propositions about reality.\r
These propositions may be expressed in text, graphics, images, audiograms, videograms or by other similar means. Documentation databases are regarded as a special case of E31 Document. This class should not be confused with the term “document” in Information Technology, which is compatible with E73 Information Object.\r
"""@en ;
    rdfs:subClassOf cidoc_crm:E73_Information_Object .

cidoc_crm:E66_Formation a owl:Class ;
    rdfs:label "Gruppenbildung"@de,
        "Συγκρότηση Ομάδας"@el,
        "Formation"@en,
        "Formation"@fr,
        "Formação"@pt,
        "Событие Формирования"@ru,
        "组成"@zh ;
    rdfs:comment """This class comprises events that result in the formation of a formal or informal E74 Group of people, such as a club, society, association, corporation or nation. \r
E66 Formation does not include the arbitrary aggregation of people who do not act as a collective.\r
The formation of an instance of E74 Group does not require that the group is populated with members at the time of formation. In order to express the joining of members at the time of formation, the respective activity should be simultaneously an instance of both E66 Formation and E85 Joining. \r
"""@en ;
    rdfs:subClassOf cidoc_crm:E63_Beginning_of_Existence,
        cidoc_crm:E7_Activity .

cidoc_crm:E78_Collection a owl:Class ;
    rdfs:label "Sammlung"@de,
        "Συλλογή"@el,
        "Collection"@en,
        "Collection"@fr,
        "Coleção"@pt,
        "Коллекция"@ru,
        "收藏"@zh ;
    rdfs:comment """This class comprises aggregations of instances of E18 Physical Thing that are assembled and maintained ("curated" and "preserved", in museological terminology) by one or more instances of E39 Actor over time for a specific purpose and audience, and according to a particular collection development plan.  \r
Items may be added or removed from an E78 Collection in pursuit of this plan. This class should not be confused with the E39 Actor maintaining the E78 Collection often referred to with the name of the E78 Collection (e.g. “The Wallace Collection decided…”).\r
Collective objects in the general sense, like a tomb full of gifts, a folder with stamps or a set of chessmen, should be documented as instances of E19 Physical Object, and not as instances of E78 Collection. This is because they form wholes either because they are physically bound together or because they are kept together for their functionality.\r
"""@en ;
    rdfs:subClassOf cidoc_crm:E24_Physical_Man-Made_Thing .

cidoc_crm:E79_Part_Addition a owl:Class ;
    rdfs:label "Teilhinzufügung"@de,
        "Προσθήκη Μερών"@el,
        "Part Addition"@en,
        "Addition d'élément"@fr,
        "Adição de Parte"@pt,
        "Добавление Части"@ru,
        "部件增加"@zh ;
    rdfs:comment """This class comprises activities that result in an instance of E24 Physical Man-Made Thing being increased, enlarged or augmented by the addition of a part. \r
Typical scenarios include the attachment of an accessory, the integration of a component, the addition of an element to an aggregate object, or the accessioning of an object into a curated E78 Collection. Objects to which parts are added are, by definition, man-made, since the addition of a part implies a human activity. Following the addition of parts, the resulting man-made assemblages are treated objectively as single identifiable wholes, made up of constituent or component parts bound together either physically (for example the engine becoming a part of the car), or by sharing a common purpose (such as the 32 chess pieces that make up a chess set). This class of activities forms a basis for reasoning about the history and continuity of identity of objects that are integrated into other objects over time, such as precious gemstones being repeatedly incorporated into different items of jewellery, or cultural artifacts being added to different museum instances of E78 Collection over their lifespan.\r
"""@en ;
    rdfs:subClassOf cidoc_crm:E11_Modification .

cidoc_crm:E80_Part_Removal a owl:Class ;
    rdfs:label "Teilentfernung"@de,
        "Αφαίρεση Μερών"@el,
        "Part Removal"@en,
        "Soustraction d'élément"@fr,
        "Remoção de Parte"@pt,
        "Удаление Части"@ru,
        "部件删除"@zh ;
    rdfs:comment """This class comprises the activities that result in an instance of E18 Physical Thing being decreased by the removal of a part.\r
Typical scenarios include the detachment of an accessory, the removal of a component or part of a composite object, or the deaccessioning of an object from a curated E78 Collection. If the E80 Part Removal results in the total decomposition of the original object into pieces, such that the whole ceases to exist, the activity should instead be modelled as an E81 Transformation, i.e. a simultaneous destruction and production. In cases where the part removed has no discernible identity prior to its removal but does have an identity subsequent to its removal, the activity should be regarded as both E80 Part Removal and E12 Production. This class of activities forms a basis for reasoning about the history, and continuity of identity over time, of objects that are removed from other objects, such as precious gemstones being extracted from different items of jewelry, or cultural artifacts being deaccessioned from different museum collections over their lifespan.\r
"""@en ;
    rdfs:subClassOf cidoc_crm:E11_Modification .

cidoc_crm:E81_Transformation a owl:Class ;
    rdfs:label "Umwandlung"@de,
        "Μετατροπή"@el,
        "Transformation"@en,
        "Transformation"@fr,
        "Transformação"@pt,
        "Трансформация"@ru,
        "转变"@zh ;
    rdfs:comment """This class comprises the events that result in the simultaneous destruction of one or more than one E77 Persistent Item and the creation of one or more than one E77 Persistent Item that preserves recognizable substance from the first one(s) but has fundamentally different nature and identity. \r
Although the old and the new instances of E77 Persistent Item are treated as discrete entities having separate, unique identities, they are causally connected through the E81 Transformation; the destruction of the old E77 Persistent Item(s) directly causes the creation of the new one(s) using or preserving some relevant substance. Instances of E81 Transformation are therefore distinct from re-classifications (documented using E17 Type Assignment) or modifications (documented using E11 Modification) of objects that do not fundamentally change their nature or identity. Characteristic cases are reconstructions and repurposing of historical buildings or ruins, fires leaving buildings in ruins, taxidermy of specimen in natural history and the reorganization of a corporate body into a new one.\r
"""@en ;
    rdfs:subClassOf cidoc_crm:E63_Beginning_of_Existence,
        cidoc_crm:E64_End_of_Existence .

cidoc_crm:E83_Type_Creation a owl:Class ;
    rdfs:label "Typuserfindung"@de,
        "Δημιουργία Τύπου"@el,
        "Type Creation"@en,
        "Création de type"@fr,
        "Criação de Tipo"@pt,
        "Создание Типа"@ru,
        "类型创造"@zh ;
    rdfs:comment """This class comprises activities formally defining new types of items. \r
It is typically a rigorous scholarly or scientific process that ensures a type is exhaustively described and appropriately named. In some cases, particularly in archaeology and the life sciences, E83 Type Creation requires the identification of an exemplary specimen and the publication of the type definition in an appropriate scholarly forum. The activity of E83 Type Creation is central to research in the life sciences, where a type would be referred to as a “taxon,” the type description as a “protologue,” and the exemplary specimens as “orgininal element” or “holotype”.\r
"""@en ;
    rdfs:subClassOf cidoc_crm:E65_Creation .

cidoc_crm:E85_Joining a owl:Class ;
    rdfs:label "Beitritt"@de,
        "Joining"@en,
        "加入"@zh ;
    rdfs:comment """This class comprises the activities that result in an instance of E39 Actor becoming a member of an instance of E74 Group. This class does not imply initiative by either party. It may be the initiative of a third party.\r
Typical scenarios include becoming a member of a social organisation, becoming employee of a company, marriage, the adoption of a child by a family and the inauguration of somebody into an official position. \r
"""@en ;
    rdfs:subClassOf cidoc_crm:E7_Activity .

cidoc_crm:E86_Leaving a owl:Class ;
    rdfs:label "Austritt"@de,
        "Leaving"@en,
        "脱离"@zh ;
    rdfs:comment """This class comprises the activities that result in an instance of E39 Actor to be disassociated from an instance of E74 Group. This class does not imply initiative by either party. It may be the initiative of a third party. \r
Typical scenarios include the termination of membership in a social organisation, ending the employment at a company, divorce, and the end of tenure of somebody in an official position."""@en ;
    rdfs:subClassOf cidoc_crm:E7_Activity .

cidoc_crm:P14_carried_out_by a owl:ObjectProperty ;
    rdfs:label "wurde ausgeführt von"@de,
        "πραγματοποιήθηκε από"@el,
        "carried out by"@en,
        "réalisée par"@fr,
        "realizada por"@pt,
        "выполнялся"@ru,
        "有执行者"@zh ;
    rdfs:comment """This property describes the active participation of an E39 Actor in an E7 Activity. \r
It implies causal or legal responsibility. The P14.1 in the role of property of the property allows the nature of an Actor’s participation to be specified.\r
"""@en ;
    rdfs:domain cidoc_crm:E7_Activity ;
    rdfs:range cidoc_crm:E39_Actor ;
    rdfs:subPropertyOf cidoc_crm:P11_had_participant .

cidoc_crm:P14i_performed a owl:ObjectProperty ;
    rdfs:label "führte aus"@de,
        "πραγματοποίησε"@el,
        "performed"@en,
        "a exécuté"@fr,
        "executou"@pt,
        "выполнял"@ru,
        "执行了"@zh ;
    rdfs:domain cidoc_crm:E39_Actor ;
    rdfs:range cidoc_crm:E7_Activity ;
    rdfs:subPropertyOf cidoc_crm:P11i_participated_in .

cidoc_crm:P15_was_influenced_by a owl:ObjectProperty ;
    rdfs:label "wurde beeinflußt durch"@de,
        "επηρεάστηκε από"@el,
        "was influenced by"@en,
        "a été influencée par"@fr,
        "foi influenciado por "@pt,
        "находился под влиянием"@ru,
        "有影响事物"@zh ;
    rdfs:comment """This is a high level property, which captures the relationship between an E7 Activity and anything that may have had some bearing upon it.\r
The property has more specific sub properties.\r
"""@en ;
    rdfs:domain cidoc_crm:E7_Activity ;
    rdfs:range cidoc_crm:E1_CRM_Entity .

cidoc_crm:P15i_influenced a owl:ObjectProperty ;
    rdfs:label "beeinflußte"@de,
        "επηρέασε"@el,
        "influenced"@en,
        "a influencé"@fr,
        "influenciou"@pt,
        "оказал влияние на"@ru,
        "影响了"@zh ;
    rdfs:domain cidoc_crm:E1_CRM_Entity ;
    rdfs:range cidoc_crm:E7_Activity .

cidoc_crm:P93_took_out_of_existence a owl:ObjectProperty ;
    rdfs:label "beendete die Existenz von"@de,
        "αναίρεσε"@el,
        "took out of existence"@en,
        "a fait cesser d’exister"@fr,
        "cessou a existência de"@pt,
        "положил конец существованию"@ru,
        "结束了"@zh ;
    rdfs:comment """This property allows an E64 End of Existence event to be linked to the E77 Persistent Item taken out of existence by it.\r
In the case of immaterial things, the E64 End of Existence is considered to take place with the destruction of the last physical carrier.\r
This allows an “end” to be attached to any Persistent Item being documented i.e. E70 Thing, E72 Legal Object, E39 Actor, E41 Appellation, E51 Contact Point and E55 Type. For many Persistent Items we know the maximum life-span and can infer, that they must have ended to exist. We assume in that case an End of Existence, which may be as unnoticeable as forgetting the secret knowledge by the last representative of some indigenous nation.\r
"""@en ;
    rdfs:domain cidoc_crm:E64_End_of_Existence ;
    rdfs:range cidoc_crm:E77_Persistent_Item ;
    rdfs:subPropertyOf cidoc_crm:P12_occurred_in_the_presence_of .

cidoc_crm:P93i_was_taken_out_of_existence_by a owl:ObjectProperty ;
    rdfs:label "wurde seiner Existenz beraubt durch"@de,
        "αναιρέθηκε από"@el,
        "was taken out of existence by"@en,
        "a cessé d’exister du fait de"@fr,
        "deixou de existir"@pt,
        "прекратил существование посредством"@ru,
        "被结束於"@zh ;
    rdfs:domain cidoc_crm:E77_Persistent_Item ;
    rdfs:range cidoc_crm:E64_End_of_Existence ;
    rdfs:subPropertyOf cidoc_crm:P12i_was_present_at .

cidoc_crm:E22_Man-Made_Object a owl:Class ;
    rdfs:label "Künstlicher Gegenstand"@de,
        "Ανθρωπογενές Αντικείμενο"@el,
        "Man-Made Object"@en,
        "Objet fabriqué"@fr,
        "Objeto Fabricado"@pt,
        "Рукотворный Объект"@ru,
        "人造物件"@zh ;
    rdfs:comment """This class comprises physical objects purposely created by human activity.\r
No assumptions are made as to the extent of modification required to justify regarding an object as man-made. For example, an inscribed piece of rock or a preserved butterfly are both regarded as instances of E22 Man-Made Object.\r
"""@en ;
    rdfs:subClassOf cidoc_crm:E19_Physical_Object,
        cidoc_crm:E24_Physical_Man-Made_Thing .

cidoc_crm:P141_assigned a owl:ObjectProperty ;
    rdfs:label "wies zu"@de,
        "απέδωσε"@el,
        "assigned"@en,
        "a attribué"@fr,
        "atribuiu"@pt,
        "присвоил"@ru,
        "指定了属性值"@zh ;
    rdfs:comment """This property indicates the attribute that was assigned or the item that was related to the item denoted by a property P140 assigned attribute to in an Attribute assignment action.\r
"""@en ;
    rdfs:domain cidoc_crm:E13_Attribute_Assignment ;
    rdfs:range cidoc_crm:E1_CRM_Entity .

cidoc_crm:P141i_was_assigned_by a owl:ObjectProperty ;
    rdfs:label "wurde zugewiesen durch"@de,
        "αποδόθηκε από"@el,
        "was assigned by"@en,
        "a été attribué par"@fr,
        "foi atribuído por"@pt,
        "был присвоен посредством"@ru,
        "被指定了属性值於"@zh ;
    rdfs:domain cidoc_crm:E1_CRM_Entity ;
    rdfs:range cidoc_crm:E13_Attribute_Assignment .

cidoc_crm:P67_refers_to a owl:ObjectProperty ;
    rdfs:label "verweist auf"@de,
        "αναφέρεται σε"@el,
        "refers to"@en,
        "fait référence à"@fr,
        "referencia"@pt,
        "ссылается на"@ru,
        "论及"@zh ;
    rdfs:comment """This property documents that an E89 Propositional Object makes a statement about an instance of E1 CRM Entity. P67 refers to (is referred to by) has the P67.1 has type link to an instance of E55 Type. This is intended to allow a more detailed description of the type of reference. This differs from P129 is about (is subject of), which describes the primary subject or subjects of the E89 Propositional Object.\r
"""@en ;
    rdfs:domain cidoc_crm:E89_Propositional_Object ;
    rdfs:range cidoc_crm:E1_CRM_Entity .

cidoc_crm:P67i_is_referred_to_by a owl:ObjectProperty ;
    rdfs:label "wird angeführt von"@de,
        "αναφέρεται από"@el,
        "is referred to by"@en,
        "est référencé par"@fr,
        "é referenciado por"@pt,
        "имеет ссылку на себя от"@ru,
        "被论及於"@zh ;
    rdfs:domain cidoc_crm:E1_CRM_Entity ;
    rdfs:range cidoc_crm:E89_Propositional_Object .

cidoc_crm:P92_brought_into_existence a owl:ObjectProperty ;
    rdfs:label "brachte in Existenz"@de,
        "γέννησε"@el,
        "brought into existence"@en,
        "a fait exister"@fr,
        "trouxe à existência"@pt,
        "создал"@ru,
        "开始了"@zh ;
    rdfs:comment """This property allows an E63 Beginning of Existence event to be linked to the E77 Persistent Item brought into existence by it.\r
It allows a “start” to be attached to any Persistent Item being documented i.e. E70 Thing, E72 Legal Object, E39 Actor, E41 Appellation, E51 Contact Point and E55 Type"""@en ;
    rdfs:domain cidoc_crm:E63_Beginning_of_Existence ;
    rdfs:range cidoc_crm:E77_Persistent_Item ;
    rdfs:subPropertyOf cidoc_crm:P12_occurred_in_the_presence_of .

cidoc_crm:P92i_was_brought_into_existence_by a owl:ObjectProperty ;
    rdfs:label "wurde in Existenz gebracht durch"@de,
        "γεννήθηκε από"@el,
        "was brought into existence by"@en,
        "a commencé à exister du fait de"@fr,
        "passou a existir por"@pt,
        "был создан посредством"@ru,
        "被开始於"@zh ;
    rdfs:domain cidoc_crm:E77_Persistent_Item ;
    rdfs:range cidoc_crm:E63_Beginning_of_Existence ;
    rdfs:subPropertyOf cidoc_crm:P12i_was_present_at .

cidoc_crm:E10_Transfer_of_Custody a owl:Class ;
    rdfs:label "Übertragung des Gewahrsams"@de,
        "Μεταβίβαση  Κατοχής"@el,
        "Transfer of Custody"@en,
        "Changement de détenteur"@fr,
        "Transferência de Custódia"@pt,
        "Передача Опеки"@ru,
        "保管作业转移"@zh ;
    rdfs:comment """This class comprises transfers of physical custody of objects between instances of E39 Actor. \r
The recording of the donor and/or recipient is optional. It is possible that in an instance of E10 Transfer of Custody there is either no donor or no recipient. Depending on the circumstances it may describe:\r
1.	the beginning of custody \r
2.	the end of custody \r
3.	the transfer of custody \r
4.	the receipt of custody from an unknown source\r
5.	the declared loss of an object\r
The distinction between the legal responsibility for custody and the actual physical possession of the object should be expressed using the property P2 has type (is type of). A specific case of transfer of custody is theft.\r
The interpretation of the museum notion of "accession" differs between institutions. The CRM therefore models legal ownership and physical custody separately. Institutions will then model their specific notions of accession and deaccession as combinations of these.\r
"""@en ;
    rdfs:subClassOf cidoc_crm:E7_Activity .

cidoc_crm:E15_Identifier_Assignment a owl:Class ;
    rdfs:label "Kennzeichenzuweisung"@de,
        "Απόδοση Αναγνωριστικού"@el,
        "Identifier Assignment"@en,
        "Attribution d’identificateur"@fr,
        "Atribuição de Identificador"@pt,
        "Назначение Идентификатора"@ru,
        "标识符指定"@zh ;
    rdfs:comment """This class comprises activities that result in the allocation of an identifier to an instance of E1 CRM Entity. An E15 Identifier Assignment may include the creation of the identifier from multiple constituents, which themselves may be instances of E41 Appellation. The syntax and kinds of constituents to be used may be declared in a rule constituting an instance of E29 Design or Procedure.\r
Examples of such identifiers include Find Numbers, Inventory Numbers, uniform titles in the sense of librarianship and Digital Object Identifiers (DOI). Documenting the act of identifier assignment and deassignment is especially useful when objects change custody or the identification system of an organization is changed. In order to keep track of the identity of things in such cases, it is important to document by whom, when and for what purpose an identifier is assigned to an item.\r
The fact that an identifier is a preferred one for an organisation can be expressed by using the property E1 CRM Entity. P48 has preferred identifier (is preferred identifier of): E42 Identifier. It can better be expressed in a context independent form by assigning a suitable E55 Type, such as “preferred identifier assignment”, to the respective instance of E15 Identifier Assignment via the P2 has type property.\r
"""@en ;
    rdfs:subClassOf cidoc_crm:E13_Attribute_Assignment .

cidoc_crm:E29_Design_or_Procedure a owl:Class ;
    rdfs:label "Entwurf oder Verfahren"@de,
        "Σχέδιο"@el,
        "Design or Procedure"@en,
        "Conception ou procédure"@fr,
        "Projeto ou Procedimento"@pt,
        "Проект или Процедура"@ru,
        "设计或程序"@zh ;
    rdfs:comment """This class comprises documented plans for the execution of actions in order to achieve a result of a specific quality, form or contents. In particular it comprises plans for deliberate human activities that may result in the modification or production of instances of E24 Physical Thing. \r
Instances of E29 Design or Procedure can be structured in parts and sequences or depend on others. This is modelled using P69 has association with (is associated with). \r
Designs or procedures can be seen as one of the following:\r
1.	A schema for the activities it describes\r
2.	A schema of the products that result from their application. \r
3.	An independent intellectual product that may have never been applied, such as Leonardo da Vinci’s famous plans for flying machines.\r
Because designs or procedures may never be applied or only partially executed, the CRM models a loose relationship between the plan and the respective product.\r
"""@en ;
    rdfs:subClassOf cidoc_crm:E73_Information_Object .

cidoc_crm:E36_Visual_Item a owl:Class ;
    rdfs:label "Bildliches"@de,
        "Οπτικό Στοιχείο"@el,
        "Visual Item"@en,
        "Item visuel"@fr,
        "Item Visual"@pt,
        "Визуальный Предмет"@ru,
        "视觉项目"@zh ;
    rdfs:comment """This class comprises the intellectual or conceptual aspects of recognisable marks and images.\r
This class does not intend to describe the idiosyncratic characteristics of an individual physical embodiment of a visual item, but the underlying prototype. For example, a mark such as the ICOM logo is generally considered to be the same logo when used on any number of publications. The size, orientation and colour may change, but the logo remains uniquely identifiable. The same is true of images that are reproduced many times. This means that visual items are independent of their physical support. \r
The class E36 Visual Item provides a means of identifying and linking together instances of E24 Physical Man-Made Thing that carry the same visual symbols, marks or images etc. The property P62 depicts (is depicted by) between E24 Physical Man-Made Thing and depicted subjects (E1 CRM Entity) can be regarded as a short-cut of the more fully developed path from E24 Physical Man-Made Thing through P65 shows visual item (is shown by), E36 Visual Item, P138 represents (has representation) to E1CRM Entity, which in addition captures the optical features of the depiction.  \r
"""@en ;
    rdfs:subClassOf cidoc_crm:E73_Information_Object .

cidoc_crm:E42_Identifier a owl:Class ;
    rdfs:label "Kennung"@de,
        "Κωδικός Αναγνώρισης"@el,
        "Identifier"@en,
        "Identificateur d'objet"@fr,
        "Identificador de Objeto"@pt,
        "Идентификатор Объекта"@ru,
        "标识符"@zh ;
    rdfs:comment "This class comprises strings or codes assigned to instances of E1 CRM Entity in order to identify them uniquely and permanently within the context of one or more organisations. Such codes are often known as inventory numbers, registration codes, etc. and are typically composed of alphanumeric sequences. The class E42 Identifier is not normally used for machine-generated identifiers used for automated processing unless these are also used by human agents."@en ;
    rdfs:subClassOf cidoc_crm:E41_Appellation .

cidoc_crm:E44_Place_Appellation a owl:Class ;
    rdfs:label "Ortsbenennung"@de,
        "Ονομασία Τόπου"@el,
        "Place Appellation"@en,
        "Appellation de lieu"@fr,
        "Designação de Local"@pt,
        "Обозначение Места"@ru,
        "地点称号"@zh ;
    rdfs:comment """This class comprises any sort of identifier characteristically used to refer to an E53 Place. \r
Instances of E44 Place Appellation may vary in their degree of precision and their meaning may vary over time - the same instance of E44 Place Appellation may be used to refer to several places, either because of cultural shifts, or because objects used as reference points have moved around. Instances of E44 Place Appellation can be extremely varied in form: postal addresses, instances of E47 Spatial Coordinate, and parts of buildings can all be considered as instances of E44 Place Appellation.\r
"""@en ;
    rdfs:subClassOf cidoc_crm:E41_Appellation .

cidoc_crm:E57_Material a owl:Class ;
    rdfs:label "Material"@de,
        "Υλικό"@el,
        "Material"@en,
        "Matériau"@fr,
        "Material"@pt,
        "Материал"@ru,
        "材料"@zh ;
    rdfs:comment """This class is a specialization of E55 Type and comprises the concepts of materials. \r
Instances of E57 Material may denote properties of matter before its use, during its use, and as incorporated in an object, such as ultramarine powder, tempera paste, reinforced concrete. Discrete pieces of raw-materials kept in museums, such as bricks, sheets of fabric, pieces of metal, should be modelled individually in the same way as other objects. Discrete used or processed pieces, such as the stones from Nefer Titi's temple, should be modelled as parts (cf. P46 is composed of).\r
This type is used categorically in the model without reference to instances of it, i.e. the Model does not foresee the description of instances of instances of E57 Material, e.g.: “instances of  gold”.\r
It is recommended that internationally or nationally agreed codes and terminology are used."""@en ;
    rdfs:subClassOf cidoc_crm:E55_Type .

cidoc_crm:E64_End_of_Existence a owl:Class ;
    rdfs:label "Daseinsende"@de,
        "Τέλος Ύπαρξης"@el,
        "End of Existence"@en,
        "Fin d'existence"@fr,
        "Fim da Existência"@pt,
        "Конец Существования"@ru,
        "存在结束"@zh ;
    rdfs:comment """This class comprises events that end the existence of any E77 Persistent Item. \r
It may be used for temporal reasoning about things (physical items, groups of people, living beings) ceasing to exist; it serves as a hook for determination of a terminus postquem and antequem. In cases where substance from a Persistent Item continues to exist in a new form, the process would be documented by E81 Transformation.\r
"""@en ;
    rdfs:subClassOf cidoc_crm:E5_Event .

cidoc_crm:E67_Birth a owl:Class ;
    rdfs:label "Geburt"@de,
        "Γέννηση"@el,
        "Birth"@en,
        "Naissance"@fr,
        "Nascimento"@pt,
        "Рождение"@ru,
        "诞生"@zh ;
    rdfs:comment """This class comprises the births of human beings. E67 Birth is a biological event focussing on the context of people coming into life. (E63 Beginning of Existence comprises the coming into life of any living beings). \r
Twins, triplets etc. are brought into life by the same E67 Birth event. The introduction of the E67 Birth event as a documentation element allows the description of a range of family relationships in a simple model. Suitable extensions may describe more details and the complexity of motherhood with the intervention of modern medicine. In this model, the biological father is not seen as a necessary participant in the E67 Birth event.\r
"""@en ;
    rdfs:subClassOf cidoc_crm:E63_Beginning_of_Existence .

cidoc_crm:E72_Legal_Object a owl:Class ;
    rdfs:label "Rechtsobjekt"@de,
        "Νομικό Αντικείμενο"@el,
        "Legal Object"@en,
        "Objet juridique"@fr,
        "Objeto Jurídico"@pt,
        "Объект Права"@ru,
        "法律物件"@zh ;
    rdfs:comment """This class comprises those material or immaterial items to which instances of E30 Right, such as the right of ownership or use, can be applied. \r
This is true for all E18 Physical Thing. In the case of instances of E28 Conceptual Object, however, the identity of the E28 Conceptual Object or the method of its use may be too ambiguous to reliably establish instances of E30 Right, as in the case of taxa and inspirations. Ownership of corporations is currently regarded as out of scope of the CRM. \r
"""@en ;
    rdfs:subClassOf cidoc_crm:E70_Thing .

cidoc_crm:E8_Acquisition a owl:Class ;
    rdfs:label "Erwerb"@de,
        "Απόκτηση"@el,
        "Acquisition"@en,
        "Acquisition"@fr,
        "Aquisição"@pt,
        "Событие Приобретения"@ru,
        "征集取得"@zh ;
    rdfs:comment """This class comprises transfers of legal ownership from one or more instances of E39 Actor to one or more other instances of E39 Actor. \r
The class also applies to the establishment or loss of ownership of instances of E18 Physical Thing. It does not, however, imply changes of any other kinds of right. The recording of the donor and/or recipient is optional. It is possible that in an instance of E8 Acquisition there is either no donor or no recipient. Depending on the circumstances, it may describe:\r
1.	the beginning of ownership\r
2.	the end of ownership\r
3.	the transfer of ownership\r
4.	the acquisition from an unknown source \r
5.	the loss of title due to destruction of the item\r
It may also describe events where a collector appropriates legal title, for example by annexation or field collection. The interpretation of the museum notion of "accession" differs between institutions. The CRM therefore models legal ownership (E8 Acquisition) and physical custody (E10 Transfer of Custody) separately. Institutions will then model their specific notions of accession and deaccession as combinations of these.\r
"""@en ;
    rdfs:subClassOf cidoc_crm:E7_Activity .

cidoc_crm:E93_Presence a owl:Class ;
    rdfs:label "Presence"@en ;
    rdfs:comment """This class comprises instances of E92 Spacetime Volume that result from intersection of instances of E92 Spacetime Volume with an instance of E52 Time-Span.  The identity of an instance of this class is determined by the identities of the  constituing spacetime volume and the time-span. \r
	\r
This class can be used to define temporal snapshots at a particular time-span, such as the extent of the Roman Empire at 33 B.C., or the extent occupied by a museum object at rest in an exhibit. In particular, it can be used to define the spatial projection of a spacetime volume during a particular time-span,  such as the maximal spatial extent of a flood at some particular hour, or all areas covered by the Poland within the 20th century AD.\r
"""@en ;
    rdfs:subClassOf cidoc_crm:E92_Spacetime_Volume .

cidoc_crm:E9_Move a owl:Class ;
    rdfs:label "Objektbewegung"@de,
        "Μετακίνηση"@el,
        "Move"@en,
        "Déplacement"@fr,
        "Locomoção"@pt,
        "Перемещение"@ru,
        "移动"@zh ;
    rdfs:comment """This class comprises changes of the physical location of the instances of E19 Physical Object. \r
Note, that the class E9 Move inherits the property P7 took place at (witnessed): E53 Place. This property should be used to describe the trajectory or a larger area within which a move takes place, whereas the properties P26 moved to (was destination of), P27 moved from (was origin of) describe the start and end points only. Moves may also be documented to consist of other moves (via P9 consists of (forms part of)), in order to describe intermediate stages on a trajectory. In that case, start and end points of the partial moves should match appropriately between each other and with the overall event.\r
"""@en ;
    rdfs:subClassOf cidoc_crm:E7_Activity .

cidoc_crm:P1_is_identified_by a owl:ObjectProperty ;
    rdfs:label "wird bezeichnet als"@de,
        "αναγνωρίζεται ως"@el,
        "is identified by"@en,
        "est identifiée par"@fr,
        "é identificado por"@pt,
        "идентифицируется посредством"@ru,
        "有识别称号"@zh ;
    rdfs:comment """This property describes the naming or identification of any real world item by a name or any other identifier. \r
This property is intended for identifiers in general use, which form part of the world the model intends to describe, and not merely for internal database identifiers which are specific to a technical system, unless these latter also have a more general use outside the technical context. This property includes in particular identification by mathematical expressions such as coordinate systems used for the identification of instances of E53 Place. The property does not reveal anything about when, where and by whom this identifier was used. A more detailed representation can be made using the fully developed (i.e. indirect) path through E15 Identifier Assignment.\r
"""@en ;
    rdfs:domain cidoc_crm:E1_CRM_Entity ;
    rdfs:range cidoc_crm:E41_Appellation .

cidoc_crm:P1i_identifies a owl:ObjectProperty ;
    rdfs:label "bezeichnet"@de,
        "είναι αναγνωριστικό"@el,
        "identifies"@en,
        "identifie"@fr,
        "identifica"@pt,
        "идентифицирует"@ru,
        "被用来识别"@zh ;
    rdfs:domain cidoc_crm:E41_Appellation ;
    rdfs:range cidoc_crm:E1_CRM_Entity .

cidoc_crm:E11_Modification a owl:Class ;
    rdfs:label "Bearbeitung"@de,
        "Τροποποίηση"@el,
        "Modification"@en,
        "Modification"@fr,
        "Modificação"@pt,
        "Событие Изменения"@ru,
        "修改"@zh ;
    rdfs:comment """This class comprises all instances of E7 Activity that create, alter or change E24 Physical Man-Made Thing. \r
This class includes the production of an item from raw materials, and other so far undocumented objects, and the preventive treatment or restoration of an object for conservation. \r
Since the distinction between modification and production is not always clear, modification is regarded as the more generally applicable concept. This implies that some items may be consumed or destroyed in a Modification, and that others may be produced as a result of it. An event should also be documented using E81 Transformation if it results in the destruction of one or more objects and the simultaneous production of others using parts or material from the originals. In this case, the new items have separate identities. \r
If the instance of the E29 Design or Procedure utilized for the modification prescribes the use of specific materials, they should be documented using property P68 foresees use of (use foreseen by): E57 Material of E29 Design or Procedure, rather than via P126 employed (was employed in): E57 Material.\r
"""@en ;
    rdfs:subClassOf cidoc_crm:E7_Activity .

cidoc_crm:E28_Conceptual_Object a owl:Class ;
    rdfs:label "Begrifflicher Gegenstand"@de,
        "Νοητικό Αντικείμενο"@el,
        "Conceptual Object"@en,
        "Objet conceptuel"@fr,
        "Objeto Conceitual"@pt,
        "Концептуальный Объект"@ru,
        "概念物件"@zh ;
    rdfs:comment """This class comprises non-material products of our minds and other human produced data that 		have become objects of a discourse about their identity, circumstances of creation or historical 		implication. The production of such information may have been supported by the use of    		technical devices such as cameras or computers.\r
Characteristically, instances of this class are created, invented or thought by someone, and then may be documented or communicated between persons. Instances of E28 Conceptual Object have the ability to exist on more than one particular carrier at the same time, such as paper, electronic signals, marks, audio media, paintings, photos, human memories, etc.\r
They cannot be destroyed. They exist as long as they can be found on at least one carrier or in at least one human memory. Their existence ends when the last carrier and the last memory are lost. \r
"""@en ;
    rdfs:subClassOf cidoc_crm:E71_Man-Made_Thing .

cidoc_crm:E63_Beginning_of_Existence a owl:Class ;
    rdfs:label "Daseinsbeginn"@de,
        "Αρχή Ύπαρξης"@el,
        "Beginning of Existence"@en,
        "Début d'existence"@fr,
        "Início da Existência"@pt,
        "Начало Существования"@ru,
        "存在开始"@zh ;
    rdfs:comment """This class comprises events that bring into existence any E77 Persistent Item. \r
It may be used for temporal reasoning about things (intellectual products, physical items, groups of people, living beings) beginning to exist; it serves as a hook for determination of a terminus post quem and ante quem. """@en ;
    rdfs:subClassOf cidoc_crm:E5_Event .

cidoc_crm:E73_Information_Object a owl:Class ;
    rdfs:label "Informationsgegenstand"@de,
        "Πληροφοριακό Αντικείμενο"@el,
        "Information Object"@en,
        "Objet d'information"@fr,
        "Objeto de Informação"@pt,
        "Информационный Объект"@ru,
        "信息物件"@zh ;
    rdfs:comment """This class comprises identifiable immaterial items, such as a poems, jokes, data sets, images, texts, multimedia objects, procedural prescriptions, computer program code, algorithm or mathematical formulae, that have an objectively recognizable structure and are documented as single units. The encoding structure known as a "named graph" also falls under this class, so that each "named graph" is an instance of an E73 Information Object. \r
An E73 Information Object does not depend on a specific physical carrier, which can include human memory, and it can exist on one or more carriers simultaneously. \r
Instances of E73 Information Object of a linguistic nature should be declared as instances of the E33 Linguistic Object subclass. Instances of E73 Information Object of a documentary nature should be declared as instances of the E31 Document subclass. Conceptual items such as types and classes are not instances of E73 Information Object, nor are ideas without a reproducible expression. \r
 """@en ;
    rdfs:subClassOf cidoc_crm:E89_Propositional_Object,
        cidoc_crm:E90_Symbolic_Object .

cidoc_crm:E13_Attribute_Assignment a owl:Class ;
    rdfs:label "Merkmalszuweisung"@de,
        "Απόδοση Ιδιοτήτων"@el,
        "Attribute Assignment"@en,
        "Affectation d'attribut"@fr,
        "Atribuição de Característica"@pt,
        "Присвоение Атрибута"@ru,
        "屬性指定"@zh ;
    rdfs:comment """This class comprises the actions of making assertions about properties of an object or any relation between two items or concepts. \r
This class allows the documentation of how the respective assignment came about, and whose opinion it was. All the attributes or properties assigned in such an action can also be seen as directly attached to the respective item or concept, possibly as a collection of contradictory values. All cases of properties in this model that are also described indirectly through an action are characterised as "short cuts" of this action. This redundant modelling of two alternative views is preferred because many implementations may have good reasons to model either the action or the short cut, and the relation between both alternatives can be captured by simple rules. \r
In particular, the class describes the actions of people making propositions and statements during certain museum procedures, e.g. the person and date when a condition statement was made, an identifier was assigned, the museum object was measured, etc. Which kinds of such assignments and statements need to be documented explicitly in structures of a schema rather than free text, depends on if this information should be accessible by structured queries. \r
"""@en ;
    rdfs:subClassOf cidoc_crm:E7_Activity .

cidoc_crm:E33_Linguistic_Object a owl:Class ;
    rdfs:label "Sprachlicher Gegenstand"@de,
        "Γλωσσικό Αντικείμενο"@el,
        "Linguistic Object"@en,
        "Objet linguistique"@fr,
        "Objeto Lingüístico"@pt,
        "Линвистический Объект"@ru,
        "语言物件"@zh ;
    rdfs:comment """This class comprises identifiable expressions in natural language or languages. \r
Instances of E33 Linguistic Object can be expressed in many ways: e.g. as written texts, recorded speech or sign language. However, the CRM treats instances of E33 Linguistic Object independently from the medium or method by which they are expressed. Expressions in formal languages, such as computer code or mathematical formulae, are not treated as instances of E33 Linguistic Object by the CRM. These should be modelled as instances of E73 Information Object.\r
The text of an instance of E33 Linguistic Object can be documented in a note by P3 has note: E62 String\r
"""@en ;
    rdfs:subClassOf cidoc_crm:E73_Information_Object .

cidoc_crm:E3_Condition_State a owl:Class ;
    rdfs:label "Zustandsphase"@de,
        "Κατάσταση"@el,
        "Condition State"@en,
        "État matériel"@fr,
        "Estado Material"@pt,
        "Состояние"@ru,
        "状态"@zh ;
    rdfs:comment """This class comprises the states of objects characterised by a certain condition over a time-span. \r
An instance of this class describes the prevailing physical condition of any material object or feature during a specific E52 Time Span. In general, the time-span for which a certain condition can be asserted may be shorter than the real time-span, for which this condition held.\r
 The nature of that condition can be described using P2 has type. For example, the E3 Condition State “condition of the SS Great Britain between 22 September 1846 and 27 August 1847” can be characterized as E55 Type “wrecked”. \r
"""@en ;
    rdfs:subClassOf cidoc_crm:E2_Temporal_Entity .

cidoc_crm:E71_Man-Made_Thing a owl:Class ;
    rdfs:label "Künstliches"@de,
        "Ανθρώπινο Δημιούργημα"@el,
        "Man-Made Thing"@en,
        "Chose fabriquée"@fr,
        "Coisa Fabricada"@pt,
        "Рукотворная Вещь"@ru,
        "人造物"@zh ;
    rdfs:comment """This class comprises discrete, identifiable man-made items that are documented as single units. \r
These items are either intellectual products or man-made physical things, and are characterized by relative stability. They may for instance have a solid physical form, an electronic encoding, or they may be logical concepts or structures.\r
"""@en ;
    rdfs:subClassOf cidoc_crm:E70_Thing .

cidoc_crm:P11_had_participant a owl:ObjectProperty ;
    rdfs:label "hatte Teilnehmer"@de,
        "είχε συμμέτοχο"@el,
        "had participant"@en,
        "a eu pour participant"@fr,
        "tem participante"@pt,
        "имел участника"@ru,
        "有参与者"@zh ;
    rdfs:comment """This property describes the active or passive participation of instances of E39 Actors in an E5 Event. \r
It connects the life-line of the related E39 Actor with the E53 Place and E50 Date of the event. The property implies that the Actor was involved in the event but does not imply any causal relationship. The subject of a portrait can be said to have participated in the creation of the portrait.\r
"""@en ;
    rdfs:domain cidoc_crm:E5_Event ;
    rdfs:range cidoc_crm:E39_Actor ;
    rdfs:subPropertyOf cidoc_crm:P12_occurred_in_the_presence_of .

cidoc_crm:P11i_participated_in a owl:ObjectProperty ;
    rdfs:label "nahm Teil an"@de,
        "συμμετείχε σε"@el,
        "participated in"@en,
        "a participé à"@fr,
        "participa em"@pt,
        "участвовал в"@ru,
        "参与了"@zh ;
    rdfs:domain cidoc_crm:E39_Actor ;
    rdfs:range cidoc_crm:E5_Event ;
    rdfs:subPropertyOf cidoc_crm:P12i_was_present_at .

cidoc_crm:P12_occurred_in_the_presence_of a owl:ObjectProperty ;
    rdfs:label "fand statt im Beisein von"@de,
        "συνέβη παρουσία του/της"@el,
        "occurred in the presence of"@en,
        "est arrivé en présence de"@fr,
        "ocorreu na presença de"@pt,
        "появился в присутствии"@ru,
        "发生现场存在"@zh ;
    rdfs:comment """This property describes the active or passive presence of an E77 Persistent Item in an E5 Event without implying any specific role. \r
It connects the history of a thing with the E53 Place and E50 Date of an event. For example, an object may be the desk, now in a museum on which a treaty was signed. The presence of an immaterial thing implies the presence of at least one of its carriers.\r
"""@en ;
    rdfs:domain cidoc_crm:E5_Event ;
    rdfs:range cidoc_crm:E77_Persistent_Item .

cidoc_crm:P12i_was_present_at a owl:ObjectProperty ;
    rdfs:label "war anwesend bei"@de,
        "ήταν παρών/παρούσα/παρόν σε"@el,
        "was present at"@en,
        "était présent à"@fr,
        "estava presente no"@pt,
        "присутствовал при"@ru,
        "当时在场於"@zh ;
    rdfs:domain cidoc_crm:E77_Persistent_Item ;
    rdfs:range cidoc_crm:E5_Event .

cidoc_crm:E4_Period a owl:Class ;
    rdfs:label "Phase"@de,
        "Περίοδος"@el,
        "Period"@en,
        "Période"@fr,
        "Período"@pt,
        "Период"@ru,
        "期间"@zh ;
    rdfs:comment """This class comprises sets of coherent phenomena or cultural manifestations occurring in time and space.\r
\r
It is the social or physical coherence of these phenomena that identify an E4 Period and not the associated spatiotemporal extent. This extent is only the "ground" or space in an abstract physical sense that the actual process of growth, spread and retreat has covered. Consequently, different periods can overlap and coexist in time and space, such as when a nomadic culture exists in the same area and time as a sedentary culture. This also means that overlapping land use rights, common among first nations, amounts to overlapping periods.\r
\r
Often, this class is used to describe prehistoric or historic periods such as the "Neolithic Period", the "Ming Dynasty" or the "McCarthy Era", but also geopolitical units and activities of settlements are regarded as special cases of E4 Period. However, there are no assumptions about the scale of the associated phenomena. In particular all events are seen as synthetic processes consisting of coherent phenomena. Therefore E4 Period is a superclass of E5 Event. For example, a modern clinical E67 Birth can be seen as both an atomic E5 Event and as an E4 Period that consists of multiple activities performed by multiple instances of E39 Actor.\r
\r
As the actual extent of an E4 Period in spacetime we regard the trajectories of the participating physical things during their participation in an instance of E4 Period. This includes the open spaces via which these things have interacted and the spaces by which they had the potential to interact during that period or event in the way defined by the type of the respective period or event. Examples include the air in a meeting room transferring the voices of the participants. Since these phenomena are fuzzy, we assume the spatiotemporal extent to be contiguous, except for cases of phenomena spreading out over islands or other separated areas, including geopolitical units distributed over disconnected areas such as islands or colonies.\r
\r
Whether the trajectories necessary for participants to travel between these areas are regarded as part of the spatiotemporal extent or not has to be decided in each case based on a concrete analysis, taking use of the sea for other purposes than travel, such as fishing, into consideration. One may also argue that the activities to govern disconnected areas imply travelling through spaces connecting them and that these areas hence are spatially connected in a way, but it appears counterintuitive to consider for instance travel routes in international waters as extensions of geopolitical units.\r
\r
Consequently, an instance of E4 Period may occupy a number of disjoint spacetime volumes, however there must not be a discontinuity in the  timespan covered by these spacetime volumes. This means that an instance of E4 Period must be contiguous in time. If it has ended in all areas, it has ended as a whole. However it may end in one area before another, such as in the Polynesian migration, and it continues as long as it is ongoing in at least  one area.\r
\r
We model E4 Period as a subclass of E2 Temporal Entity and of E92 Spacetime volume. The latter is intended as a phenomenal spacetime volume as defined in CRMgeo (Doerr and Hiebel 2013). By virtue of this multiple inheritance we can discuss the physical extent of an E4 Period without representing each instance of it together with an instance of its associated spacetime volume. This model combines two quite different kinds of substance: an instance of E4 Period is a phenomena while a space-time volume is an aggregation of points in spacetime. However, the real spatiotemporal extent of an instance of E4 Period is regarded to be unique to it due to all its details and fuzziness; its identity and existence depends uniquely on the identity of the instance of E4 Period. Therefore this multiple inheritance is unambiguous and effective and furthermore corresponds to the intuitions of natural language.\r
\r
There are two different conceptualisations of 'artistic style', defined either by physical features or by historical context. For example, “Impressionism” can be viewed as a period lasting from approximately 1870 to 1905 during which paintings with particular characteristics were produced by a group of artists that included (among others) Monet, Renoir, Pissarro, Sisley and Degas. Alternatively, it can be regarded as a style applicable to all paintings sharing the characteristics of the works produced by the Impressionist painters, regardless of historical context. The first interpretation is an instance of E4 Period, and the second defines morphological object types that fall under E55 Type.\r
\r
Another specific case of an E4 Period is the set of activities and phenomena associated with a settlement, such as the populated period of Nineveh.\r
"""@en ;
    rdfs:subClassOf cidoc_crm:E2_Temporal_Entity,
        cidoc_crm:E92_Spacetime_Volume .

cidoc_crm:E5_Event a owl:Class ;
    rdfs:label "Ereignis"@de,
        "Συμβάν"@el,
        "Event"@en,
        "Événement"@fr,
        "Evento"@pt,
        "Событие"@ru,
        "事件"@zh ;
    rdfs:comment """This class comprises changes of states in cultural, social or physical systems, regardless of scale, brought about by a series or group of coherent physical, cultural, technological or legal phenomena. Such changes of state will affect instances of E77 Persistent Item or its subclasses.\r
The distinction between an E5 Event and an E4 Period is partly a question of the scale of observation. Viewed at a coarse level of detail, an E5 Event is an ‘instantaneous’ change of state. At a fine level, the E5 Event can be analysed into its component phenomena within a space and time frame, and as such can be seen as an E4 Period. The reverse is not necessarily the case: not all instances of E4 Period give rise to a noteworthy change of state.\r
"""@en ;
    rdfs:subClassOf cidoc_crm:E4_Period .

cidoc_crm:E89_Propositional_Object a owl:Class ;
    rdfs:label "Aussagenobjekt"@de,
        "Propositional Object"@en,
        "陈述性物件"@zh ;
    rdfs:comment """This class comprises immaterial items, including but not limited to stories, plots, procedural prescriptions, algorithms, laws of physics or images that are, or represent in some sense, sets of propositions about real or imaginary things and that are documented as single units or serve as topics of discourse. \r
	\r
This class also comprises items that are “about” something in the sense of a subject. In the wider sense, this class includes expressions of psychological value such as non-figural art and musical themes. However, conceptual items such as types and classes are not instances of E89 Propositional Object. This should not be confused with the definition of a type, which is indeed an instance of E89 Propositional Object.\r
"""@en ;
    rdfs:subClassOf cidoc_crm:E28_Conceptual_Object .

cidoc_crm:E19_Physical_Object a owl:Class ;
    rdfs:label "Materieller Gegenstand"@de,
        "Υλικό Αντικείμενο"@el,
        "Physical Object"@en,
        "Objet matériel"@fr,
        "Objeto Material"@pt,
        "Физический Объект"@ru,
        "实体物件"@zh ;
    rdfs:comment """This class comprises items of a material nature that are units for documentation and have physical boundaries that separate them completely in an objective way from other objects. \r
The class also includes all aggregates of objects made for functional purposes of whatever kind, independent of physical coherence, such as a set of chessmen. Typically, instances of E19 Physical Object can be moved (if not too heavy).\r
In some contexts, such objects, except for aggregates, are also called “bona fide objects” (Smith & Varzi, 2000, pp.401-420), i.e. naturally defined objects. \r
The decision as to what is documented as a complete item, rather than by its parts or components, may be a purely administrative decision or may be a result of the order in which the item was acquired.\r
"""@en ;
    rdfs:subClassOf cidoc_crm:E18_Physical_Thing .

cidoc_crm:E54_Dimension a owl:Class ;
    rdfs:label "Maß"@de,
        "Μέγεθος"@el,
        "Dimension"@en,
        "Dimensions"@fr,
        "Dimensão"@pt,
        "Величина"@ru,
        "规模数量"@zh ;
    rdfs:comment """This class comprises quantifiable properties that can be measured by some calibrated means and can be approximated by values, i.e. points or regions in a mathematical or conceptual space, such as natural or real numbers, RGB values etc.\r
An instance of E54 Dimension represents the true quantity, independent from its numerical approximation, e.g. in inches or in cm. The properties of the class E54 Dimension allow for expressing the numerical approximation of the values of an instance of E54 Dimension. If the true values belong to a non-discrete space, such as spatial distances, it is recommended to record them as approximations by intervals or regions of indeterminacy enclosing the assumed true values. For instance, a length of 5 cm may be recorded as 4.5-5.5 cm, according to the precision of the respective observation. Note, that interoperability of values described in different units depends critically on the representation as value regions.\r
Numerical approximations in archaic instances of E58 Measurement Unit used in historical records should be preserved. Equivalents corresponding to current knowledge should be recorded as additional instances of E54 Dimension as appropriate.\r
"""@en ;
    rdfs:subClassOf cidoc_crm:E1_CRM_Entity .

cidoc_crm:E21_Person a owl:Class ;
    rdfs:label "Person"@de,
        "Πρόσωπο"@el,
        "Person"@en,
        "Personne"@fr,
        "Pessoa"@pt,
        "Личность"@ru,
        "人物"@zh ;
    rdfs:comment """This class comprises real persons who live or are assumed to have lived. \r
Legendary figures that may have existed, such as Ulysses and King Arthur, fall into this class if the documentation refers to them as historical figures. In cases where doubt exists as to whether several persons are in fact identical, multiple instances can be created and linked to indicate their relationship. The CRM does not propose a specific form to support reasoning about possible identity.\r
"""@en ;
    rdfs:subClassOf cidoc_crm:E20_Biological_Object,
        cidoc_crm:E39_Actor .

cidoc_crm:E41_Appellation a owl:Class ;
    rdfs:label "Benennung"@de,
        "Ονομασία"@el,
        "Appellation"@en,
        "Appellation"@fr,
        "Designação"@pt,
        "Обозначение"@ru,
        "称号"@zh ;
    rdfs:comment """This class comprises signs, either meaningful or not, or arrangements of signs following a specific syntax, that are used or can be used to refer to and identify a specific instance of some class or category within a certain context.\r
Instances of E41 Appellation do not identify things by their meaning, even if they happen to have one, but instead by convention, tradition, or agreement. Instances of E41 Appellation are cultural constructs; as such, they have a context, a history, and a use in time and space by some group of users. A given instance of E41 Appellation can have alternative forms, i.e., other instances of E41 Appellation that are always regarded as equivalent independent from the thing it denotes. \r
Specific subclasses of E41 Appellation should be used when instances of E41 Appellation of a characteristic form are used for particular objects. Instances of E49 Time Appellation, for example, which take the form of instances of E50 Date, can be easily recognised.\r
E41 Appellation should not be confused with the act of naming something. Cf. E15 Identifier Assignment\r
"""@en ;
    rdfs:subClassOf cidoc_crm:E90_Symbolic_Object .

cidoc_crm:E77_Persistent_Item a owl:Class ;
    rdfs:label "Seiendes"@de,
        "Ον"@el,
        "Persistent Item"@en,
        "Entité persistante"@fr,
        "Entidade Persistente"@pt,
        "Постоянная Сущность"@ru,
        "持续性项目"@zh ;
    rdfs:comment """This class comprises items that have a persistent identity, sometimes known as “endurants” in philosophy. \r
They can be repeatedly recognized within the duration of their existence by identity criteria rather than by continuity or observation. Persistent Items can be either physical entities, such as people, animals or things, or conceptual entities such as ideas, concepts, products of the imagination or common names.\r
The criteria that determine the identity of an item are often difficult to establish -; the decision depends largely on the judgement of the observer. For example, a building is regarded as no longer existing if it is dismantled and the materials reused in a different configuration. On the other hand, human beings go through radical and profound changes during their life-span, affecting both material composition and form, yet preserve their identity by other criteria. Similarly, inanimate objects may be subject to exchange of parts and matter. The class E77 Persistent Item does not take any position about the nature of the applicable identity criteria and if actual knowledge about identity of an instance of this class exists. There may be cases, where the identity of an E77 Persistent Item is not decidable by a certain state of knowledge.\r
The main classes of objects that fall outside the scope the E77 Persistent Item class are temporal objects such as periods, events and acts, and descriptive properties. """@en ;
    rdfs:subClassOf cidoc_crm:E1_CRM_Entity .

cidoc_crm:E70_Thing a owl:Class ;
    rdfs:label "Sache"@de,
        "Πράγμα"@el,
        "Thing"@en,
        "Chose"@fr,
        "Coisa"@pt,
        ""@ru,
        "万物"@zh ;
    rdfs:comment """This general class comprises discrete, identifiable, instances of E77 Persistent Item that are documented as single units, that either consist of matter or depend on being carried by matter and are characterized by relative stability.\r
They may be intellectual products or physical things. They may for instance have a solid physical form, an electronic encoding, or they may be a logical concept or structure.\r
"""@en ;
    rdfs:subClassOf cidoc_crm:E77_Persistent_Item .

cidoc_crm:E74_Group a owl:Class ;
    rdfs:label "Menschliche Gruppe"@de,
        "Ομάδα"@el,
        "Group"@en,
        "Groupe"@fr,
        "Grupo"@pt,
        "Группа"@ru,
        "群组"@zh ;
    rdfs:comment """This class comprises any gatherings or organizations of E39 Actors that act collectively or in a similar way due to any form of unifying relationship. In the wider sense this class also comprises official positions which used to be regarded in certain contexts as one actor, independent of the current holder of the office, such as the president of a country. In such cases, it may happen that the Group never had more than one member. A joint pseudonym (i.e., a name that seems indicative of an individual but that is actually used as a persona by two or more people) is a particular case of E74 Group.\r
A gathering of people becomes an E74 Group when it exhibits organizational characteristics usually typified by a set of ideas or beliefs held in common, or actions performed together. These might be communication, creating some common artifact, a common purpose such as study, worship, business, sports, etc. Nationality can be modeled as membership in an E74 Group (cf. HumanML markup). Married couples and other concepts of family are regarded as particular examples of E74 Group.\r
"""@en ;
    rdfs:subClassOf cidoc_crm:E39_Actor .

cidoc_crm:E90_Symbolic_Object a owl:Class ;
    rdfs:label "Symbolisches Objekt"@de,
        "Symbolic Object"@en,
        "符号物件"@zh ;
    rdfs:comment """This class comprises identifiable symbols and any aggregation of symbols, such as characters, identifiers, traffic signs, emblems, texts, data sets, images, musical scores, multimedia objects, computer program code or mathematical formulae that have an objectively recognizable structure and that are documented as single units.\r
	It includes sets of signs of any nature, which may serve to designate something, or to communicate some propositional content.\r
	An instance of E90 Symbolic Object does not depend on a specific physical carrier, which can include human memory, and it can exist on one or more carriers simultaneously. An instance of E90 Symbolic Object may or may not have a specific meaning, for example an arbitrary character string.\r
	In some cases, the content of an instance of E90 Symbolic Object may completely be represented by a serialized content model, such.. as the property P3 has note allows for describing this content model…P3.1 has type: E55 Type to specify the encoding..\r
"""@en ;
    rdfs:subClassOf cidoc_crm:E28_Conceptual_Object,
        cidoc_crm:E72_Legal_Object .

cidoc_crm:E24_Physical_Man-Made_Thing a owl:Class ;
    rdfs:label "Hergestelltes"@de,
        "Ανθρωπογενές Υλικό Πράγμα"@el,
        "Physical Man-Made Thing"@en,
        "Chose matérielle fabriquée"@fr,
        "Coisa Material Fabricada"@pt,
        "Физическая Рукотворная Вещь"@ru,
        "人造实体物"@zh ;
    rdfs:comment """This class comprises all persistent physical items that are purposely created by human activity.\r
This class comprises man-made objects, such as a swords, and man-made features, such as rock art. No assumptions are made as to the extent of modification required to justify regarding an object as man-made. For example, a “cup and ring” carving on bedrock is regarded as instance of E24 Physical Man-Made Thing. \r
"""@en ;
    rdfs:subClassOf cidoc_crm:E18_Physical_Thing,
        cidoc_crm:E71_Man-Made_Thing .

cidoc_crm:E92_Spacetime_Volume a owl:Class ;
    rdfs:label "Spacetime Volume"@en ;
    rdfs:comment """This class comprises 4 dimensional point sets (volumes) in physical spacetime regardless its true geometric form. They may derive their identity from being the extent of a material phenomenon or from being the interpretation of an expression defining an extent in spacetime. \r
	Intersections of instances of E92 Spacetime Volume, Place and Timespan are also regarded as instances of E92 Spacetime Volume.  An instance of E92 Spacetime Volume is either contiguous or composed of a finite number of contiguous subsets. \r
	Its boundaries may be fuzzy due to the properties of the phenomena it derives from or due to the limited precision up to which defining expression can be identified with a real extent in spacetime. The duration of existence of an instance of a spacetime volume is trivially its projection on time.\r
"""@en ;
    rdfs:subClassOf cidoc_crm:E1_CRM_Entity .

cidoc_crm:E52_Time-Span a owl:Class ;
    rdfs:label "Zeitspanne"@de,
        "Χρονικό Διάστημα"@el,
        "Time-Span"@en,
        "Durée"@fr,
        "Período de Tempo"@pt,
        "Интервал Времени"@ru,
        "时段"@zh ;
    rdfs:comment """This class comprises abstract temporal extents, in the sense of Galilean physics, having a beginning, an end and a duration. \r
Time Span has no other semantic connotations. Time-Spans are used to define the temporal extent of instances of E4 Period, E5 Event and any other phenomena valid for a certain time. An E52 Time-Span may be identified by one or more instances of E49 Time Appellation. \r
Since our knowledge of history is imperfect, instances of E52 Time-Span can best be considered as approximations of the actual Time-Spans of temporal entities. The properties of E52 Time-Span are intended to allow these approximations to be expressed precisely.  An extreme case of approximation, might, for example, define an E52 Time-Span having unknown beginning, end and duration. Used as a common E52 Time-Span for two events, it would nevertheless define them as being simultaneous, even if nothing else was known. \r
	Automatic processing and querying of instances of E52 Time-Span is facilitated if data can be parsed into an E61 Time Primitive.\r
"""@en ;
    rdfs:subClassOf cidoc_crm:E1_CRM_Entity .

cidoc_crm:E55_Type a owl:Class ;
    rdfs:label "Typus"@de,
        "Τύπος"@el,
        "Type"@en,
        "Type"@fr,
        "Tipo"@pt,
        "Тип"@ru,
        "类型"@zh ;
    rdfs:comment """This class comprises concepts denoted by terms from thesauri and controlled vocabularies used to characterize and classify instances of CRM classes. Instances of E55 Type represent concepts  in contrast to instances of E41 Appellation which are used to name instances of CRM classes. \r
E55 Type is the CRM’s interface to domain specific ontologies and thesauri. These can be represented in the CRM as subclasses of E55 Type, forming hierarchies of terms, i.e. instances of E55 Type linked via P127 has broader  term (has narrower term). Such hierarchies may be extended with additional properties. \r
"""@en ;
    rdfs:subClassOf cidoc_crm:E28_Conceptual_Object .

cidoc_crm:E2_Temporal_Entity a owl:Class ;
    rdfs:label "Geschehendes"@de,
        "Έγχρονη  Οντότητα"@el,
        "Temporal Entity"@en,
        "Entité temporelle"@fr,
        "Entidade Temporal"@pt,
        "Временная Сущность"@ru,
        "时间实体"@zh ;
    rdfs:comment """This class comprises all phenomena, such as the instances of E4 Periods, E5 Events and states, which happen over a limited extent in time. \r
	In some contexts, these are also called perdurants. This class is disjoint from E77 Persistent Item. This is an abstract class and has no direct instances. E2 Temporal Entity is specialized into E4 Period, which applies to a particular geographic area (defined with a greater or lesser degree of precision), and E3 Condition State, which applies to instances of E18 Physical Thing.\r
"""@en ;
    rdfs:subClassOf cidoc_crm:E1_CRM_Entity .

cidoc_crm:E7_Activity a owl:Class ;
    rdfs:label "Handlung"@de,
        "Δράση"@el,
        "Activity"@en,
        "Activité"@fr,
        "Atividade"@pt,
        "Деятельность"@ru,
        "活动"@zh ;
    rdfs:comment """This class comprises actions intentionally carried out by instances of E39 Actor that result in changes of state in the cultural, social, or physical systems documented. \r
This notion includes complex, composite and long-lasting actions such as the building of a settlement or a war, as well as simple, short-lived actions such as the opening of a door.\r
"""@en ;
    rdfs:subClassOf cidoc_crm:E5_Event .

cidoc_crm:E53_Place a owl:Class ;
    rdfs:label "Ort"@de,
        "Τόπος"@el,
        "Place"@en,
        "Lieu"@fr,
        "Local"@pt,
        "Место"@ru,
        "地点"@zh ;
    rdfs:comment """This class comprises extents in space, in particular on the surface of the earth, in the pure sense of physics: independent from temporal phenomena and matter. \r
The instances of E53 Place are usually determined by reference to the position of “immobile” objects such as buildings, cities, mountains, rivers, or dedicated geodetic marks. A Place can be determined by combining a frame of reference and a location with respect to this frame. It may be identified by one or more instances of E44 Place Appellation.\r
 It is sometimes argued that instances of E53 Place are best identified by global coordinates or absolute reference systems. However, relative references are often more relevant in the context of cultural documentation and tend to be more precise. In particular, we are often interested in position in relation to large, mobile objects, such as ships. For example, the Place at which Nelson died is known with reference to a large mobile object – H.M.S Victory. A resolution of this Place in terms of absolute coordinates would require knowledge of the movements of the vessel and the precise time of death, either of which may be revised, and the result would lack historical and cultural relevance.\r
Any object can serve as a frame of reference for E53 Place determination. The model foresees the notion of a "section" of an E19 Physical Object as a valid E53 Place determination."""@en ;
    rdfs:subClassOf cidoc_crm:E1_CRM_Entity .

cidoc_crm:E39_Actor a owl:Class ;
    rdfs:label "Akteur"@de,
        "Δράστης"@el,
        "Actor"@en,
        "Agent"@fr,
        "Agente"@pt,
        "Агент"@ru,
        "角色"@zh ;
    rdfs:comment """This class comprises people, either individually or in groups, who have the potential to perform intentional actions of kinds for which someone may be held responsible.\r
The CRM does not attempt to model the inadvertent actions of such actors. Individual people should be documented as instances of E21 Person, whereas groups should be documented as instances of either E74 Group or its subclass E40 Legal Body.\r
"""@en ;
    rdfs:subClassOf cidoc_crm:E77_Persistent_Item .

cidoc_crm:E1_CRM_Entity a owl:Class ;
    rdfs:label "CRM Entität"@de,
        "Οντότητα CIDOC CRM"@el,
        "CRM Entity"@en,
        "Entité CRM"@fr,
        "Entidade CRM"@pt,
        "CRM Сущность"@ru,
        "CRM实体"@zh ;
    rdfs:comment """This class comprises all things in the universe of discourse of the CIDOC Conceptual Reference Model. \r
It is an abstract concept providing for three general properties:\r
1.	Identification by name or appellation, and in particular by a preferred identifier\r
2.	Classification by type, allowing further refinement of the specific subclass an instance belongs to \r
3.	Attachment of free text for the expression of anything not captured by formal properties\r
With the exception of E59 Primitive Value, all other classes within the CRM are directly or indirectly specialisations of E1 CRM Entity. \r
"""@en .

cidoc_crm:E18_Physical_Thing a owl:Class ;
    rdfs:label "Materielles"@de,
        "Υλικό Πράγμα"@el,
        "Physical Thing"@en,
        "Chose matérielle"@fr,
        "Coisa Material"@pt,
        "Физическая Вещь"@ru,
        "实体物"@zh ;
    rdfs:comment """This class comprises all persistent physical items with a relatively stable form, man-made or natural.\r
\r
Depending on the existence of natural boundaries of such things, the CRM distinguishes the instances of E19 Physical Object from instances of E26 Physical Feature, such as holes, rivers, pieces of land etc. Most instances of E19 Physical Object can be moved (if not too heavy), whereas features are integral to the surrounding matter.\r
\r
An instance of E18 Physical Thing occupies not only a particular geometric space, but in the course of its existence it also forms a trajectory through spacetime, which occupies a real, that is phenomenal, volume in spacetime. We include in the occupied space the space filled by the matter of the physical thing and all its inner spaces, such as the interior of a box. Physical things consisting of aggregations of physically unconnected objects, such as a set of chessmen, occupy a number of individually contiguous spacetime volumes equal to the number of unconnected objects that constitute the set.\r
\r
We model E18 Physical Thing to be a subclass of E72 Legal Object and of E92 Spacetime volume. The latter is intended as a phenomenal spacetime volume as defined in CRMgeo (Doerr and Hiebel 2013). By virtue of this multiple inheritance we can discuss the physical extent of an E18 Physical Thing without representing each instance of it together with an instance of its associated spacetime volume. This model combines two quite different kinds of substance: an instance of E18 Physical Thing is matter while a spacetime volume is an aggregation of points in spacetime. However, the real spatiotemporal extent of an instance of E18 Physical Thing is regarded to be unique to it, due to all its details and fuzziness; its identity and existence depends uniquely on the identity of the instance of E18 Physical Thing. Therefore this multiple inheritance is unambiguous and effective and furthermore corresponds to the intuitions of natural language.\r
\r
The CIDOC CRM is generally not concerned with amounts of matter in fluid or gaseous states. \r
"""@en ;
    rdfs:subClassOf cidoc_crm:E72_Legal_Object,
        cidoc_crm:E92_Spacetime_Volume .

